@prefix g36: <http://data.ashrae.org/standard223/1.0/extension/g36#> .
@prefix owl: <http://www.w3.org/2002/07/owl#> .
@prefix psm: <http://data.ashrae.org/standard223/1.0/data/brick-test#> .
@prefix quantitykind: <http://qudt.org/vocab/quantitykind/> .
@prefix qudt: <http://qudt.org/schema/qudt/> .
@prefix rdf: <http://www.w3.org/1999/02/22-rdf-syntax-ns#> .
@prefix rdfs: <http://www.w3.org/2000/01/rdf-schema#> .
@prefix ref: <https://brickschema.org/schema/Brick/ref#> .
@prefix s223: <http://data.ashrae.org/standard223#> .
@prefix sh: <http://www.w3.org/ns/shacl#> .
@prefix sp: <http://spinrdf.org/sp#> .
@prefix spin: <http://spinrdf.org/spin#> .
@prefix spl: <http://spinrdf.org/spl#> .
@prefix unit: <http://qudt.org/vocab/unit/> .
@prefix xsd: <http://www.w3.org/2001/XMLSchema#> .

s223:Class a rdfs:Class,
        sh:NodeShape ;
    rdfs:label "Class" ;
    rdfs:subClassOf rdfs:Class ;
    sh:property [ rdfs:comment "This Class must have a label" ;
            sh:path rdfs:label ;
            sh:sparql [ a sh:SPARQLConstraint ;
                    sh:message "{$this} must have an rdfs:label" ;
                    sh:prefixes s223: ;
                    sh:select """
SELECT $this
WHERE {
FILTER (NOT EXISTS {$this rdfs:label ?something}) .
}
""" ] ] .

sh:AbstractResult a rdfs:Class ;
    rdfs:label "Abstract result"@en ;
    rdfs:comment "The base class of validation results, typically not instantiated directly."@en ;
    rdfs:isDefinedBy sh: ;
    rdfs:subClassOf rdfs:Resource .

sh:ConstraintComponent a rdfs:Class ;
    rdfs:label "Constraint component"@en ;
    rdfs:comment "The class of constraint components."@en ;
    rdfs:isDefinedBy sh: ;
    rdfs:subClassOf sh:Parameterizable .

sh:Function a rdfs:Class ;
    rdfs:label "Function"@en ;
    rdfs:comment "The class of SHACL functions."@en ;
    rdfs:isDefinedBy sh: ;
    rdfs:subClassOf sh:Parameterizable .

sh:JSConstraint a rdfs:Class ;
    rdfs:label "JavaScript-based constraint"@en ;
    rdfs:comment "The class of constraints backed by a JavaScript function."@en ;
    rdfs:isDefinedBy sh: ;
    rdfs:subClassOf sh:JSExecutable .

sh:JSExecutable a rdfs:Class ;
    rdfs:label "JavaScript executable"@en ;
    rdfs:comment "Abstract base class of resources that declare an executable JavaScript."@en ;
    rdfs:isDefinedBy sh: ;
    rdfs:subClassOf rdfs:Resource .

sh:JSFunction a rdfs:Class ;
    rdfs:label "JavaScript function"@en ;
    rdfs:comment "The class of SHACL functions that execute a JavaScript function when called."@en ;
    rdfs:isDefinedBy sh: ;
    rdfs:subClassOf sh:Function,
        sh:JSExecutable .

sh:JSLibrary a rdfs:Class ;
    rdfs:label "JavaScript library"@en ;
    rdfs:comment "Represents a JavaScript library, typically identified by one or more URLs of files to include."@en ;
    rdfs:isDefinedBy sh: ;
    rdfs:subClassOf rdfs:Resource .

sh:JSRule a rdfs:Class ;
    rdfs:label "JavaScript rule"@en ;
    rdfs:comment "The class of SHACL rules expressed using JavaScript."@en ;
    rdfs:isDefinedBy sh: ;
    rdfs:subClassOf sh:JSExecutable,
        sh:Rule .

sh:JSTarget a rdfs:Class ;
    rdfs:label "JavaScript target"@en ;
    rdfs:comment "The class of targets that are based on JavaScript functions."@en ;
    rdfs:isDefinedBy sh: ;
    rdfs:subClassOf sh:JSExecutable,
        sh:Target .

sh:JSTargetType a rdfs:Class ;
    rdfs:label "JavaScript target type"@en ;
    rdfs:comment "The (meta) class for parameterizable targets that are based on JavaScript functions."@en ;
    rdfs:isDefinedBy sh: ;
    rdfs:subClassOf sh:JSExecutable,
        sh:TargetType .

sh:JSValidator a rdfs:Class ;
    rdfs:label "JavaScript validator"@en ;
    rdfs:comment "A SHACL validator based on JavaScript. This can be used to declare SHACL constraint components that perform JavaScript-based validation when used."@en ;
    rdfs:isDefinedBy sh: ;
    rdfs:subClassOf sh:JSExecutable,
        sh:Validator .

sh:NodeKind a rdfs:Class ;
    rdfs:label "Node kind"@en ;
    rdfs:comment "The class of all node kinds, including sh:BlankNode, sh:IRI, sh:Literal or the combinations of these: sh:BlankNodeOrIRI, sh:BlankNodeOrLiteral, sh:IRIOrLiteral."@en ;
    rdfs:isDefinedBy sh: ;
    rdfs:subClassOf rdfs:Resource .

sh:NodeShape a rdfs:Class ;
    rdfs:label "Node shape"@en ;
    rdfs:comment "A node shape is a shape that specifies constraint that need to be met with respect to focus nodes."@en ;
    rdfs:isDefinedBy sh: ;
    rdfs:subClassOf sh:Shape .

sh:Parameter a rdfs:Class ;
    rdfs:label "Parameter"@en ;
    rdfs:comment "The class of parameter declarations, consisting of a path predicate and (possibly) information about allowed value type, cardinality and other characteristics."@en ;
    rdfs:isDefinedBy sh: ;
    rdfs:subClassOf sh:PropertyShape .

sh:Parameterizable a rdfs:Class ;
    rdfs:label "Parameterizable"@en ;
    rdfs:comment "Superclass of components that can take parameters, especially functions and constraint components."@en ;
    rdfs:isDefinedBy sh: ;
    rdfs:subClassOf rdfs:Resource .

sh:PrefixDeclaration a rdfs:Class ;
    rdfs:label "Prefix declaration"@en ;
    rdfs:comment "The class of prefix declarations, consisting of pairs of a prefix with a namespace."@en ;
    rdfs:isDefinedBy sh: ;
    rdfs:subClassOf rdfs:Resource .

sh:PropertyGroup a rdfs:Class ;
    rdfs:label "Property group"@en ;
    rdfs:comment "Instances of this class represent groups of property shapes that belong together."@en ;
    rdfs:isDefinedBy sh: ;
    rdfs:subClassOf rdfs:Resource .

sh:PropertyShape a rdfs:Class ;
    rdfs:label "Property shape"@en ;
    rdfs:comment "A property shape is a shape that specifies constraints on the values of a focus node for a given property or path."@en ;
    rdfs:isDefinedBy sh: ;
    rdfs:subClassOf sh:Shape .

sh:ResultAnnotation a rdfs:Class ;
    rdfs:label "Result annotation"@en ;
    rdfs:comment "A class of result annotations, which define the rules to derive the values of a given annotation property as extra values for a validation result."@en ;
    rdfs:isDefinedBy sh: ;
    rdfs:subClassOf rdfs:Resource .

sh:Rule a rdfs:Class ;
    rdfs:label "Rule"@en ;
    rdfs:comment "The class of SHACL rules. Never instantiated directly."@en ;
    rdfs:isDefinedBy sh: ;
    rdfs:subClassOf rdfs:Resource .

sh:SPARQLAskExecutable a rdfs:Class ;
    rdfs:label "SPARQL ASK executable"@en ;
    rdfs:comment "The class of SPARQL executables that are based on an ASK query."@en ;
    rdfs:isDefinedBy sh: ;
    rdfs:subClassOf sh:SPARQLExecutable .

sh:SPARQLAskValidator a rdfs:Class ;
    rdfs:label "SPARQL ASK validator"@en ;
    rdfs:comment "The class of validators based on SPARQL ASK queries. The queries are evaluated for each value node and are supposed to return true if the given node conforms."@en ;
    rdfs:isDefinedBy sh: ;
    rdfs:subClassOf sh:SPARQLAskExecutable,
        sh:Validator .

sh:SPARQLConstraint a rdfs:Class ;
    rdfs:label "SPARQL constraint"@en ;
    rdfs:comment "The class of constraints based on SPARQL SELECT queries."@en ;
    rdfs:isDefinedBy sh: ;
    rdfs:subClassOf sh:SPARQLSelectExecutable .

sh:SPARQLConstructExecutable a rdfs:Class ;
    rdfs:label "SPARQL CONSTRUCT executable"@en ;
    rdfs:comment "The class of SPARQL executables that are based on a CONSTRUCT query."@en ;
    rdfs:isDefinedBy sh: ;
    rdfs:subClassOf sh:SPARQLExecutable .

sh:SPARQLExecutable a rdfs:Class ;
    rdfs:label "SPARQL executable"@en ;
    rdfs:comment "The class of resources that encapsulate a SPARQL query."@en ;
    rdfs:isDefinedBy sh: ;
    rdfs:subClassOf rdfs:Resource .

sh:SPARQLFunction a rdfs:Class ;
    rdfs:label "SPARQL function"@en ;
    rdfs:comment "A function backed by a SPARQL query - either ASK or SELECT."@en ;
    rdfs:isDefinedBy sh: ;
    rdfs:subClassOf sh:Function,
        sh:SPARQLAskExecutable,
        sh:SPARQLSelectExecutable .

sh:SPARQLRule a rdfs:Class ;
    rdfs:label "SPARQL CONSTRUCT rule"@en ;
    rdfs:comment "The class of SHACL rules based on SPARQL CONSTRUCT queries."@en ;
    rdfs:isDefinedBy sh: ;
    rdfs:subClassOf sh:Rule,
        sh:SPARQLConstructExecutable .

sh:SPARQLSelectExecutable a rdfs:Class ;
    rdfs:label "SPARQL SELECT executable"@en ;
    rdfs:comment "The class of SPARQL executables based on a SELECT query."@en ;
    rdfs:isDefinedBy sh: ;
    rdfs:subClassOf sh:SPARQLExecutable .

sh:SPARQLSelectValidator a rdfs:Class ;
    rdfs:label "SPARQL SELECT validator"@en ;
    rdfs:comment "The class of validators based on SPARQL SELECT queries. The queries are evaluated for each focus node and are supposed to produce bindings for all focus nodes that do not conform."@en ;
    rdfs:isDefinedBy sh: ;
    rdfs:subClassOf sh:SPARQLSelectExecutable,
        sh:Validator .

sh:SPARQLTarget a rdfs:Class ;
    rdfs:label "SPARQL target"@en ;
    rdfs:comment "The class of targets that are based on SPARQL queries."@en ;
    rdfs:isDefinedBy sh: ;
    rdfs:subClassOf sh:SPARQLAskExecutable,
        sh:SPARQLSelectExecutable,
        sh:Target .

sh:SPARQLTargetType a rdfs:Class ;
    rdfs:label "SPARQL target type"@en ;
    rdfs:comment "The (meta) class for parameterizable targets that are based on SPARQL queries."@en ;
    rdfs:isDefinedBy sh: ;
    rdfs:subClassOf sh:SPARQLAskExecutable,
        sh:SPARQLSelectExecutable,
        sh:TargetType .

sh:SPARQLUpdateExecutable a rdfs:Class ;
    rdfs:label "SPARQL UPDATE executable"@en ;
    rdfs:comment "The class of SPARQL executables based on a SPARQL UPDATE."@en ;
    rdfs:isDefinedBy sh: ;
    rdfs:subClassOf sh:SPARQLExecutable .

sh:Severity a rdfs:Class ;
    rdfs:label "Severity"@en ;
    rdfs:comment "The class of validation result severity levels, including violation and warning levels."@en ;
    rdfs:isDefinedBy sh: ;
    rdfs:subClassOf rdfs:Resource .

sh:Shape a rdfs:Class ;
    rdfs:label "Shape"@en ;
    rdfs:comment "A shape is a collection of constraints that may be targeted for certain nodes."@en ;
    rdfs:isDefinedBy sh: ;
    rdfs:subClassOf rdfs:Resource .

sh:Target a rdfs:Class ;
    rdfs:label "Target"@en ;
    rdfs:comment "The base class of targets such as those based on SPARQL queries."@en ;
    rdfs:isDefinedBy sh: ;
    rdfs:subClassOf rdfs:Resource .

sh:TargetType a rdfs:Class ;
    rdfs:label "Target type"@en ;
    rdfs:comment "The (meta) class for parameterizable targets.	Instances of this are instantiated as values of the sh:target property."@en ;
    rdfs:isDefinedBy sh: ;
    rdfs:subClassOf rdfs:Class,
        sh:Parameterizable .

sh:TripleRule a rdfs:Class ;
    rdfs:label "A rule based on triple (subject, predicate, object) pattern."@en ;
    rdfs:isDefinedBy sh: ;
    rdfs:subClassOf sh:Rule .

sh:ValidationReport a rdfs:Class ;
    rdfs:label "Validation report"@en ;
    rdfs:comment "The class of SHACL validation reports."@en ;
    rdfs:isDefinedBy sh: ;
    rdfs:subClassOf rdfs:Resource .

sh:ValidationResult a rdfs:Class ;
    rdfs:label "Validation result"@en ;
    rdfs:comment "The class of validation results."@en ;
    rdfs:isDefinedBy sh: ;
    rdfs:subClassOf sh:AbstractResult .

sh:Validator a rdfs:Class ;
    rdfs:label "Validator"@en ;
    rdfs:comment "The class of validators, which provide instructions on how to process a constraint definition. This class serves as base class for the SPARQL-based validators and other possible implementations."@en ;
    rdfs:isDefinedBy sh: ;
    rdfs:subClassOf rdfs:Resource .

s223:AC-1.73kVLN-1Ph-60Hz a s223:Electricity-AC ;
    rdfs:label "AC-1.73kVLN-1Ph-60Hz" ;
    s223:hasFrequency s223:Frequency-60Hz ;
    s223:hasNumberOfElectricalPhases s223:NumberOfElectricalPhases-SinglePhase ;
    s223:hasVoltage s223:LineNeutralVoltage-1.73kV .

s223:AC-1.91kVLN-1Ph-60Hz a s223:Electricity-AC ;
    rdfs:label "AC-1.91kVLN-1Ph-60Hz" ;
    s223:hasFrequency s223:Frequency-60Hz ;
    s223:hasNumberOfElectricalPhases s223:NumberOfElectricalPhases-SinglePhase ;
    s223:hasVoltage s223:LineNeutralVoltage-1.91kV .

s223:AC-10.0kVLL-1Ph-60Hz a s223:Electricity-AC ;
    rdfs:label "AC-10.0kVLL-1Ph-60Hz" ;
    s223:hasFrequency s223:Frequency-60Hz ;
    s223:hasNumberOfElectricalPhases s223:NumberOfElectricalPhases-SinglePhase ;
    s223:hasVoltage s223:LineLineVoltage-10.0kV .

s223:AC-10.0kVLL-3Ph-60Hz a s223:Electricity-AC ;
    rdfs:label "AC-10.0kVLL-3Ph-60Hz" ;
    s223:hasFrequency s223:Frequency-60Hz ;
    s223:hasNumberOfElectricalPhases s223:NumberOfElectricalPhases-ThreePhase ;
    s223:hasVoltage s223:LineLineVoltage-10.0kV .

s223:AC-10.0kVLL-5.77kVLN-1Ph-60Hz a s223:Electricity-AC ;
    rdfs:label "AC-10.0kVLL-5.77kVLN-1Ph-60Hz" ;
    s223:hasFrequency s223:Frequency-60Hz ;
    s223:hasNumberOfElectricalPhases s223:NumberOfElectricalPhases-SinglePhase ;
    s223:hasVoltage s223:LineLineVoltage-10.0kV,
        s223:LineNeutralVoltage-5.77kV .

s223:AC-10.0kVLL-5.77kVLN-3Ph-60Hz a s223:Electricity-AC ;
    rdfs:label "AC-10.0kVLL-5.77kVLN-3Ph-60Hz" ;
    s223:hasFrequency s223:Frequency-60Hz ;
    s223:hasNumberOfElectricalPhases s223:NumberOfElectricalPhases-ThreePhase ;
    s223:hasVoltage s223:LineLineVoltage-10.0kV,
        s223:LineNeutralVoltage-5.77kV .

s223:AC-110.0VLN-1Ph-50Hz a s223:Electricity-AC ;
    rdfs:label "AC-110.0VLN-1Ph-50Hz" ;
    s223:hasFrequency s223:Frequency-50Hz ;
    s223:hasNumberOfElectricalPhases s223:NumberOfElectricalPhases-SinglePhase ;
    s223:hasVoltage s223:LineNeutralVoltage-110.0V .

s223:AC-120.0VLN-1Ph-60Hz a s223:Electricity-AC ;
    rdfs:label "AC-120.0VLN-1Ph-60Hz" ;
    s223:hasFrequency s223:Frequency-60Hz ;
    s223:hasNumberOfElectricalPhases s223:NumberOfElectricalPhases-SinglePhase ;
    s223:hasVoltage s223:LineNeutralVoltage-120.0V .

s223:AC-127.0VLN-1Ph-50Hz a s223:Electricity-AC ;
    rdfs:label "AC-127.0VLN-1Ph-50Hz" ;
    s223:hasFrequency s223:Frequency-50Hz ;
    s223:hasNumberOfElectricalPhases s223:NumberOfElectricalPhases-SinglePhase ;
    s223:hasVoltage s223:LineNeutralVoltage-127.0V .

s223:AC-139.0VLN-1Ph-50Hz a s223:Electricity-AC ;
    rdfs:label "AC-139.0VLN-1Ph-50Hz" ;
    s223:hasFrequency s223:Frequency-50Hz ;
    s223:hasNumberOfElectricalPhases s223:NumberOfElectricalPhases-SinglePhase ;
    s223:hasVoltage s223:LineNeutralVoltage-139.0V .

s223:AC-190.0VLL-110.0VLN-1Ph-50Hz a s223:Electricity-AC ;
    rdfs:label "AC-190.0VLL-110.0VLN-1Ph-50Hz" ;
    s223:hasFrequency s223:Frequency-50Hz ;
    s223:hasNumberOfElectricalPhases s223:NumberOfElectricalPhases-SinglePhase ;
    s223:hasVoltage s223:LineLineVoltage-190.0V,
        s223:LineNeutralVoltage-110.0V .

s223:AC-190.0VLL-110.0VLN-3Ph-50Hz a s223:Electricity-AC ;
    rdfs:label "AC-190.0VLL-110.0VLN-3Ph-50Hz" ;
    s223:hasFrequency s223:Frequency-50Hz ;
    s223:hasNumberOfElectricalPhases s223:NumberOfElectricalPhases-ThreePhase ;
    s223:hasVoltage s223:LineLineVoltage-190.0V,
        s223:LineNeutralVoltage-110.0V .

s223:AC-190.0VLL-1Ph-50Hz a s223:Electricity-AC ;
    rdfs:label "AC-190.0VLL-1Ph-50Hz" ;
    s223:hasFrequency s223:Frequency-50Hz ;
    s223:hasNumberOfElectricalPhases s223:NumberOfElectricalPhases-SinglePhase ;
    s223:hasVoltage s223:LineLineVoltage-190.0V .

s223:AC-190.0VLL-3Ph-50Hz a s223:Electricity-AC ;
    rdfs:label "AC-190.0VLL-3Ph-50Hz" ;
    s223:hasFrequency s223:Frequency-50Hz ;
    s223:hasNumberOfElectricalPhases s223:NumberOfElectricalPhases-ThreePhase ;
    s223:hasVoltage s223:LineLineVoltage-190.0V .

s223:AC-2.4kVLN-1Ph-60Hz a s223:Electricity-AC ;
    rdfs:label "AC-2.4kVLN-1Ph-60Hz" ;
    s223:hasFrequency s223:Frequency-60Hz ;
    s223:hasNumberOfElectricalPhases s223:NumberOfElectricalPhases-SinglePhase ;
    s223:hasVoltage s223:LineNeutralVoltage-2.4kV .

s223:AC-208.0VLL-120.0VLN-1Ph-60Hz a s223:Electricity-AC ;
    rdfs:label "AC-208.0VLL-120.0VLN-1Ph-60Hz" ;
    s223:hasFrequency s223:Frequency-60Hz ;
    s223:hasNumberOfElectricalPhases s223:NumberOfElectricalPhases-SinglePhase ;
    s223:hasVoltage s223:LineLineVoltage-208.0V,
        s223:LineNeutralVoltage-120.0V .

s223:AC-208.0VLL-120.0VLN-3Ph-60Hz a s223:Electricity-AC ;
    rdfs:label "AC-208.0VLL-120.0VLN-3Ph-60Hz" ;
    s223:hasFrequency s223:Frequency-60Hz ;
    s223:hasNumberOfElectricalPhases s223:NumberOfElectricalPhases-ThreePhase ;
    s223:hasVoltage s223:LineLineVoltage-208.0V,
        s223:LineNeutralVoltage-120.0V .

s223:AC-208.0VLL-1Ph-60Hz a s223:Electricity-AC ;
    rdfs:label "AC-208.0VLL-1Ph-60Hz" ;
    s223:hasFrequency s223:Frequency-60Hz ;
    s223:hasNumberOfElectricalPhases s223:NumberOfElectricalPhases-SinglePhase ;
    s223:hasVoltage s223:LineLineVoltage-208.0V .

s223:AC-208.0VLL-3Ph-60Hz a s223:Electricity-AC ;
    rdfs:label "AC-208.0VLL-3Ph-60Hz" ;
    s223:hasFrequency s223:Frequency-60Hz ;
    s223:hasNumberOfElectricalPhases s223:NumberOfElectricalPhases-ThreePhase ;
    s223:hasVoltage s223:LineLineVoltage-208.0V .

s223:AC-219.0VLN-1Ph-60Hz a s223:Electricity-AC ;
    rdfs:label "AC-219.0VLN-1Ph-60Hz" ;
    s223:hasFrequency s223:Frequency-60Hz ;
    s223:hasNumberOfElectricalPhases s223:NumberOfElectricalPhases-SinglePhase ;
    s223:hasVoltage s223:LineNeutralVoltage-219.0V .

s223:AC-220.0VLL-127.0VLN-1Ph-50Hz a s223:Electricity-AC ;
    rdfs:label "AC-220.0VLL-127.0VLN-1Ph-50Hz" ;
    s223:hasFrequency s223:Frequency-50Hz ;
    s223:hasNumberOfElectricalPhases s223:NumberOfElectricalPhases-SinglePhase ;
    s223:hasVoltage s223:LineLineVoltage-220.0V,
        s223:LineNeutralVoltage-127.0V .

s223:AC-220.0VLL-127.0VLN-3Ph-50Hz a s223:Electricity-AC ;
    rdfs:label "AC-220.0VLL-127.0VLN-3Ph-50Hz" ;
    s223:hasFrequency s223:Frequency-50Hz ;
    s223:hasNumberOfElectricalPhases s223:NumberOfElectricalPhases-ThreePhase ;
    s223:hasVoltage s223:LineLineVoltage-220.0V,
        s223:LineNeutralVoltage-127.0V .

s223:AC-220.0VLL-1Ph-50Hz a s223:Electricity-AC ;
    rdfs:label "AC-220.0VLL-1Ph-50Hz" ;
    s223:hasFrequency s223:Frequency-50Hz ;
    s223:hasNumberOfElectricalPhases s223:NumberOfElectricalPhases-SinglePhase ;
    s223:hasVoltage s223:LineLineVoltage-220.0V .

s223:AC-220.0VLL-3Ph-50Hz a s223:Electricity-AC ;
    rdfs:label "AC-220.0VLL-3Ph-50Hz" ;
    s223:hasFrequency s223:Frequency-50Hz ;
    s223:hasNumberOfElectricalPhases s223:NumberOfElectricalPhases-ThreePhase ;
    s223:hasVoltage s223:LineLineVoltage-220.0V .

s223:AC-231.0VLN-1Ph-50Hz a s223:Electricity-AC ;
    rdfs:label "AC-231.0VLN-1Ph-50Hz" ;
    s223:hasFrequency s223:Frequency-50Hz ;
    s223:hasNumberOfElectricalPhases s223:NumberOfElectricalPhases-SinglePhase ;
    s223:hasVoltage s223:LineNeutralVoltage-231.0V .

s223:AC-240.0VLL-120.0VLN-1Ph-60Hz a s223:Electricity-AC ;
    rdfs:label "AC-240.0VLL-120.0VLN-1Ph-60Hz" ;
    s223:hasFrequency s223:Frequency-60Hz ;
    s223:hasNumberOfElectricalPhases s223:NumberOfElectricalPhases-SinglePhase ;
    s223:hasVoltage s223:LineLineVoltage-240.0V,
        s223:LineNeutralVoltage-120.0V .

s223:AC-240.0VLL-139.0VLN-1Ph-50Hz a s223:Electricity-AC ;
    rdfs:label "AC-240.0VLL-139.0VLN-1Ph-50Hz" ;
    s223:hasFrequency s223:Frequency-50Hz ;
    s223:hasNumberOfElectricalPhases s223:NumberOfElectricalPhases-SinglePhase ;
    s223:hasVoltage s223:LineLineVoltage-240.0V,
        s223:LineNeutralVoltage-139.0V .

s223:AC-240.0VLL-139.0VLN-3Ph-50Hz a s223:Electricity-AC ;
    rdfs:label "AC-240.0VLL-139.0VLN-3Ph-50Hz" ;
    s223:hasFrequency s223:Frequency-50Hz ;
    s223:hasNumberOfElectricalPhases s223:NumberOfElectricalPhases-ThreePhase ;
    s223:hasVoltage s223:LineLineVoltage-240.0V,
        s223:LineNeutralVoltage-139.0V .

s223:AC-240.0VLL-1Ph-50Hz a s223:Electricity-AC ;
    rdfs:label "AC-240.0VLL-1Ph-50Hz" ;
    s223:hasFrequency s223:Frequency-50Hz ;
    s223:hasNumberOfElectricalPhases s223:NumberOfElectricalPhases-SinglePhase ;
    s223:hasVoltage s223:LineLineVoltage-240.0V .

s223:AC-240.0VLL-1Ph-60Hz a s223:Electricity-AC ;
    rdfs:label "AC-240.0VLL-1Ph-60Hz" ;
    s223:hasFrequency s223:Frequency-60Hz ;
    s223:hasNumberOfElectricalPhases s223:NumberOfElectricalPhases-SinglePhase ;
    s223:hasVoltage s223:LineLineVoltage-240.0V .

s223:AC-240.0VLL-208.0VLN-120.0VLN-1Ph-60Hz a s223:Electricity-AC ;
    rdfs:label "AC-240.0VLL-208.0VLN-120.0VLN-1Ph-60Hz" ;
    s223:hasFrequency s223:Frequency-60Hz ;
    s223:hasNumberOfElectricalPhases s223:NumberOfElectricalPhases-SinglePhase ;
    s223:hasVoltage s223:LineLineVoltage-240.0V,
        s223:LineNeutralVoltage-120.0V,
        s223:LineNeutralVoltage-208.0V .

s223:AC-240.0VLL-208.0VLN-120.0VLN-3Ph-60Hz a s223:Electricity-AC ;
    rdfs:label "AC-240.0VLL-208.0VLN-120.0VLN-3Ph-60Hz" ;
    s223:hasFrequency s223:Frequency-60Hz ;
    s223:hasNumberOfElectricalPhases s223:NumberOfElectricalPhases-ThreePhase ;
    s223:hasVoltage s223:LineLineVoltage-240.0V,
        s223:LineNeutralVoltage-120.0V,
        s223:LineNeutralVoltage-208.0V .

s223:AC-240.0VLL-3Ph-50Hz a s223:Electricity-AC ;
    rdfs:label "AC-240.0VLL-3Ph-50Hz" ;
    s223:hasFrequency s223:Frequency-50Hz ;
    s223:hasNumberOfElectricalPhases s223:NumberOfElectricalPhases-ThreePhase ;
    s223:hasVoltage s223:LineLineVoltage-240.0V .

s223:AC-240.0VLL-3Ph-60Hz a s223:Electricity-AC ;
    rdfs:label "AC-240.0VLL-3Ph-60Hz" ;
    s223:hasFrequency s223:Frequency-60Hz ;
    s223:hasNumberOfElectricalPhases s223:NumberOfElectricalPhases-ThreePhase ;
    s223:hasVoltage s223:LineLineVoltage-240.0V .

s223:AC-240.0VLN-1Ph-50Hz a s223:Electricity-AC ;
    rdfs:label "AC-240.0VLN-1Ph-50Hz" ;
    s223:hasFrequency s223:Frequency-50Hz ;
    s223:hasNumberOfElectricalPhases s223:NumberOfElectricalPhases-SinglePhase ;
    s223:hasVoltage s223:LineNeutralVoltage-240.0V .

s223:AC-277.0VLN-1Ph-60Hz a s223:Electricity-AC ;
    rdfs:label "AC-277.0VLN-1Ph-60Hz" ;
    s223:hasFrequency s223:Frequency-60Hz ;
    s223:hasNumberOfElectricalPhases s223:NumberOfElectricalPhases-SinglePhase ;
    s223:hasVoltage s223:LineNeutralVoltage-277.0V .

s223:AC-3.0kVLL-1.73kVLN-1Ph-60Hz a s223:Electricity-AC ;
    rdfs:label "AC-3.0kVLL-1.73kVLN-1Ph-60Hz" ;
    s223:hasFrequency s223:Frequency-60Hz ;
    s223:hasNumberOfElectricalPhases s223:NumberOfElectricalPhases-SinglePhase ;
    s223:hasVoltage s223:LineLineVoltage-3.0kV,
        s223:LineNeutralVoltage-1.73kV .

s223:AC-3.0kVLL-1.73kVLN-3Ph-60Hz a s223:Electricity-AC ;
    rdfs:label "AC-3.0kVLL-1.73kVLN-3Ph-60Hz" ;
    s223:hasFrequency s223:Frequency-60Hz ;
    s223:hasNumberOfElectricalPhases s223:NumberOfElectricalPhases-ThreePhase ;
    s223:hasVoltage s223:LineLineVoltage-3.0kV,
        s223:LineNeutralVoltage-1.73kV .

s223:AC-3.0kVLL-1Ph-60Hz a s223:Electricity-AC ;
    rdfs:label "AC-3.0kVLL-1Ph-60Hz" ;
    s223:hasFrequency s223:Frequency-60Hz ;
    s223:hasNumberOfElectricalPhases s223:NumberOfElectricalPhases-SinglePhase ;
    s223:hasVoltage s223:LineLineVoltage-3.0kV .

s223:AC-3.0kVLL-3Ph-60Hz a s223:Electricity-AC ;
    rdfs:label "AC-3.0kVLL-3Ph-60Hz" ;
    s223:hasFrequency s223:Frequency-60Hz ;
    s223:hasNumberOfElectricalPhases s223:NumberOfElectricalPhases-ThreePhase ;
    s223:hasVoltage s223:LineLineVoltage-3.0kV .

s223:AC-3.3kVLL-1.91kVLN-1Ph-60Hz a s223:Electricity-AC ;
    rdfs:label "AC-3.3kVLL-1.91kVLN-1Ph-60Hz" ;
    s223:hasFrequency s223:Frequency-60Hz ;
    s223:hasNumberOfElectricalPhases s223:NumberOfElectricalPhases-SinglePhase ;
    s223:hasVoltage s223:LineLineVoltage-3.3kV,
        s223:LineNeutralVoltage-1.91kV .

s223:AC-3.3kVLL-1.91kVLN-3Ph-60Hz a s223:Electricity-AC ;
    rdfs:label "AC-3.3kVLL-1.91kVLN-3Ph-60Hz" ;
    s223:hasFrequency s223:Frequency-60Hz ;
    s223:hasNumberOfElectricalPhases s223:NumberOfElectricalPhases-ThreePhase ;
    s223:hasVoltage s223:LineLineVoltage-3.3kV,
        s223:LineNeutralVoltage-1.91kV .

s223:AC-3.3kVLL-1Ph-60Hz a s223:Electricity-AC ;
    rdfs:label "AC-3.3kVLL-1Ph-60Hz" ;
    s223:hasFrequency s223:Frequency-60Hz ;
    s223:hasNumberOfElectricalPhases s223:NumberOfElectricalPhases-SinglePhase ;
    s223:hasVoltage s223:LineLineVoltage-3.3kV .

s223:AC-3.3kVLL-3Ph-60Hz a s223:Electricity-AC ;
    rdfs:label "AC-3.3kVLL-3Ph-60Hz" ;
    s223:hasFrequency s223:Frequency-60Hz ;
    s223:hasNumberOfElectricalPhases s223:NumberOfElectricalPhases-ThreePhase ;
    s223:hasVoltage s223:LineLineVoltage-3.3kV .

s223:AC-3.46kVLN-1Ph-60Hz a s223:Electricity-AC ;
    rdfs:label "AC-3.46kVLN-1Ph-60Hz" ;
    s223:hasFrequency s223:Frequency-60Hz ;
    s223:hasNumberOfElectricalPhases s223:NumberOfElectricalPhases-SinglePhase ;
    s223:hasVoltage s223:LineNeutralVoltage-3.46kV .

s223:AC-3.81kVLN-1Ph-60Hz a s223:Electricity-AC ;
    rdfs:label "AC-3.81kVLN-1Ph-60Hz" ;
    s223:hasFrequency s223:Frequency-60Hz ;
    s223:hasNumberOfElectricalPhases s223:NumberOfElectricalPhases-SinglePhase ;
    s223:hasVoltage s223:LineNeutralVoltage-3.81kV .

s223:AC-347.0VLN-1Ph-60Hz a s223:Electricity-AC ;
    rdfs:label "AC-347.0VLN-1Ph-60Hz" ;
    s223:hasFrequency s223:Frequency-60Hz ;
    s223:hasNumberOfElectricalPhases s223:NumberOfElectricalPhases-SinglePhase ;
    s223:hasVoltage s223:LineNeutralVoltage-347.0V .

s223:AC-380.0VLL-1Ph-60Hz a s223:Electricity-AC ;
    rdfs:label "AC-380.0VLL-1Ph-60Hz" ;
    s223:hasFrequency s223:Frequency-60Hz ;
    s223:hasNumberOfElectricalPhases s223:NumberOfElectricalPhases-SinglePhase ;
    s223:hasVoltage s223:LineLineVoltage-380.0V .

s223:AC-380.0VLL-219.0VLN-1Ph-60Hz a s223:Electricity-AC ;
    rdfs:label "AC-380.0VLL-219.0VLN-1Ph-60Hz" ;
    s223:hasFrequency s223:Frequency-60Hz ;
    s223:hasNumberOfElectricalPhases s223:NumberOfElectricalPhases-SinglePhase ;
    s223:hasVoltage s223:LineLineVoltage-380.0V,
        s223:LineNeutralVoltage-219.0V .

s223:AC-380.0VLL-219.0VLN-3Ph-60Hz a s223:Electricity-AC ;
    rdfs:label "AC-380.0VLL-219.0VLN-3Ph-60Hz" ;
    s223:hasFrequency s223:Frequency-60Hz ;
    s223:hasNumberOfElectricalPhases s223:NumberOfElectricalPhases-ThreePhase ;
    s223:hasVoltage s223:LineLineVoltage-380.0V,
        s223:LineNeutralVoltage-219.0V .

s223:AC-380.0VLL-3Ph-60Hz a s223:Electricity-AC ;
    rdfs:label "AC-380.0VLL-3Ph-60Hz" ;
    s223:hasFrequency s223:Frequency-60Hz ;
    s223:hasNumberOfElectricalPhases s223:NumberOfElectricalPhases-ThreePhase ;
    s223:hasVoltage s223:LineLineVoltage-380.0V .

s223:AC-4.16kVLL-1Ph-60Hz a s223:Electricity-AC ;
    rdfs:label "AC-4.16kVLL-1Ph-60Hz" ;
    s223:hasFrequency s223:Frequency-60Hz ;
    s223:hasNumberOfElectricalPhases s223:NumberOfElectricalPhases-SinglePhase ;
    s223:hasVoltage s223:LineLineVoltage-4.16kV .

s223:AC-4.16kVLL-2.4kVLN-1Ph-60Hz a s223:Electricity-AC ;
    rdfs:label "AC-4.16kVLL-2.4kVLN-1Ph-60Hz" ;
    s223:hasFrequency s223:Frequency-60Hz ;
    s223:hasNumberOfElectricalPhases s223:NumberOfElectricalPhases-SinglePhase ;
    s223:hasVoltage s223:LineLineVoltage-4.16kV,
        s223:LineNeutralVoltage-2.4kV .

s223:AC-4.16kVLL-2.4kVLN-3Ph-60Hz a s223:Electricity-AC ;
    rdfs:label "AC-4.16kVLL-2.4kVLN-3Ph-60Hz" ;
    s223:hasFrequency s223:Frequency-60Hz ;
    s223:hasNumberOfElectricalPhases s223:NumberOfElectricalPhases-ThreePhase ;
    s223:hasVoltage s223:LineLineVoltage-4.16kV,
        s223:LineNeutralVoltage-2.4kV .

s223:AC-4.16kVLL-3Ph-60Hz a s223:Electricity-AC ;
    rdfs:label "AC-4.16kVLL-3Ph-60Hz" ;
    s223:hasFrequency s223:Frequency-60Hz ;
    s223:hasNumberOfElectricalPhases s223:NumberOfElectricalPhases-ThreePhase ;
    s223:hasVoltage s223:LineLineVoltage-4.16kV .

s223:AC-400.0VLL-1Ph-50Hz a s223:Electricity-AC ;
    rdfs:label "AC-400.0VLL-1Ph-50Hz" ;
    s223:hasFrequency s223:Frequency-50Hz ;
    s223:hasNumberOfElectricalPhases s223:NumberOfElectricalPhases-SinglePhase ;
    s223:hasVoltage s223:LineLineVoltage-400.0V .

s223:AC-400.0VLL-231.0VLN-1Ph-50Hz a s223:Electricity-AC ;
    rdfs:label "AC-400.0VLL-231.0VLN-1Ph-50Hz" ;
    s223:hasFrequency s223:Frequency-50Hz ;
    s223:hasNumberOfElectricalPhases s223:NumberOfElectricalPhases-SinglePhase ;
    s223:hasVoltage s223:LineLineVoltage-400.0V,
        s223:LineNeutralVoltage-231.0V .

s223:AC-400.0VLL-231.0VLN-3Ph-50Hz a s223:Electricity-AC ;
    rdfs:label "AC-400.0VLL-231.0VLN-3Ph-50Hz" ;
    s223:hasFrequency s223:Frequency-50Hz ;
    s223:hasNumberOfElectricalPhases s223:NumberOfElectricalPhases-ThreePhase ;
    s223:hasVoltage s223:LineLineVoltage-400.0V,
        s223:LineNeutralVoltage-231.0V .

s223:AC-400.0VLL-3Ph-50Hz a s223:Electricity-AC ;
    rdfs:label "AC-400.0VLL-3Ph-50Hz" ;
    s223:hasFrequency s223:Frequency-50Hz ;
    s223:hasNumberOfElectricalPhases s223:NumberOfElectricalPhases-ThreePhase ;
    s223:hasVoltage s223:LineLineVoltage-400.0V .

s223:AC-415.0VLL-1Ph-50Hz a s223:Electricity-AC ;
    rdfs:label "AC-415.0VLL-1Ph-50Hz" ;
    s223:hasFrequency s223:Frequency-50Hz ;
    s223:hasNumberOfElectricalPhases s223:NumberOfElectricalPhases-SinglePhase ;
    s223:hasVoltage s223:LineLineVoltage-415.0V .

s223:AC-415.0VLL-240.0VLN-1Ph-50Hz a s223:Electricity-AC ;
    rdfs:label "AC-415.0VLL-240.0VLN-1Ph-50Hz" ;
    s223:hasFrequency s223:Frequency-50Hz ;
    s223:hasNumberOfElectricalPhases s223:NumberOfElectricalPhases-SinglePhase ;
    s223:hasVoltage s223:LineLineVoltage-415.0V,
        s223:LineNeutralVoltage-240.0V .

s223:AC-415.0VLL-240.0VLN-3Ph-50Hz a s223:Electricity-AC ;
    rdfs:label "AC-415.0VLL-240.0VLN-3Ph-50Hz" ;
    s223:hasFrequency s223:Frequency-50Hz ;
    s223:hasNumberOfElectricalPhases s223:NumberOfElectricalPhases-ThreePhase ;
    s223:hasVoltage s223:LineLineVoltage-415.0V,
        s223:LineNeutralVoltage-240.0V .

s223:AC-415.0VLL-3Ph-50Hz a s223:Electricity-AC ;
    rdfs:label "AC-415.0VLL-3Ph-50Hz" ;
    s223:hasFrequency s223:Frequency-50Hz ;
    s223:hasNumberOfElectricalPhases s223:NumberOfElectricalPhases-ThreePhase ;
    s223:hasVoltage s223:LineLineVoltage-415.0V .

s223:AC-480.0VLL-1Ph-60Hz a s223:Electricity-AC ;
    rdfs:label "AC-480.0VLL-1Ph-60Hz" ;
    s223:hasFrequency s223:Frequency-60Hz ;
    s223:hasNumberOfElectricalPhases s223:NumberOfElectricalPhases-SinglePhase ;
    s223:hasVoltage s223:LineLineVoltage-480.0V .

s223:AC-480.0VLL-277.0VLN-1Ph-60Hz a s223:Electricity-AC ;
    rdfs:label "AC-480.0VLL-277.0VLN-1Ph-60Hz" ;
    s223:hasFrequency s223:Frequency-60Hz ;
    s223:hasNumberOfElectricalPhases s223:NumberOfElectricalPhases-SinglePhase ;
    s223:hasVoltage s223:LineLineVoltage-480.0V,
        s223:LineNeutralVoltage-277.0V .

s223:AC-480.0VLL-277.0VLN-3Ph-60Hz a s223:Electricity-AC ;
    rdfs:label "AC-480.0VLL-277.0VLN-3Ph-60Hz" ;
    s223:hasFrequency s223:Frequency-60Hz ;
    s223:hasNumberOfElectricalPhases s223:NumberOfElectricalPhases-ThreePhase ;
    s223:hasVoltage s223:LineLineVoltage-480.0V,
        s223:LineNeutralVoltage-277.0V .

s223:AC-480.0VLL-3Ph-60Hz a s223:Electricity-AC ;
    rdfs:label "AC-480.0VLL-3Ph-60Hz" ;
    s223:hasFrequency s223:Frequency-60Hz ;
    s223:hasNumberOfElectricalPhases s223:NumberOfElectricalPhases-ThreePhase ;
    s223:hasVoltage s223:LineLineVoltage-480.0V .

s223:AC-5.77kVLN-1Ph-60Hz a s223:Electricity-AC ;
    rdfs:label "AC-5.77kVLN-1Ph-60Hz" ;
    s223:hasFrequency s223:Frequency-60Hz ;
    s223:hasNumberOfElectricalPhases s223:NumberOfElectricalPhases-SinglePhase ;
    s223:hasVoltage s223:LineNeutralVoltage-5.77kV .

s223:AC-6.0kVLL-1Ph-60Hz a s223:Electricity-AC ;
    rdfs:label "AC-6.0kVLL-1Ph-60Hz" ;
    s223:hasFrequency s223:Frequency-60Hz ;
    s223:hasNumberOfElectricalPhases s223:NumberOfElectricalPhases-SinglePhase ;
    s223:hasVoltage s223:LineLineVoltage-6.0kV .

s223:AC-6.0kVLL-3.46kVLN-1Ph-60Hz a s223:Electricity-AC ;
    rdfs:label "AC-6.0kVLL-3.46kVLN-1Ph-60Hz" ;
    s223:hasFrequency s223:Frequency-60Hz ;
    s223:hasNumberOfElectricalPhases s223:NumberOfElectricalPhases-SinglePhase ;
    s223:hasVoltage s223:LineLineVoltage-6.0kV,
        s223:LineNeutralVoltage-3.46kV .

s223:AC-6.0kVLL-3.46kVLN-3Ph-60Hz a s223:Electricity-AC ;
    rdfs:label "AC-6.0kVLL-3.46kVLN-3Ph-60Hz" ;
    s223:hasFrequency s223:Frequency-60Hz ;
    s223:hasNumberOfElectricalPhases s223:NumberOfElectricalPhases-ThreePhase ;
    s223:hasVoltage s223:LineLineVoltage-6.0kV,
        s223:LineNeutralVoltage-3.46kV .

s223:AC-6.0kVLL-3Ph-60Hz a s223:Electricity-AC ;
    rdfs:label "AC-6.0kVLL-3Ph-60Hz" ;
    s223:hasFrequency s223:Frequency-60Hz ;
    s223:hasNumberOfElectricalPhases s223:NumberOfElectricalPhases-ThreePhase ;
    s223:hasVoltage s223:LineLineVoltage-6.0kV .

s223:AC-6.6kVLL-1Ph-60Hz a s223:Electricity-AC ;
    rdfs:label "AC-6.6kVLL-1Ph-60Hz" ;
    s223:hasFrequency s223:Frequency-60Hz ;
    s223:hasNumberOfElectricalPhases s223:NumberOfElectricalPhases-SinglePhase ;
    s223:hasVoltage s223:LineLineVoltage-6.6kV .

s223:AC-6.6kVLL-3.81kVLN-1Ph-60Hz a s223:Electricity-AC ;
    rdfs:label "AC-6.6kVLL-3.81kVLN-1Ph-60Hz" ;
    s223:hasFrequency s223:Frequency-60Hz ;
    s223:hasNumberOfElectricalPhases s223:NumberOfElectricalPhases-SinglePhase ;
    s223:hasVoltage s223:LineLineVoltage-6.6kV,
        s223:LineNeutralVoltage-3.81kV .

s223:AC-6.6kVLL-3.81kVLN-3Ph-60Hz a s223:Electricity-AC ;
    rdfs:label "AC-6.6kVLL-3.81kVLN-3Ph-60Hz" ;
    s223:hasFrequency s223:Frequency-60Hz ;
    s223:hasNumberOfElectricalPhases s223:NumberOfElectricalPhases-ThreePhase ;
    s223:hasVoltage s223:LineLineVoltage-6.6kV,
        s223:LineNeutralVoltage-3.81kV .

s223:AC-6.6kVLL-3Ph-60Hz a s223:Electricity-AC ;
    rdfs:label "AC-6.6kVLL-3Ph-60Hz" ;
    s223:hasFrequency s223:Frequency-60Hz ;
    s223:hasNumberOfElectricalPhases s223:NumberOfElectricalPhases-ThreePhase ;
    s223:hasVoltage s223:LineLineVoltage-6.6kV .

s223:AC-600.0VLL-1Ph-60Hz a s223:Electricity-AC ;
    rdfs:label "AC-600.0VLL-1Ph-60Hz" ;
    s223:hasFrequency s223:Frequency-60Hz ;
    s223:hasNumberOfElectricalPhases s223:NumberOfElectricalPhases-SinglePhase ;
    s223:hasVoltage s223:LineLineVoltage-600.0V .

s223:AC-600.0VLL-347.0VLN-1Ph-60Hz a s223:Electricity-AC ;
    rdfs:label "AC-600.0VLL-347.0VLN-1Ph-60Hz" ;
    s223:hasFrequency s223:Frequency-60Hz ;
    s223:hasNumberOfElectricalPhases s223:NumberOfElectricalPhases-SinglePhase ;
    s223:hasVoltage s223:LineLineVoltage-600.0V,
        s223:LineNeutralVoltage-347.0V .

s223:AC-600.0VLL-347.0VLN-3Ph-60Hz a s223:Electricity-AC ;
    rdfs:label "AC-600.0VLL-347.0VLN-3Ph-60Hz" ;
    s223:hasFrequency s223:Frequency-60Hz ;
    s223:hasNumberOfElectricalPhases s223:NumberOfElectricalPhases-ThreePhase ;
    s223:hasVoltage s223:LineLineVoltage-600.0V,
        s223:LineNeutralVoltage-347.0V .

s223:AC-600.0VLL-3Ph-60Hz a s223:Electricity-AC ;
    rdfs:label "AC-600.0VLL-3Ph-60Hz" ;
    s223:hasFrequency s223:Frequency-60Hz ;
    s223:hasNumberOfElectricalPhases s223:NumberOfElectricalPhases-ThreePhase ;
    s223:hasVoltage s223:LineLineVoltage-600.0V .

s223:AirFilter a s223:Class,
        sh:NodeShape ;
    rdfs:label "Air filter" ;
    rdfs:comment "A device that removes particulates from gasses such as air." ;
    rdfs:subClassOf s223:Filter ;
    sh:property [ rdfs:comment "An AirFilter shall have at least one inlet using the medium Air." ;
            sh:path s223:hasConnectionPoint ;
            sh:qualifiedMinCount 1 ;
            sh:qualifiedValueShape [ sh:class s223:InletConnectionPoint ;
                    sh:node [ sh:property [ sh:class s223:Medium-Air ;
                                    sh:path s223:hasMedium ] ] ] ],
        [ rdfs:comment "An AirFilter shall have at least one outlet using the medium Air." ;
            sh:path s223:hasConnectionPoint ;
            sh:qualifiedMinCount 1 ;
            sh:qualifiedValueShape [ sh:class s223:OutletConnectionPoint ;
                    sh:node [ sh:property [ sh:class s223:Medium-Air ;
                                    sh:path s223:hasMedium ] ] ] ] .

s223:Attribute-CatalogNumber a s223:Context-Attribute ;
    rdfs:label "Attribute-CatalogNumber" ;
    rdfs:comment "The value of the associated Property identifies the catalog number." .

s223:Attribute-Face a s223:Context-Attribute ;
    rdfs:label "Attribute-Face" ;
    rdfs:comment "The value of the associated Property identifies a property related to a face, e.g. Coil Face Velocity." .

s223:Attribute-Manufacturer a s223:Context-Attribute ;
    rdfs:label "Attribute-Manufacturer" ;
    rdfs:comment "The value of the associated Property identifies the manufacturer." .

s223:Attribute-Model a s223:Context-Attribute ;
    rdfs:label "Attribute-Model" ;
    rdfs:comment "The value of the associated Property identifies the model." .

s223:Attribute-SerialNumber a s223:Context-Attribute ;
    rdfs:label "Attribute-SerialNumber" ;
    rdfs:comment "The value of the associated Property identifies the serial number." .

s223:Attribute-Year a s223:Context-Attribute ;
    rdfs:label "Attribute-Year" ;
    rdfs:comment "The value of the associated Property identifies the year of manufacture." .

s223:Battery a s223:Class,
        sh:NodeShape ;
    rdfs:label "Battery" ;
    rdfs:comment "A container consisting of one or more cells, in which chemical energy is converted into electricity and used as a source of power." ;
    rdfs:subClassOf s223:Equipment ;
    sh:or ( [ sh:property [ rdfs:comment "A Battery shall have at least one outlet or bidirectional ConnectionPoint using the medium Electricity." ;
                        sh:minCount 1 ;
                        sh:path s223:hasConnectionPoint ;
                        sh:qualifiedMinCount 1 ;
                        sh:qualifiedValueShape [ sh:class s223:OutletConnectionPoint ;
                                sh:node [ sh:property [ sh:class s223:Medium-Electricity ;
                                                sh:path s223:hasMedium ] ] ] ] ] [ sh:property [ rdfs:comment "A Battery shall have at least one outlet or bidirectional ConnectionPoint using the medium Electricity." ;
                        sh:minCount 1 ;
                        sh:path s223:hasConnectionPoint ;
                        sh:qualifiedMinCount 1 ;
                        sh:qualifiedValueShape [ sh:class s223:BidirectionalConnectionPoint ;
                                sh:node [ sh:property [ sh:class s223:Medium-Electricity ;
                                                sh:path s223:hasMedium ] ] ] ] ] ) .

s223:Binary-False a s223:EnumerationKind-Binary ;
    rdfs:label "Binary False" .

s223:Binary-True a s223:EnumerationKind-Binary ;
    rdfs:label "Binary True" .

s223:Binary-Unknown a s223:EnumerationKind-Binary ;
    rdfs:label "Binary Unknown" .

s223:Boiler a s223:Class,
        sh:NodeShape ;
    rdfs:label "Boiler" ;
    rdfs:comment "A closed, pressure vessel that uses fuel or electricity for heating water or other fluids to supply steam or hot water for heating, humidification, or other applications." ;
    rdfs:subClassOf s223:Equipment ;
    sh:property [ rdfs:comment "A Boiler shall have at least one inlet using the medium Water." ;
            sh:path s223:hasConnectionPoint ;
            sh:qualifiedMinCount 1 ;
            sh:qualifiedValueShape [ sh:class s223:InletConnectionPoint ;
                    sh:node [ sh:property [ sh:class s223:Medium-Water ;
                                    sh:path s223:hasMedium ] ] ] ],
        [ rdfs:comment "A Boiler shall have at least one outlet using the medium Water." ;
            sh:path s223:hasConnectionPoint ;
            sh:qualifiedMinCount 1 ;
            sh:qualifiedValueShape [ sh:class s223:OutletConnectionPoint ;
                    sh:node [ sh:property [ sh:class s223:Medium-Water ;
                                    sh:path s223:hasMedium ] ] ] ],
        [ sh:minCount 2 ;
            sh:path s223:hasConnectionPoint ] .

s223:ChilledBeam a s223:Class,
        sh:NodeShape ;
    rdfs:label "Chilled beam" ;
    rdfs:comment "A structure with a colder surface temperature where air passes through, and air movement is induced in the room to achieve cooling. Cooling medium is generally water." ;
    rdfs:subClassOf s223:Equipment ;
    sh:property [ rdfs:comment "A ChilledBeam shall have at least one inlet using the medium Water." ;
            sh:path s223:hasConnectionPoint ;
            sh:qualifiedMinCount 1 ;
            sh:qualifiedValueShape [ sh:class s223:InletConnectionPoint ;
                    sh:node [ sh:property [ sh:class s223:Medium-Water ;
                                    sh:path s223:hasMedium ] ] ] ],
        [ rdfs:comment "A ChilledBeam shall have at least one outlet using the medium Water." ;
            sh:path s223:hasConnectionPoint ;
            sh:qualifiedMinCount 1 ;
            sh:qualifiedValueShape [ sh:class s223:OutletConnectionPoint ;
                    sh:node [ sh:property [ sh:class s223:Medium-Water ;
                                    sh:path s223:hasMedium ] ] ] ],
        [ sh:minCount 2 ;
            sh:path s223:hasConnectionPoint ],
        [ rdfs:comment "A ChilledBeam must be associated with the Role-Cooling using the relation hasRole" ;
            sh:minCount 1 ;
            sh:path s223:hasRole ;
            sh:qualifiedMinCount 1 ;
            sh:qualifiedValueShape [ sh:class s223:Role-Cooling ] ] .

s223:Chiller a s223:Class,
        sh:NodeShape ;
    rdfs:label "Chiller" ;
    rdfs:comment "A refrigerating machine used to transfer heat from fluids." ;
    rdfs:subClassOf s223:Equipment ;
    sh:property [ rdfs:comment "A Chiller shall have at least one inlet using the medium Water." ;
            sh:path s223:hasConnectionPoint ;
            sh:qualifiedMinCount 1 ;
            sh:qualifiedValueShape [ sh:class s223:InletConnectionPoint ;
                    sh:node [ sh:property [ sh:class s223:Medium-Water ;
                                    sh:path s223:hasMedium ] ] ] ],
        [ rdfs:comment "A Chiller shall have at least one outlet using the medium Water." ;
            sh:path s223:hasConnectionPoint ;
            sh:qualifiedMinCount 1 ;
            sh:qualifiedValueShape [ sh:class s223:OutletConnectionPoint ;
                    sh:node [ sh:property [ sh:class s223:Medium-Water ;
                                    sh:path s223:hasMedium ] ] ] ],
        [ sh:minCount 2 ;
            sh:path s223:hasConnectionPoint ] .

s223:Compressor a s223:Class,
        sh:NodeShape ;
    rdfs:label "Compressor" ;
    rdfs:comment "A device for mechanically increasing the pressure of a gas." ;
    rdfs:subClassOf s223:Equipment ;
    sh:property [ rdfs:comment "A Compressor shall have at least one inlet." ;
            sh:path s223:hasConnectionPoint ;
            sh:qualifiedMinCount 1 ;
            sh:qualifiedValueShape [ sh:class s223:InletConnectionPoint ] ],
        [ rdfs:comment "A Compressor shall have at least one outlet." ;
            sh:path s223:hasConnectionPoint ;
            sh:qualifiedMinCount 1 ;
            sh:qualifiedValueShape [ sh:class s223:OutletConnectionPoint ] ],
        [ sh:minCount 2 ;
            sh:path s223:hasConnectionPoint ] .

s223:ConcentrationSensor a s223:Class,
        sh:NodeShape ;
    rdfs:label "Concentration sensor" ;
    rdfs:comment "A ConcentrationSensor is a specialization of a Sensor that observes a QuantifiableObservableProperty that represents the concentration of a substance in a medium." ;
    rdfs:subClassOf s223:Sensor .

s223:Controller a s223:Class,
        sh:NodeShape ;
    rdfs:label "Controller" ;
    rdfs:comment "A device for regulation of a system or component in normal operation, which exectues function blocks." ;
    rdfs:subClassOf s223:Equipment ;
    sh:property [ rdfs:comment "An instance of Controller can be associated with any number of Function block instances using the relation 'executes'." ;
            sh:class s223:FunctionBlock ;
            sh:path s223:executes ] .

s223:CoolingTower a s223:Class,
        sh:NodeShape ;
    rdfs:label "Cooling tower" ;
    rdfs:comment "A heat transfer device in which atmospheric air cools warm water, generally by direct contact via evaporation." ;
    rdfs:subClassOf s223:Equipment ;
    sh:property [ rdfs:comment "A CoolingTower shall have at least one inlet using the medium Water." ;
            sh:path s223:hasConnectionPoint ;
            sh:qualifiedMinCount 1 ;
            sh:qualifiedValueShape [ sh:class s223:InletConnectionPoint ;
                    sh:node [ sh:property [ sh:class s223:Medium-Water ;
                                    sh:path s223:hasMedium ] ] ] ],
        [ rdfs:comment "A CoolingTower shall have at least one outlet using the medium Water." ;
            sh:path s223:hasConnectionPoint ;
            sh:qualifiedMinCount 1 ;
            sh:qualifiedValueShape [ sh:class s223:OutletConnectionPoint ;
                    sh:node [ sh:property [ sh:class s223:Medium-Water ;
                                    sh:path s223:hasMedium ] ] ] ],
        [ sh:minCount 2 ;
            sh:path s223:hasConnectionPoint ] .

s223:CorrelatedColorTemperatureSensor a s223:Class,
        sh:NodeShape ;
    rdfs:label "Correlated color temperature sensor" ;
    rdfs:subClassOf s223:LightSensor ;
    sh:property [ rdfs:comment "A CorrelatedColorTemperatureSensor will always observe a Property that has a QuantityKind of ThermodynamicTemperature." ;
            sh:path s223:observes ;
            sh:qualifiedMinCount 1 ;
            sh:qualifiedValueShape [ sh:class s223:Property ;
                    sh:node [ sh:property [ sh:hasValue quantitykind:ThermodynamicTemperature ;
                                    sh:path qudt:hasQuantityKind ] ] ] ] .

s223:DC-12V a s223:Electricity-DC ;
    rdfs:label "DC 12V" ;
    s223:hasVoltage s223:Voltage-12V .

s223:DC-24V a s223:Electricity-DC ;
    rdfs:label "DC 24V" ;
    s223:hasVoltage s223:Voltage-24V .

s223:DC-380V a s223:Electricity-DC ;
    rdfs:label "DC 380V" ;
    s223:hasVoltage s223:Voltage-380V .

s223:DC-48V a s223:Electricity-DC ;
    rdfs:label "DC 48V" ;
    s223:hasVoltage s223:Voltage-48V .

s223:DC-5V a s223:Electricity-DC ;
    rdfs:label "DC 5V" ;
    s223:hasVoltage s223:Voltage-5V .

s223:DC-6V a s223:Electricity-DC ;
    rdfs:label "DC 6V" ;
    s223:hasVoltage s223:Voltage-6V .

s223:DifferentialSensor a s223:Class,
        sh:NodeShape ;
    rdfs:label "Differential sensor" ;
    rdfs:comment "A sensor that measures the difference of a quantity between any two points in the system." ;
    rdfs:subClassOf s223:AbstractSensor ;
    sh:property [ rdfs:comment "A Differential Sensor must be defined in terms of the QuantityKind that is being measured." ;
            sh:class qudt:QuantityKind ;
            sh:minCount 1 ;
            sh:path ( s223:observes qudt:hasQuantityKind ) ],
        [ rdfs:comment "Ensure that the values of hasObservationLocationHigh and hasObservationLocationLow are distinct." ;
            sh:path s223:hasObservationLocationHigh ;
            sh:sparql [ a sh:SPARQLConstraint ;
                    rdfs:comment "Ensure that the values of hasObservationLocationHigh and hasObservationLocationLow are distinct." ;
                    sh:message "{$this} cannot have the same value, {?high}, for both hasObservationLocationHigh and hasObservationLocationLow" ;
                    sh:prefixes s223: ;
                    sh:select """
SELECT $this ?high
WHERE {
  ?this s223:hasObservationLocationHigh ?high .
    ?this s223:hasObservationLocationLow ?low .
FILTER (?high = ?low) .
}
""" ] ] ;
    sh:xone ( [ sh:property [ rdfs:comment "A DifferentialSensor must be associated with exactly 1 of Connectable, Connection, Segment, or ConnectionPoint using the relation hasObservationLocationLow." ;
                        sh:class s223:Connectable ;
                        sh:path s223:hasObservationLocationLow ] ] [ sh:property [ rdfs:comment "A DifferentialSensor must be associated with exactly 1 of Connectable, Connection, Segment, or ConnectionPoint using the relation hasObservationLocationLow." ;
                        sh:class s223:Connection ;
                        sh:path s223:hasObservationLocationLow ] ] [ sh:property [ rdfs:comment "A DifferentialSensor must be associated with exactly 1 of Connectable, Connection, Segment, or ConnectionPoint using the relation hasObservationLocationLow." ;
                        sh:class s223:Segment ;
                        sh:path s223:hasObservationLocationLow ] ] [ sh:property [ rdfs:comment "A DifferentialSensor must be associated with exactly 1 of Connectable, Connection, Segment, or ConnectionPoint using the relation hasObservationLocationLow." ;
                        sh:class s223:ConnectionPoint ;
                        sh:path s223:hasObservationLocationLow ] ] ),
        ( [ sh:property [ rdfs:comment "A DifferentialSensor must be associated with exactly 1 of Connectable, Connection, Segment, or ConnectionPoint using the relation hasObservationLocationHigh." ;
                        sh:class s223:Connectable ;
                        sh:path s223:hasObservationLocationHigh ] ] [ sh:property [ rdfs:comment "A DifferentialSensor must be associated with exactly 1 of Connectable, Connection, Segment, or ConnectionPoint using the relation hasObservationLocationHigh." ;
                        sh:class s223:Connection ;
                        sh:path s223:hasObservationLocationHigh ] ] [ sh:property [ rdfs:comment "A DifferentialSensor must be associated with exactly 1 of Connectable, Connection, Segment, or ConnectionPoint using the relation hasObservationLocationHigh." ;
                        sh:class s223:Segment ;
                        sh:path s223:hasObservationLocationHigh ] ] [ sh:property [ rdfs:comment "A DifferentialSensor must be associated with exactly 1 of Connectable, Connection, Segment, or ConnectionPoint using the relation hasObservationLocationHigh." ;
                        sh:class s223:ConnectionPoint ;
                        sh:path s223:hasObservationLocationHigh ] ] ) .

s223:Dimensioned-ABLineLineVoltage a s223:Dimensioned-LineLineVoltage ;
    rdfs:label "Dimensioned-ABLineLineVoltage" ;
    rdfs:comment "The value of the associated Property identifies the A-B Line-to-line voltage of the medium" .

s223:Dimensioned-ANLineNeutralVoltage a s223:Dimensioned-LineNeutralVoltage ;
    rdfs:label "Dimensioned-ANLineNeutralVoltage" ;
    rdfs:comment "The value of the associated Property identifies the A-N Line-to-neutral voltage of the medium" .

s223:Dimensioned-BCLineLineVoltage a s223:Dimensioned-LineLineVoltage ;
    rdfs:label "Dimensioned-BCLineLineVoltage" ;
    rdfs:comment "The value of the associated Property identifies the B-C Line-to-line voltage of the medium" .

s223:Dimensioned-BNLineNeutralVoltage a s223:Dimensioned-LineNeutralVoltage ;
    rdfs:label "Dimensioned-BNLineNeutralVoltage" ;
    rdfs:comment "The value of the associated Property identifies the B-N Line-to-neutral voltage of the medium" .

s223:Dimensioned-CALineLineVoltage a s223:Dimensioned-LineLineVoltage ;
    rdfs:label "Dimensioned-CALineLineVoltage" ;
    rdfs:comment "The value of the associated Property identifies the C-A Line-to-line voltage of the medium" .

s223:Dimensioned-CNLineNeutralVoltage a s223:Dimensioned-LineNeutralVoltage ;
    rdfs:label "Dimensioned-CNLineNeutralVoltage" ;
    rdfs:comment "The value of the associated Property identifies the C-N Line-to-neutral voltage of the medium" .

s223:Dimensioned-Delta a s223:Context-Dimensioned ;
    rdfs:label "Dimensioned-Delta" ;
    rdfs:comment "Used to signify the associated Property has a delta (difference) value." .

s223:Dimensioned-DryBulb a s223:Context-Dimensioned ;
    rdfs:label "Dimensioned-DryBulb" ;
    rdfs:comment "The associated Property is a DryBulb temperature." .

s223:Dimensioned-Latent a s223:Context-Dimensioned ;
    rdfs:label "Dimensioned-Latent" ;
    rdfs:comment "The latent value of something characterized by this Property." .

s223:Dimensioned-Loss a s223:Context-Dimensioned ;
    rdfs:label "Dimensioned-Loss" ;
    rdfs:comment "The magnitude of loss of something characterized by this Property." .

s223:Dimensioned-Maximum a s223:Context-Dimensioned ;
    rdfs:label "Dimensioned-Maximum" ;
    rdfs:comment "The maximum allowable level of something characterized by this Property." .

s223:Dimensioned-Minimum a s223:Context-Dimensioned ;
    rdfs:label "Dimensioned-Minimum" ;
    rdfs:comment "The minimum allowable level of something characterized by this Property." .

s223:Dimensioned-Nominal a s223:Context-Dimensioned ;
    rdfs:label "Dimensioned-Nominal" ;
    rdfs:comment "The nominal level of something characterized by this Property." .

s223:Dimensioned-NominalFrequency a s223:Context-Dimensioned ;
    rdfs:label "Dimensioned-Nominal Frequency" ;
    rdfs:comment "The value of the associated Property identifies the nominal frequency of the medium" .

s223:Dimensioned-Rated a s223:Context-Dimensioned ;
    rdfs:label "Dimensioned-Rated" ;
    rdfs:comment "The rated value of something characterized by this Property." .

s223:Dimensioned-Sensible a s223:Context-Dimensioned ;
    rdfs:label "Dimensioned-Sensible" ;
    rdfs:comment "The sensible value of something characterized by this Property." .

s223:Dimensioned-StandardConditions a s223:Context-Dimensioned ;
    rdfs:label "Dimensioned-StandardConditions" ;
    rdfs:comment "Indicates the Property applies under standard conditions (such as standard temperature and pressure)." .

s223:Dimensioned-Standby a s223:Context-Dimensioned ;
    rdfs:label "Dimensioned-Standby" ;
    rdfs:comment "The standby value of something characterized by this Property." .

s223:Dimensioned-Startup a s223:Context-Dimensioned ;
    rdfs:label "Dimensioned-Startup" ;
    rdfs:comment "The startup value of something characterized by this Property." .

s223:Dimensioned-Threshold a s223:Context-Dimensioned ;
    rdfs:label "Dimensioned-Threshold" ;
    rdfs:comment "The threshold value of something characterized by this Property." .

s223:Dimensioned-Total a s223:Context-Dimensioned ;
    rdfs:label "Dimensioned-Total" ;
    rdfs:comment "The total amount of something characterized by this Property." .

s223:Dimensioned-Weight a s223:Context-Dimensioned ;
    rdfs:label "Dimensioned-Weight" ;
    rdfs:comment "The weight of something characterized by this Property." .

s223:Dimensioned-WetBulb a s223:Context-Dimensioned ;
    rdfs:label "Dimensioned-WetBulb" ;
    rdfs:comment "The associated Property is a WetBulb temperature." .

s223:Dimensionless-Efficiency a s223:Context-Dimensionless ;
    rdfs:label "Dimensionless-Efficiency" ;
    rdfs:comment "The efficiency of something characterized by a dimensionless value of this Property." .

s223:Dimensionless-PhaseAngle a s223:Context-Dimensionless ;
    rdfs:label "Dimensionless-Phase angle" .

s223:Dimensionless-PowerFactor a s223:Context-Dimensionless ;
    rdfs:label "Dimensionless-PowerFactor" ;
    rdfs:comment "The power factor of something characterized by a dimensionless value of this Property." .

s223:Dimensionless-ServiceFactor a s223:Context-Dimensionless ;
    rdfs:label "Dimensionless-ServiceFactor" ;
    rdfs:comment "The service factor of something characterized by a dimensionless value of this Property." .

s223:Direction-Bidirectional a s223:EnumerationKind-Direction ;
    rdfs:label "Direction-Bidirectional" ;
    rdfs:comment "One of the  set of enumeration values for the hasDirection property used to characterize the direction of flow associated with an instance of a ConnectionPoint. The value Bidirectional indicates that the flow direction is not fixed in one direction. It depends on the status of some other part of the system, such as a valve position, that is expected to change during operation." .

s223:Direction-Inlet a s223:EnumerationKind-Direction ;
    rdfs:label "Direction-Inlet"@en ;
    rdfs:comment "One of the set of enumeration values for the hasDirection property used to characterize the direction of flow associated with an instance of a ConnectionPoint. The value Inlet indicates that the direction of flow is into the Equipment." .

s223:Direction-Outlet a s223:EnumerationKind-Direction ;
    rdfs:label "Direction-Outlet"@en,
        "Direction-Sortie"@fr ;
    rdfs:comment "One member of the enumerated valid values to characterize the hasDirection property. It is an instance of the Direction class." .

s223:Domain-ConveyanceSystems a s223:EnumerationKind-Domain ;
    rdfs:label "Domain-ConveyanceSystems" ;
    rdfs:comment "The domain ConveyanceSystems represents equipment used to move people or things from one place in a building to another. Example equipment that might fall within a ConveyanceSystems domain include elevators, escalators, and conveyer belts." .

s223:Domain-Electrical a s223:EnumerationKind-Domain ;
    rdfs:label "Domain-Electrical" ;
    rdfs:comment "The domain Electrical represents equipment used to provide electrical power within a building. Example equipment that might fall within an Electrical domain include breaker panels, switchgear, photovoltaic panels, and generators. " .

s223:Domain-Fire a s223:EnumerationKind-Domain ;
    rdfs:label "Domain-Fire" ;
    rdfs:comment "The domain Fire represents equipment used to provide fire detection and protection within a building. Example equipment that might be fall within a Fire domain include smoke detectors, alarm annunciators, and emergency public address systems. " .

s223:Domain-Networking a s223:EnumerationKind-Domain ;
    rdfs:label "Domain-Networking" ;
    rdfs:comment "The domain Networking represents equipment used to provide information technology communication for a building." .

s223:Domain-PhysicalSecurity a s223:EnumerationKind-Domain ;
    rdfs:label "Domain-PhysicalSecurity" ;
    rdfs:comment "The domain Security represents equipment that provides physical access control within or outside a building. Example equipment that might fall within a PhysicalSecurity domain include cameras, keycard sensors, and biometric scanners." .

s223:Domain-Plumbing a s223:EnumerationKind-Domain ;
    rdfs:label "Domain-Plumbing" ;
    rdfs:comment "The domain Plumbing represents equipment used to provide domestic water within or outside a building. Example equipment that might fall within a Plumbing domain includes water meters, domestic hot water tanks, and sinks." .

s223:Domain-Refrigeration a s223:EnumerationKind-Domain ;
    rdfs:label "Domain-Refrigeration" ;
    rdfs:comment "The domain Refrigeration represents equipment used to provide cooling for a purpose other than space conditioning in a building." .

s223:Door a s223:Class,
        sh:NodeShape ;
    rdfs:label "Door" ;
    rdfs:comment "A hinged, sliding, or revolving barrier at the entrance to a building or room." ;
    rdfs:subClassOf s223:Equipment ;
    sh:property [ rdfs:comment "A Door shall have at least one inlet using the medium Air." ;
            sh:path s223:hasConnectionPoint ;
            sh:qualifiedMinCount 1 ;
            sh:qualifiedValueShape [ sh:class s223:InletConnectionPoint ;
                    sh:node [ sh:property [ sh:class s223:Medium-Air ;
                                    sh:path s223:hasMedium ] ] ] ],
        [ rdfs:comment "A Door shall have at least one outlet using the medium Air." ;
            sh:path s223:hasConnectionPoint ;
            sh:qualifiedMinCount 1 ;
            sh:qualifiedValueShape [ sh:class s223:OutletConnectionPoint ;
                    sh:node [ sh:property [ sh:class s223:Medium-Air ;
                                    sh:path s223:hasMedium ] ] ] ],
        [ sh:minCount 2 ;
            sh:path s223:hasConnectionPoint ] .

s223:DualDuctTerminal a s223:Class,
        sh:NodeShape ;
    rdfs:label "Dual duct air terminal." ;
    rdfs:comment "A dual duct air terminal mixes two independent sources of primary air." ;
    rdfs:seeAlso s223:TerminalUnit ;
    rdfs:subClassOf s223:TerminalUnit ;
    sh:property [ rdfs:comment "A DualDuctTerminal shall have at least two inlets using the medium Air." ;
            sh:path s223:hasConnectionPoint ;
            sh:qualifiedMinCount 2 ;
            sh:qualifiedValueShape [ sh:class s223:InletConnectionPoint ;
                    sh:node [ sh:property [ sh:class s223:Medium-Air ;
                                    sh:path s223:hasMedium ] ] ] ] .

s223:Duct a s223:Class,
        sh:NodeShape ;
    rdfs:label "Duct" ;
    rdfs:comment "A Duct is a subclass of Connection, that represents a conduit through which air is conveyed." ;
    rdfs:subClassOf s223:Connection .

s223:DuvSensor a s223:Class,
        sh:NodeShape ;
    rdfs:label "Duv sensor" ;
    rdfs:subClassOf s223:LightSensor ;
    sh:property [ rdfs:comment "A DuvSensor will always observe a Property that has a QuantityKind of Duv." ;
            sh:path s223:observes ;
            sh:qualifiedMinCount 1 ;
            sh:qualifiedValueShape [ sh:class s223:Property ;
                    sh:node [ sh:property [ sh:hasValue quantitykind:Duv ;
                                    sh:path qudt:hasQuantityKind ] ] ] ] .

s223:EM-Microwave a s223:Medium-EM ;
    rdfs:label "EM-Microwave" .

s223:EM-RF a s223:Medium-EM ;
    rdfs:label "EM-RF" .

s223:Effectiveness-Active a s223:Attribute-Effectiveness ;
    rdfs:label "Active" .

s223:ElectricMeter a s223:Class,
        sh:NodeShape ;
    rdfs:label "Electric meter" ;
    rdfs:comment "A device that measures the properties of electric energy." ;
    rdfs:subClassOf s223:Equipment .

s223:ElectricOutlet a s223:Class,
        sh:NodeShape ;
    rdfs:label "Electric outlet" ;
    rdfs:comment "A device to which a piece of electrical equipment can be connected in order to provide it with electricity" ;
    rdfs:subClassOf s223:Equipment ;
    sh:property [ rdfs:comment "An ElectricOutlet shall have exactly one inlet using the medium Electricity." ;
            sh:path s223:hasConnectionPoint ;
            sh:qualifiedMaxCount 1 ;
            sh:qualifiedMinCount 1 ;
            sh:qualifiedValueShape [ sh:class s223:InletConnectionPoint ;
                    sh:node [ sh:property [ sh:class s223:Medium-Electricity ;
                                    sh:path s223:hasMedium ] ] ] ],
        [ rdfs:comment "An ElectricOutlet shall have at least one outlet using the medium Electricity." ;
            sh:path s223:hasConnectionPoint ;
            sh:qualifiedMinCount 1 ;
            sh:qualifiedValueShape [ sh:class s223:OutletConnectionPoint ;
                    sh:node [ sh:property [ sh:class s223:Medium-Electricity ;
                                    sh:path s223:hasMedium ] ] ] ],
        [ sh:minCount 2 ;
            sh:path s223:hasConnectionPoint ] .

s223:ElectricTransformer a s223:Class,
        sh:NodeShape ;
    rdfs:label "Electric transformer" ;
    rdfs:comment "A piece of electrical equipment used to convert alternative current (AC) electric power from one voltage to another voltage." ;
    rdfs:subClassOf s223:Equipment ;
    sh:property [ rdfs:comment "An ElectricTransformer shall have at least one inlet using the medium Electricity." ;
            sh:path s223:hasConnectionPoint ;
            sh:qualifiedMinCount 1 ;
            sh:qualifiedValueShape [ sh:class s223:InletConnectionPoint ;
                    sh:node [ sh:property [ sh:class s223:Medium-Electricity ;
                                    sh:path s223:hasMedium ] ] ] ],
        [ rdfs:comment "An ElectricTransformer shall have at least one outlet using the medium Electricity." ;
            sh:path s223:hasConnectionPoint ;
            sh:qualifiedMinCount 1 ;
            sh:qualifiedValueShape [ sh:class s223:OutletConnectionPoint ;
                    sh:node [ sh:property [ sh:class s223:Medium-Electricity ;
                                    sh:path s223:hasMedium ] ] ] ],
        [ sh:minCount 2 ;
            sh:path s223:hasConnectionPoint ] .

s223:ElectricalPhaseIdentifier-AB a s223:Attribute-ElectricalPhaseIdentifier ;
    rdfs:label "Electrical Phase Identifier AB" ;
    rdfs:comment "The value of the associated Property identifies the electrical phase AB of the Connection." .

s223:ElectricalPhaseIdentifier-ABC a s223:Attribute-ElectricalPhaseIdentifier ;
    rdfs:label "Electrical Phase Identifier ABC" ;
    rdfs:comment "The value of the associated Property identifies the electrical phase ABC of the Connection." .

s223:ElectricalPhaseIdentifier-C a s223:Attribute-ElectricalPhaseIdentifier ;
    rdfs:label "Electrical Phase Identifier C" ;
    rdfs:comment "The value of the associated Property identifies the electrical phase C of the Connection." .

s223:ElectricalPhaseIdentifier-CA a s223:Attribute-ElectricalPhaseIdentifier ;
    rdfs:label "Electrical Phase Identifier CA" ;
    rdfs:comment "The value of the associated Property identifies the electrical phase CA of the Connection." .

s223:Electricity-Earth a s223:Medium-Electricity ;
    rdfs:label "Electricity-Earth" .

s223:Electricity-Neutral a s223:Medium-Electricity ;
    rdfs:label "Electricity-Neutral" .

s223:EthernetSwitch a s223:Class,
        sh:NodeShape ;
    rdfs:label "Ethernet switch" ;
    rdfs:comment "A device that connects wired devices such as computers, laptops, routers, servers, and printers to one another." ;
    rdfs:subClassOf s223:Equipment ;
    sh:property [ rdfs:comment "An EthernetSwitch shall have at least one BidirectionalConnectionPoint using the medium Electricity." ;
            sh:path s223:hasConnectionPoint ;
            sh:qualifiedMinCount 1 ;
            sh:qualifiedValueShape [ sh:class s223:BidirectionalConnectionPoint ;
                    sh:node [ sh:property [ sh:class s223:Medium-Electricity ;
                                    sh:path s223:hasMedium ] ] ] ] .

s223:ExternalSource a s223:Class,
        sh:NodeShape ;
    rdfs:label "External source" ;
    rdfs:subClassOf s223:Concept .

s223:FanCoilUnit a s223:Class,
        sh:NodeShape ;
    rdfs:label "Fan coil unit" ;
    rdfs:comment "A device consisting of a heat exchanger (coil) and a fan to regulate the temperature of one or more spaces." ;
    rdfs:subClassOf s223:Equipment ;
    sh:property [ rdfs:comment "A FanCoilUnit must be associated with at least 1 Coil using the relation contains." ;
            sh:path s223:contains ;
            sh:qualifiedMinCount 1 ;
            sh:qualifiedValueShape [ sh:class s223:Coil ] ],
        [ rdfs:comment "A FanCoilUnit must be associated with at least 1 Fan using the relation contains." ;
            sh:path s223:contains ;
            sh:qualifiedMinCount 1 ;
            sh:qualifiedValueShape [ sh:class s223:Fan ] ],
        [ sh:minCount 2 ;
            sh:path s223:contains ],
        [ rdfs:comment "A FanCoilUnit shall have at least one inlet using the medium Air." ;
            sh:path s223:hasConnectionPoint ;
            sh:qualifiedMinCount 1 ;
            sh:qualifiedValueShape [ sh:class s223:InletConnectionPoint ;
                    sh:node [ sh:property [ sh:class s223:Medium-Air ;
                                    sh:path s223:hasMedium ] ] ] ],
        [ rdfs:comment "A FanCoilUnit shall have at least one outlet using the medium Air." ;
            sh:path s223:hasConnectionPoint ;
            sh:qualifiedMinCount 1 ;
            sh:qualifiedValueShape [ sh:class s223:OutletConnectionPoint ;
                    sh:node [ sh:property [ sh:class s223:Medium-Air ;
                                    sh:path s223:hasMedium ] ] ] ],
        [ sh:minCount 2 ;
            sh:path s223:hasConnectionPoint ],
        [ rdfs:comment "A FanCoilUnit must at least have the role Role-Heating or Role-Cooling." ;
            sh:minCount 1 ;
            sh:path s223:hasRole ;
            sh:qualifiedMinCount 1 ;
            sh:qualifiedValueShape [ sh:in ( s223:Role-Heating s223:Role-Cooling ) ] ] .

s223:FanPoweredTerminal a s223:Class,
        sh:NodeShape ;
    rdfs:label "Fan Powered Air Terminal" ;
    rdfs:comment "An air terminal containing a fan. Airflow may pass through or be parallel to the fan. These units may also have supplemental heating or cooling." ;
    rdfs:subClassOf s223:TerminalUnit ;
    sh:property [ rdfs:comment "A FanPoweredTerminal must be associated with at least 1 Fan by contains" ;
            sh:minCount 1 ;
            sh:path s223:contains ;
            sh:qualifiedMinCount 1 ;
            sh:qualifiedValueShape [ sh:class s223:Fan ] ] .

s223:FumeHood a s223:Class,
        sh:NodeShape ;
    rdfs:label "Fume hood" ;
    rdfs:comment "A fume-collection device mounted over a work space, table, or shelf and serving to conduct unwanted gases away from an area." ;
    rdfs:subClassOf s223:Equipment ;
    sh:property [ rdfs:comment "A FumeHood shall have at least one inlet using the medium Air." ;
            sh:path s223:hasConnectionPoint ;
            sh:qualifiedMinCount 1 ;
            sh:qualifiedValueShape [ sh:class s223:InletConnectionPoint ;
                    sh:node [ sh:property [ sh:class s223:Medium-Air ;
                                    sh:path s223:hasMedium ] ] ] ],
        [ rdfs:comment "A FumeHood shall have at least one outlet using the medium Air." ;
            sh:path s223:hasConnectionPoint ;
            sh:qualifiedMinCount 1 ;
            sh:qualifiedValueShape [ sh:class s223:OutletConnectionPoint ;
                    sh:node [ sh:property [ sh:class s223:Medium-Air ;
                                    sh:path s223:hasMedium ] ] ] ],
        [ sh:minCount 2 ;
            sh:path s223:hasConnectionPoint ] .

s223:Furnace a s223:Class,
        sh:NodeShape ;
    rdfs:label "Furnace" ;
    rdfs:comment "An enclosed chamber or structure in which heat is produced, as by burning fuel or by converting electrical energy. " ;
    rdfs:subClassOf s223:Equipment ;
    sh:property [ rdfs:comment "A Furnace shall have at least one outlet using the medium Air." ;
            sh:path s223:hasConnectionPoint ;
            sh:qualifiedMinCount 1 ;
            sh:qualifiedValueShape [ sh:class s223:OutletConnectionPoint ;
                    sh:node [ sh:property [ sh:class s223:Medium-Air ;
                                    sh:path s223:hasMedium ] ] ] ],
        [ sh:minCount 2 ;
            sh:path s223:hasConnectionPoint ],
        [ rdfs:comment "A Furnace shall have at least one inlet using the medium Air." ;
            sh:path s223:hasConnectionPoint ;
            sh:qualifiedMinCount 1 ;
            sh:qualifiedValueShape [ sh:class s223:InletConnectionPoint ;
                    sh:node [ sh:property [ sh:class s223:Medium-Air ;
                                    sh:path s223:hasMedium ] ] ] ] .

s223:Gas-SuperHeated a s223:Phase-Gas ;
    rdfs:label "Gas-Super heated" .

s223:Generator a s223:Class,
        sh:NodeShape ;
    rdfs:label "Generator" ;
    rdfs:comment "An energy transducer that transforms non-electric energy into electric energy." ;
    rdfs:subClassOf s223:Equipment ;
    sh:property [ rdfs:comment "A Generator shall have at least one outlet using the medium Electricity." ;
            sh:class s223:OutletConnectionPoint ;
            sh:minCount 1 ;
            sh:node [ sh:property [ sh:class s223:Medium-Electricity ;
                            sh:path s223:hasMedium ] ] ;
            sh:path s223:hasConnectionPoint ],
        [ sh:minCount 1 ;
            sh:path s223:hasConnectionPoint ] .

s223:GlycolSolution-15Percent a s223:Water-GlycolSolution ;
    rdfs:label "GlycolSolution-15Percent" ;
    s223:hasProperty [ a s223:QuantifiableProperty ;
            rdfs:label "Glycol conc" ;
            s223:hasAspect s223:Medium-Glycol ;
            s223:hasValue 15.0 ;
            qudt:hasQuantityKind quantitykind:VolumeFraction ;
            qudt:hasUnit unit:PERCENT ],
        [ a s223:QuantifiableProperty ;
            rdfs:label "Water conc" ;
            s223:hasAspect s223:Medium-Water ;
            s223:hasValue 85.0 ;
            qudt:hasQuantityKind quantitykind:VolumeFraction ;
            qudt:hasUnit unit:PERCENT ] .

s223:GlycolSolution-30Percent a s223:Water-GlycolSolution ;
    rdfs:label "GlycolSolution-30Percent" ;
    s223:hasProperty [ a s223:QuantifiableProperty ;
            rdfs:label "Glycol conc" ;
            s223:hasAspect s223:Medium-Glycol ;
            s223:hasValue 30.0 ;
            qudt:hasQuantityKind quantitykind:VolumeFraction ;
            qudt:hasUnit unit:PERCENT ],
        [ a s223:QuantifiableProperty ;
            rdfs:label "Water conc" ;
            s223:hasAspect s223:Medium-Water ;
            s223:hasValue 70.0 ;
            qudt:hasQuantityKind quantitykind:VolumeFraction ;
            qudt:hasUnit unit:PERCENT ] .

s223:HVACOperatingMode-Auto a s223:EnumerationKind-HVACOperatingMode ;
    rdfs:label "Auto" .

s223:HVACOperatingMode-CoolOnly a s223:EnumerationKind-HVACOperatingMode ;
    rdfs:label "CoolOnly" .

s223:HVACOperatingMode-FanOnly a s223:EnumerationKind-HVACOperatingMode ;
    rdfs:label "FanOnly" .

s223:HVACOperatingMode-HeatOnly a s223:EnumerationKind-HVACOperatingMode ;
    rdfs:label "HeatOnly" .

s223:HVACOperatingMode-Off a s223:EnumerationKind-HVACOperatingMode ;
    rdfs:label "Off" .

s223:HVACOperatingStatus-Cooling a s223:EnumerationKind-HVACOperatingStatus ;
    rdfs:label "Cooling" .

s223:HVACOperatingStatus-Dehumidifying a s223:EnumerationKind-HVACOperatingStatus ;
    rdfs:label "Dehumidifying" .

s223:HVACOperatingStatus-Heating a s223:EnumerationKind-HVACOperatingStatus ;
    rdfs:label "Heating" .

s223:HVACOperatingStatus-Off a s223:EnumerationKind-HVACOperatingStatus ;
    rdfs:label "Off" .

s223:HVACOperatingStatus-Ventilating a s223:EnumerationKind-HVACOperatingStatus ;
    rdfs:label "Ventilating" .

s223:HasDomainLookingUpRule a sh:NodeShape ;
    sh:rule [ a sh:TripleRule ;
            rdfs:comment "Traverse up the contains hierarchy to determine the domain" ;
            sh:object [ sh:path ( [ sh:zeroOrMorePath [ sh:inversePath s223:contains ] ] s223:hasDomain ) ] ;
            sh:predicate s223:hasDomain ;
            sh:subject sh:this ] ;
    sh:targetClass s223:DomainSpace,
        s223:Zone .

s223:HeatPump a s223:Class,
        sh:NodeShape ;
    rdfs:label "HeatPump" ;
    rdfs:comment "A device that can heat or cool by transferring thermal energy using a reversible refrigeration cycle." ;
    rdfs:subClassOf s223:Equipment ;
    sh:property [ rdfs:comment "A HeatPump shall have at least one inlet using the medium Air." ;
            sh:path s223:hasConnectionPoint ;
            sh:qualifiedMinCount 1 ;
            sh:qualifiedValueShape [ sh:class s223:InletConnectionPoint ;
                    sh:node [ sh:property [ sh:class s223:Medium-Air ;
                                    sh:path s223:hasMedium ] ] ] ],
        [ rdfs:comment "A HeatPump shall have at least one outlet using the medium Air." ;
            sh:path s223:hasConnectionPoint ;
            sh:qualifiedMinCount 1 ;
            sh:qualifiedValueShape [ sh:class s223:OutletConnectionPoint ;
                    sh:node [ sh:property [ sh:class s223:Medium-Air ;
                                    sh:path s223:hasMedium ] ] ] ],
        [ sh:minCount 2 ;
            sh:path s223:hasConnectionPoint ] .

s223:Humidifier a s223:Class,
        sh:NodeShape ;
    rdfs:label "Humidifier" ;
    rdfs:comment "A device to add moisture to gases such as air." ;
    rdfs:subClassOf s223:Equipment .

s223:Humidistat a s223:Class,
        sh:NodeShape ;
    rdfs:label "Humidistat" ;
    rdfs:comment "An automatic control device used to maintain humidity at a fixed or adjustable setpoint." ;
    rdfs:subClassOf s223:Equipment .

s223:HumiditySensor a s223:Class,
        sh:NodeShape ;
    rdfs:label "Humidity sensor" ;
    rdfs:comment "A HumiditySensor is a specialization of a Sensor that observes a QuantifiableObservableProperty that represents a humidity measurement. " ;
    rdfs:subClassOf s223:Sensor ;
    sh:rule [ a sh:SPARQLRule ;
            rdfs:comment "A HumiditySensor will always observe a Property that has a QuantityKind of RelativeHumidity." ;
            sh:construct """
CONSTRUCT {?prop qudt:hasQuantityKind qudtqk:RelativeHumidity .}
WHERE {
  $this s223:observes ?prop .
}
""" ;
            sh:prefixes s223: ] .

s223:InversePropertyShape a sh:NodeShape ;
    sh:rule [ a sh:SPARQLRule ;
            rdfs:comment "Declare the inverse triples for relations that have defined inverse relations" ;
            sh:construct """
CONSTRUCT {
?o ?invP $this .
}
WHERE {
  $this ?p ?o .
  ?p s223:inverseOf ?invP .
}
			""" ;
            sh:prefixes s223: ] ;
    sh:targetClass s223:Concept .

s223:Inverter a s223:Class,
        sh:NodeShape ;
    rdfs:label "Inverter" ;
    rdfs:comment "An electric energy converter that changes direct electric current to alternating current." ;
    rdfs:subClassOf s223:Equipment ;
    sh:property [ rdfs:comment "An Inverter shall have at least one inlet using the medium Electricity-DC." ;
            sh:path s223:hasConnectionPoint ;
            sh:qualifiedMinCount 1 ;
            sh:qualifiedValueShape [ sh:class s223:InletConnectionPoint ;
                    sh:node [ sh:property [ sh:class s223:Electricity-DC ;
                                    sh:path s223:hasMedium ] ] ] ],
        [ rdfs:comment "An Inverter shall have at least one outlet using the medium Electricity-AC." ;
            sh:path s223:hasConnectionPoint ;
            sh:qualifiedMinCount 1 ;
            sh:qualifiedValueShape [ sh:class s223:OutletConnectionPoint ;
                    sh:node [ sh:property [ sh:class s223:Electricity-AC ;
                                    sh:path s223:hasMedium ] ] ] ],
        [ sh:minCount 2 ;
            sh:path s223:hasConnectionPoint ] .

s223:Light-Infrared a s223:EM-Light ;
    rdfs:label "Light-Infrared" .

s223:Light-Ultraviolet a s223:EM-Light ;
    rdfs:label "Light-Ultraviolet" .

s223:LineLineVoltage-190V a s223:Dimensioned-LineLineVoltage ;
    rdfs:label "190V Line-Line Voltage" .

s223:LineLineVoltage-208V a s223:Dimensioned-LineLineVoltage ;
    rdfs:label "208V Line-Line Voltage" .

s223:LineLineVoltage-220V a s223:Dimensioned-LineLineVoltage ;
    rdfs:label "220V Line-Line Voltage" .

s223:LineLineVoltage-240V a s223:Dimensioned-LineLineVoltage ;
    rdfs:label "240V Line-Line Voltage" .

s223:LineLineVoltage-380V a s223:Dimensioned-LineLineVoltage ;
    rdfs:label "380V Line-Line Voltage" .

s223:LineLineVoltage-400V a s223:Dimensioned-LineLineVoltage ;
    rdfs:label "400V Line-Line Voltage" .

s223:LineLineVoltage-415V a s223:Dimensioned-LineLineVoltage ;
    rdfs:label "415V Line-Line Voltage" .

s223:LineLineVoltage-480V a s223:Dimensioned-LineLineVoltage ;
    rdfs:label "480V Line-Line Voltage" .

s223:LineLineVoltage-600V a s223:Dimensioned-LineLineVoltage ;
    rdfs:label "600V Line-Line Voltage" .

s223:LineNeutralVoltage-10.0kV a s223:Dimensioned-LineNeutralVoltage ;
    rdfs:label "10.0kV Line-Neutral Voltage" .

s223:LineNeutralVoltage-120V a s223:Dimensioned-LineNeutralVoltage ;
    rdfs:label "120V Line-Neutral Voltage" .

s223:LineNeutralVoltage-190V a s223:Dimensioned-LineNeutralVoltage ;
    rdfs:label "190V Line-Neutral Voltage" .

s223:LineNeutralVoltage-208V a s223:Dimensioned-LineNeutralVoltage ;
    rdfs:label "208V Line-Neutral Voltage" .

s223:LineNeutralVoltage-220V a s223:Dimensioned-LineNeutralVoltage ;
    rdfs:label "220V Line-Neutral Voltage" .

s223:LineNeutralVoltage-240V a s223:Dimensioned-LineNeutralVoltage ;
    rdfs:label "240V Line-Neutral Voltage" .

s223:LineNeutralVoltage-3.0kV a s223:Dimensioned-LineNeutralVoltage ;
    rdfs:label "3.0kV Line-Neutral Voltage" .

s223:LineNeutralVoltage-3.3kV a s223:Dimensioned-LineNeutralVoltage ;
    rdfs:label "3.3kV Line-Neutral Voltage" .

s223:LineNeutralVoltage-380V a s223:Dimensioned-LineNeutralVoltage ;
    rdfs:label "380V Line-Neutral Voltage" .

s223:LineNeutralVoltage-4.16kV a s223:Dimensioned-LineNeutralVoltage ;
    rdfs:label "4.16kV Line-Neutral Voltage" .

s223:LineNeutralVoltage-400V a s223:Dimensioned-LineNeutralVoltage ;
    rdfs:label "400V Line-Neutral Voltage" .

s223:LineNeutralVoltage-415V a s223:Dimensioned-LineNeutralVoltage ;
    rdfs:label "415V Line-Neutral Voltage" .

s223:LineNeutralVoltage-480V a s223:Dimensioned-LineNeutralVoltage ;
    rdfs:label "480V Line-Neutral Voltage" .

s223:LineNeutralVoltage-6.0kV a s223:Dimensioned-LineNeutralVoltage ;
    rdfs:label "6.0kV Line-Neutral Voltage" .

s223:LineNeutralVoltage-6.6kV a s223:Dimensioned-LineNeutralVoltage ;
    rdfs:label "6.6kV Line-Neutral Voltage" .

s223:LineNeutralVoltage-600V a s223:Dimensioned-LineNeutralVoltage ;
    rdfs:label "600V Line-Neutral Voltage" .

s223:Liquid-SubCooled a s223:Phase-Liquid ;
    rdfs:label "Liquid-Sub cooled" .

s223:ManualDamper a s223:Class ;
    rdfs:label "Manual damper" ;
    rdfs:subClassOf s223:Damper .

s223:MeasuredPropertyRule a sh:NodeShape ;
    rdfs:comment "Associate the object of hasObservationLocation directly with the observed Property." ;
    sh:rule [ a sh:TripleRule ;
            rdfs:comment "Associate the object of hasObservationLocation directly with the observed Property." ;
            sh:object [ sh:path ( [ sh:inversePath s223:hasObservationLocation ] s223:observes ) ] ;
            sh:predicate s223:hasProperty ;
            sh:subject sh:this ] ;
    sh:targetClass s223:Concept .

s223:Modulated-0-10V a s223:Signal-Modulated ;
    rdfs:label "Modulated 0-10V" .

s223:Modulated-4-20mA a s223:Signal-Modulated ;
    rdfs:label "Modulated 4-20mA" .

s223:Motion-False a s223:Occupancy-Motion ;
    rdfs:label "Motion-False" .

s223:Motor a s223:Class,
        sh:NodeShape ;
    rdfs:label "Motor" ;
    rdfs:comment "A machine in which power is applied to do work by the conversion of various forms of energy into mechanical force and motion." ;
    rdfs:subClassOf s223:Equipment ;
    sh:property [ sh:minCount 2 ;
            sh:path s223:hasConnectionPoint ] .

s223:MotorizedThreeWayValve a s223:Class,
        sh:NodeShape ;
    rdfs:label "Motorized three way valve" ;
    rdfs:subClassOf s223:MotorizedValve .

s223:MotorizedTwoWayValve a s223:Class,
        sh:NodeShape ;
    rdfs:label "Motorized two way valve" ;
    rdfs:subClassOf s223:MotorizedValve .

s223:Occupancy-Occupied a s223:EnumerationKind-Occupancy ;
    rdfs:label "Occupied" .

s223:Occupancy-Unknown a s223:EnumerationKind-Occupancy ;
    rdfs:label "Unknown" .

s223:Occupancy-Unoccupied a s223:EnumerationKind-Occupancy ;
    rdfs:label "Unoccupied" .

s223:OnOff-Unknown a s223:EnumerationKind-OnOff ;
    rdfs:label "Unknown" .

s223:Particulate-PM1.0 a s223:Substance-Particulate ;
    rdfs:label "Particulate-PM1.0" .

s223:Particulate-PM10.0 a s223:Substance-Particulate ;
    rdfs:label "Particulate-PM10.0" .

s223:Particulate-PM2.5 a s223:Substance-Particulate ;
    rdfs:label "Particulate-PM2.5" .

s223:ParticulateSensor a s223:Class,
        sh:NodeShape ;
    rdfs:label "Particulate sensor" ;
    rdfs:comment "A ParticulateSensor is a specialization of a Sensor that observes a QuantifiableObservableProperty that represents a particulate concentration measurement." ;
    rdfs:subClassOf s223:Sensor ;
    sh:property [ rdfs:comment "A ParticulateSensor can be associated with a Substance-Particulate by measuresSubstance" ;
            sh:class s223:Substance-Particulate ;
            sh:path s223:measuresSubstance ] .

s223:Phase-Solid a s223:EnumerationKind-Phase ;
    rdfs:label "Phase-Solid" .

s223:Phase-Vapor a s223:EnumerationKind-Phase ;
    rdfs:label "Phase-Vapor" .

s223:PhotovoltaicModule a s223:Class,
        sh:NodeShape ;
    rdfs:label "Photovoltaic module" ;
    rdfs:comment "A device that converts sunlight into electricity." ;
    rdfs:subClassOf s223:Equipment ;
    sh:property [ rdfs:comment "An PhotovoltaicModule shall have at least one outlet using the medium Electricity." ;
            sh:path s223:hasConnectionPoint ;
            sh:qualifiedMinCount 1 ;
            sh:qualifiedValueShape [ sh:class s223:OutletConnectionPoint ;
                    sh:node [ sh:property [ sh:class s223:Medium-Electricity ;
                                    sh:path s223:hasMedium ] ] ] ],
        [ rdfs:comment "An PhotovoltaicModule shall have at least one inlet using the medium EM-Light." ;
            sh:path s223:hasConnectionPoint ;
            sh:qualifiedMinCount 1 ;
            sh:qualifiedValueShape [ sh:class s223:InletConnectionPoint ;
                    sh:node [ sh:property [ sh:class s223:EM-Light ;
                                    sh:path s223:hasMedium ] ] ] ],
        [ sh:minCount 2 ;
            sh:path s223:hasConnectionPoint ] .

s223:Pipe a s223:Class,
        sh:NodeShape ;
    rdfs:label "Pipe" ;
    rdfs:comment "A Pipe is a subclass of Connection, that represents a hollow cylinder of metal or other material used to convey a Medium." ;
    rdfs:subClassOf s223:Connection .

s223:PositionStatus-Closed a s223:EnumerationKind-PositionStatus ;
    rdfs:label "Closed" .

s223:PositionStatus-Open a s223:EnumerationKind-PositionStatus ;
    rdfs:label "Open" .

s223:PositionStatus-Unknown a s223:EnumerationKind-PositionStatus ;
    rdfs:label "Unknown" .

s223:Presence-False a s223:Occupancy-Presence ;
    rdfs:label "Presence-False" .

s223:Pump a s223:Class,
        sh:NodeShape ;
    rdfs:label "Pump" ;
    rdfs:comment "A machine for imparting energy to a fluid, drawing a fluid into itself through an entrance port, and forcing the fluid out through an exhaust port." ;
    rdfs:subClassOf s223:Equipment ;
    sh:property [ rdfs:comment "A Pump shall have at least one inlet using the medium Water, Oil or Refrigerant." ;
            sh:path s223:hasConnectionPoint ;
            sh:qualifiedMinCount 1 ;
            sh:qualifiedValueShape [ sh:class s223:InletConnectionPoint ;
                    sh:node [ sh:or ( [ sh:property [ sh:class s223:Medium-Water ;
                                                sh:path s223:hasMedium ] ] [ sh:property [ sh:class s223:Medium-Refrigerant ;
                                                sh:path s223:hasMedium ] ] [ sh:property [ sh:class s223:Medium-Oil ;
                                                sh:path s223:hasMedium ] ] ) ] ] ],
        [ rdfs:comment "A Pump shall have at least one outlet using the medium Water, Oil or Refrigerant." ;
            sh:path s223:hasConnectionPoint ;
            sh:qualifiedMinCount 1 ;
            sh:qualifiedValueShape [ sh:class s223:OutletConnectionPoint ;
                    sh:node [ sh:or ( [ sh:property [ sh:class s223:Medium-Water ;
                                                sh:path s223:hasMedium ] ] [ sh:property [ sh:class s223:Medium-Refrigerant ;
                                                sh:path s223:hasMedium ] ] [ sh:property [ sh:class s223:Medium-Oil ;
                                                sh:path s223:hasMedium ] ] ) ] ] ],
        [ sh:minCount 2 ;
            sh:path s223:hasConnectionPoint ],
        [ rdfs:comment "The non-electrical ConnectionPoints of a Pump must have compatible Media." ;
            sh:path qudt:hasConnectionPoint ;
            sh:sparql [ a sh:SPARQLConstraint ;
                    sh:message "{?cpa} and {?cpb} on the Pump {$this} have incompatible Media {$mediuma} and {$mediumb}." ;
                    sh:prefixes s223: ;
                    sh:select """
SELECT $this ?cpa ?cpb ?mediuma ?mediumb
WHERE {
  $this s223:hasConnectionPoint ?cpa .
  $this s223:hasConnectionPoint ?cpb .
  FILTER (?cpa != ?cpb) .
  ?cpa s223:hasMedium ?mediuma .
  FILTER (NOT EXISTS {?mediuma a/rdfs:subClassOf* s223:Medium-Electricity}) .
  ?cpb s223:hasMedium ?mediumb .
  FILTER (NOT EXISTS {?mediumb a/rdfs:subClassOf* s223:Medium-Electricity}) .
  FILTER (?mediuma != ?mediumb) .
  FILTER (NOT EXISTS {?mediumb a/rdfs:subClassOf* ?mediuma}) .
  FILTER (NOT EXISTS {?mediuma a/rdfs:subClassOf* ?mediumb}) .
}
""" ] ] .

s223:RadiantPanel a s223:Class,
        sh:NodeShape ;
    rdfs:label "Radiant panel" ;
    rdfs:comment "A heating or cooling surface that delivers 50% or more of its heat transfer by radiation." ;
    rdfs:subClassOf s223:Equipment ;
    sh:or ( [ sh:property [ rdfs:comment "A radiant panel shall have at least one inlet using the medium Electricity, NaturalGas, or Water." ;
                        sh:minCount 1 ;
                        sh:path s223:hasConnectionPoint ;
                        sh:qualifiedMinCount 1 ;
                        sh:qualifiedValueShape [ sh:class s223:InletConnectionPoint ;
                                sh:node [ sh:property [ sh:class s223:Medium-Electricity ;
                                                sh:path s223:hasMedium ] ] ] ] ] [ sh:property [ rdfs:comment "A radiant panel shall have at least one inlet using the medium Electricity, NaturalGas, or Water." ;
                        sh:minCount 1 ;
                        sh:path s223:hasConnectionPoint ;
                        sh:qualifiedMinCount 1 ;
                        sh:qualifiedValueShape [ sh:class s223:InletConnectionPoint ;
                                sh:node [ sh:property [ sh:class s223:Medium-NaturalGas ;
                                                sh:path s223:hasMedium ] ] ] ] ] [ sh:property [ rdfs:comment "A radiant panel shall have at least one inlet using the medium Electricity, NaturalGas, or Water." ;
                        sh:minCount 2 ;
                        sh:path s223:hasConnectionPoint ;
                        sh:qualifiedMinCount 1 ;
                        sh:qualifiedValueShape [ sh:class s223:InletConnectionPoint ;
                                sh:node [ sh:property [ sh:class s223:Medium-Water ;
                                                sh:path s223:hasMedium ] ] ] ],
                    [ rdfs:comment "A radiant panel shall have at least one outlet using the medium Water." ;
                        sh:path s223:hasConnectionPoint ;
                        sh:qualifiedMinCount 1 ;
                        sh:qualifiedValueShape [ sh:class s223:OutletConnectionPoint ;
                                sh:node [ sh:property [ sh:class s223:Medium-Water ;
                                                sh:path s223:hasMedium ] ] ] ] ] ) ;
    sh:property [ rdfs:comment "A radiant panel must hasRole Role-Heating." ;
            sh:minCount 1 ;
            sh:path s223:hasRole ;
            sh:qualifiedMinCount 1 ;
            sh:qualifiedValueShape [ sh:class s223:Role-Heating ] ] .

s223:Radiator a s223:Class,
        sh:NodeShape ;
    rdfs:label "Radiator" ;
    rdfs:comment "A radiator provides heating to a room using electricity, steam or water (e.g., electric baseboard heaters)." ;
    rdfs:subClassOf s223:Equipment ;
    sh:or ( [ sh:property [ rdfs:comment "A Radiator shall have at least one inlet using the medium Electricity or Water." ;
                        sh:minCount 1 ;
                        sh:path s223:hasConnectionPoint ;
                        sh:qualifiedMinCount 1 ;
                        sh:qualifiedValueShape [ sh:class s223:InletConnectionPoint ;
                                sh:node [ sh:property [ sh:class s223:Medium-Electricity ;
                                                sh:path s223:hasMedium ] ] ] ] ] [ sh:property [ rdfs:comment "A Radiator shall have at least one inlet using the medium Electricity or Water." ;
                        sh:minCount 1 ;
                        sh:path s223:hasConnectionPoint ;
                        sh:qualifiedMinCount 1 ;
                        sh:qualifiedValueShape [ sh:class s223:InletConnectionPoint ;
                                sh:node [ sh:property [ sh:class s223:Medium-Water ;
                                                sh:path s223:hasMedium ] ] ] ],
                    [ rdfs:comment "A Radiator shall have at least one outlet using the medium Water." ;
                        sh:minCount 1 ;
                        sh:path s223:hasConnectionPoint ;
                        sh:qualifiedMinCount 1 ;
                        sh:qualifiedValueShape [ sh:class s223:OutletConnectionPoint ;
                                sh:node [ sh:property [ sh:class s223:Medium-Water ;
                                                sh:path s223:hasMedium ] ] ] ] ] ) ;
    sh:property [ rdfs:comment "Radiators must have the role Role-Heating." ;
            sh:minCount 1 ;
            sh:path s223:hasRole ;
            sh:qualifiedMinCount 1 ;
            sh:qualifiedValueShape [ sh:class s223:Role-Heating ] ] .

s223:Refrigerant-R-22 a s223:Medium-Refrigerant ;
    rdfs:label "Refrigerant-R-22" .

s223:Refrigerant-R-410A a s223:Medium-Refrigerant ;
    rdfs:label "Refrigerant-R-410A" .

s223:ResistanceHeater a s223:Class,
        sh:NodeShape ;
    rdfs:label "Electrical resistance heater" ;
    rdfs:comment "Resistance heaters provide electrical resistance heating, for example an electric heating coil within a Fan Coil Unit." ;
    rdfs:subClassOf s223:Equipment ;
    sh:property [ rdfs:comment "A ResistanceHeater shall have at least one inlet using the medium Electricity." ;
            sh:minCount 1 ;
            sh:path s223:hasConnectionPoint ;
            sh:qualifiedMinCount 1 ;
            sh:qualifiedValueShape [ sh:class s223:InletConnectionPoint ;
                    sh:node [ sh:property [ sh:class s223:Medium-Electricity ;
                                    sh:path s223:hasMedium ] ] ] ],
        [ rdfs:comment "ResistanceHeaters must have the role Role-Heating." ;
            sh:minCount 1 ;
            sh:path s223:hasRole ;
            sh:qualifiedMinCount 1 ;
            sh:qualifiedValueShape [ sh:class s223:Role-Heating ] ] .

s223:Role-Condenser a s223:EnumerationKind-Role ;
    rdfs:label "Role-Condenser" .

s223:Role-Discharge a s223:EnumerationKind-Role ;
    rdfs:label "Role-Discharge" .

s223:Role-Economizer a s223:EnumerationKind-Role ;
    rdfs:label "Role-Economizer" .

s223:Role-Evaporator a s223:EnumerationKind-Role ;
    rdfs:label "Role-Evaporator" .

s223:Role-Generator a s223:EnumerationKind-Role ;
    rdfs:label "Role-Generator" .

s223:Role-HeatRecovery a s223:EnumerationKind-Role ;
    rdfs:label "Heat Recovery" .

s223:Role-Load a s223:EnumerationKind-Role ;
    rdfs:label "Role-Load" .

s223:Role-Primary a s223:EnumerationKind-Role ;
    rdfs:label "Role-Primary" .

s223:Role-Recirculating a s223:EnumerationKind-Role ;
    rdfs:label "Role-Recirculating" .

s223:Role-Secondary a s223:EnumerationKind-Role ;
    rdfs:label "Role-Secondary" .

s223:RunStatus-Off a s223:EnumerationKind-RunStatus ;
    rdfs:label "Off" .

s223:RunStatus-On a s223:EnumerationKind-RunStatus ;
    rdfs:label "On" .

s223:RunStatus-Unknown a s223:EnumerationKind-RunStatus ;
    rdfs:label "Unknown" .

s223:Signal-EIA485 a s223:Electricity-Signal ;
    rdfs:label "Signal EIA485" .

s223:Signal-Ethernet a s223:Electricity-Signal ;
    rdfs:label "Signal Ethernet" .

s223:Signal-IEC14908 a s223:Electricity-Signal ;
    rdfs:label "Signal IEC14908" .

s223:Signal-USB a s223:Electricity-Signal ;
    rdfs:label "Signal USB" .

s223:SolarThermalCollector a s223:Class,
        sh:NodeShape ;
    rdfs:label "Solar thermal collector" ;
    rdfs:comment "A device that converts sunlight into thermal energy." ;
    rdfs:subClassOf s223:Equipment ;
    sh:property [ rdfs:comment "An SolarThermalCollector shall have at least one outlet using the medium Water." ;
            sh:path s223:hasConnectionPoint ;
            sh:qualifiedMinCount 1 ;
            sh:qualifiedValueShape [ sh:class s223:OutletConnectionPoint ;
                    sh:node [ sh:property [ sh:class s223:Medium-Water ;
                                    sh:path s223:hasMedium ] ] ] ],
        [ sh:minCount 2 ;
            sh:path s223:hasConnectionPoint ] .

s223:State a s223:Class,
        sh:NodeShape ;
    rdfs:label "State" ;
    rdfs:subClassOf s223:Concept .

s223:Substance-CO a s223:EnumerationKind-Substance ;
    rdfs:label "Substance-CO" .

s223:Substance-Soot a s223:EnumerationKind-Substance ;
    rdfs:label "Substance-Soot" .

s223:SymmetricPropertyShape a sh:NodeShape ;
    sh:rule [ a sh:SPARQLRule ;
            rdfs:comment "Declare the inverse triples for symmetric relations" ;
            sh:construct """
CONSTRUCT {
?o ?p $this .
}
WHERE {
  $this ?p ?o .
  ?p a s223:SymmetricProperty .
}
			""" ;
            sh:prefixes s223: ] ;
    sh:targetClass s223:Concept .

s223:Thermostat a s223:Class,
        sh:NodeShape ;
    rdfs:label "Thermostat" ;
    rdfs:comment "An automatic control device used to maintain temperature at a fixed or adjustable setpoint." ;
    rdfs:subClassOf s223:Equipment .

s223:ThreeSpeedSetting-High a s223:EnumerationKind-ThreeSpeedSetting ;
    rdfs:label "High" .

s223:ThreeSpeedSetting-Low a s223:EnumerationKind-ThreeSpeedSetting ;
    rdfs:label "Low" .

s223:ThreeSpeedSetting-Medium a s223:EnumerationKind-ThreeSpeedSetting ;
    rdfs:label "Medium" .

s223:ThreeSpeedSetting-Off a s223:EnumerationKind-ThreeSpeedSetting ;
    rdfs:label "Off" .

s223:ThreeWayValve a s223:Class,
        sh:NodeShape ;
    rdfs:label "Three way valve" ;
    rdfs:subClassOf s223:ManualValve .

s223:Turbine a s223:Class,
        sh:NodeShape ;
    rdfs:label "Turbine" ;
    rdfs:comment "An energy transducer that converts mechanical energy into electric energy." ;
    rdfs:subClassOf s223:Equipment ;
    sh:property [ rdfs:comment "A Turbine shall have at least one outlet using the medium Electricity." ;
            sh:class s223:OutletConnectionPoint ;
            sh:minCount 1 ;
            sh:node [ sh:property [ sh:class s223:Medium-Electricity ;
                            sh:path s223:hasMedium ] ] ;
            sh:path s223:hasConnectionPoint ],
        [ sh:minCount 1 ;
            sh:path s223:hasConnectionPoint ] .

s223:TwoWayValve a s223:Class,
        sh:NodeShape ;
    rdfs:label "Two way valve" ;
    rdfs:subClassOf s223:ManualValve .

s223:VFD a s223:Class,
        sh:NodeShape ;
    rdfs:label "VFD" ;
    rdfs:comment "An electronic device that varies its output frequency to vary the rotating speed of a motor, given a fixed input frequency. Used with fans or pumps to vary the flow in the system as a function of a maintained pressure." ;
    rdfs:subClassOf s223:Equipment ;
    sh:property [ rdfs:comment "A VFD shall have at least one inlet using the medium Electricity." ;
            sh:path s223:hasConnectionPoint ;
            sh:qualifiedMinCount 1 ;
            sh:qualifiedValueShape [ sh:class s223:InletConnectionPoint ;
                    sh:node [ sh:property [ sh:class s223:Medium-Electricity ;
                                    sh:path s223:hasMedium ] ] ] ],
        [ rdfs:comment "A VFD shall have at least one outlet using the medium Electricity." ;
            sh:path s223:hasConnectionPoint ;
            sh:qualifiedMinCount 1 ;
            sh:qualifiedValueShape [ sh:class s223:OutletConnectionPoint ;
                    sh:node [ sh:property [ sh:class s223:Medium-Electricity ;
                                    sh:path s223:hasMedium ] ] ] ],
        [ sh:minCount 2 ;
            sh:path s223:hasConnectionPoint ] .

s223:VariableFrequencyDrive a s223:Class,
        sh:NodeShape ;
    rdfs:label "VariableFrequencyDrive" ;
    rdfs:comment "electronic device that varies its output frequency to vary the rotating speed of a motor, given a fixed input frequency. Used with fans or pumps to vary the flow in the system as a function of a maintained pressure." ;
    rdfs:subClassOf s223:Equipment ;
    sh:property [ rdfs:comment "A VariableFrequencyDrive must connect to an equipment using electricity." ;
            sh:minCount 1 ;
            sh:path s223:hasConnectionPoint ;
            sh:qualifiedMinCount 1 ;
            sh:qualifiedValueShape [ sh:class s223:OutletConnectionPoint ;
                    sh:node [ sh:property [ sh:class s223:Medium-Electricity ;
                                    sh:path s223:hasMedium ] ] ] ],
        [ rdfs:comment "A VariableFrequencyDrive can only connect to equipment." ;
            sh:class s223:Equipment ;
            sh:path s223:connectedTo ] .

s223:Water-Steam a s223:Medium-Water ;
    rdfs:label "Steam" .

s223:WaterFilter a s223:Class,
        sh:NodeShape ;
    rdfs:label "Water filter" ;
    rdfs:comment "A device that removes particulates from water." ;
    rdfs:subClassOf s223:Filter ;
    sh:property [ rdfs:comment "A WaterFilter shall have at least one inlet using the medium Water." ;
            sh:path s223:hasConnectionPoint ;
            sh:qualifiedMinCount 1 ;
            sh:qualifiedValueShape [ sh:class s223:InletConnectionPoint ;
                    sh:node [ sh:property [ sh:class s223:Medium-Water ;
                                    sh:path s223:hasMedium ] ] ] ],
        [ rdfs:comment "A WaterFilter shall have at least one outlet using the medium Water." ;
            sh:path s223:hasConnectionPoint ;
            sh:qualifiedMinCount 1 ;
            sh:qualifiedValueShape [ sh:class s223:OutletConnectionPoint ;
                    sh:node [ sh:property [ sh:class s223:Medium-Water ;
                                    sh:path s223:hasMedium ] ] ] ] .

s223:Weekday-Friday a s223:DayOfWeek-Weekday ;
    rdfs:label "Friday" .

s223:Weekday-Monday a s223:DayOfWeek-Weekday ;
    rdfs:label "Monday" .

s223:Weekday-Thursday a s223:DayOfWeek-Weekday ;
    rdfs:label "Thursday" .

s223:Weekday-Tuesday a s223:DayOfWeek-Weekday ;
    rdfs:label "Tuesday" .

s223:Weekday-Wednesday a s223:DayOfWeek-Weekday ;
    rdfs:label "Wednesday" .

s223:Weekend-Saturday a s223:DayOfWeek-Weekend ;
    rdfs:label "Saturday" .

s223:Weekend-Sunday a s223:DayOfWeek-Weekend ;
    rdfs:label "Sunday" .

s223:WindowShade a s223:Class,
        sh:NodeShape ;
    rdfs:label "Window shade" ;
    rdfs:comment "A window covering that can be moved to block out or allow in light. " ;
    rdfs:subClassOf s223:Equipment .

s223:abstract a rdf:Property ;
    rdfs:label "abstract" ;
    rdfs:range xsd:boolean .

s223:countConnectedSystemCPs a sh:SPARQLFunction ;
    rdfs:comment "Given a SystemConnectionPoint, return the number in the connected set. This is not foolproof yet" ;
    sh:parameter [ a sh:Parameter ;
            sh:description "The starting SystemConnectionPoint" ;
            sh:path s223:scp ] ;
    sh:prefixes s223: ;
    sh:returnType xsd:integer ;
    sh:select """SELECT  (COUNT (DISTINCT ?others)AS ?count)
WHERE {
{
$scp  s223:systemConnected+ ?others .
}
UNION
{
$scp  ^s223:systemConnected+ ?others .
}
UNION
{
$scp  s223:systemConnected+/^s223:systemConnected+ ?others .
}
UNION
{
$scp  ^s223:systemConnected+/s223:systemConnected+ ?others .
}
}
GROUP BY $scp
  """ .

s223:hasFrequency a rdf:Property ;
    rdfs:label "has frequency" ;
    rdfs:comment "The relation hasFrequency is used to identify the frequency of an AC electricity enumeration kind. " .

s223:hasNumberOfElectricalPhases a rdf:Property ;
    rdfs:label "has number of electrical phases" ;
    rdfs:comment "The relation hasNumberOfElectricalPhases is used to identify the number of electrical phases in an AC electricity enumeration kind. " .

s223:hasTemperature a rdf:Property ;
    rdfs:label "hasTemperature" ;
    rdfs:subPropertyOf s223:hasProperty .

s223:hasVoltage a rdf:Property ;
    rdfs:label "hasVoltage" ;
    rdfs:comment "The relation hasVoltage is used to identify the voltage of an electricity enumeration kind. " .

s223:inverseOf a rdf:Property ;
    rdfs:label "inverse of" .

s223:lnxConnected a sh:SPARQLFunction ;
    rdfs:comment "Given two entities (Junctions or ConnectionPoints), return a Junction in the lnx network, if a path exists." ;
    sh:parameter [ a sh:Parameter ;
            sh:description "The starting entity" ;
            sh:path s223:entity1 ],
        [ a sh:Parameter ;
            sh:description "The ending entity" ;
            sh:path s223:entity2 ] ;
    sh:prefixes s223: ;
    sh:returnType s223:Junction ;
    sh:select """SELECT ?others
WHERE {
$entity1 s223:lnx+ $entity2 .
$entity1 s223:lnx+ ?others .
?others a s223:Junction .
FILTER(?others != $entity1) .
FILTER(?others != $entity2) .
}
  """ .

s223:networkCrossesSystemBoundary a sh:SPARQLFunction ;
    rdfs:comment "Given a ConnectionPoint, determine if its contiguous lnx network crosses the containing System boundary. This assumes the network is complete." ;
    sh:ask """
ASK {
$arg1 s223:isConnectionPointOf/^s223:contains ?homeSystem .
$arg1 s223:lnx* ?member .
?class rdfs:subClassOf* s223:ConnectionPoint .
?member a ?class .
?member s223:isConnectionPointOf ?dev .
?dev ^s223:contains ?system .
FILTER (?system != ?homeSystem) .
}
  """ ;
    sh:parameter [ a sh:Parameter ;
            sh:description "The starting ConnectionPoint" ;
            sh:path s223:arg1 ] ;
    sh:prefixes s223: ;
    sh:returnType xsd:boolean .

<http://data.ashrae.org/standard223/1.0/data/brick-test> a owl:Ontology ;
    rdfs:comment "This graph is a sample population of the so-called Pritoni Office Building (suggested by Marco Pritoni) and is used for testing and demonstration." ;
    owl:imports <http://data.ashrae.org/standard223/1.0/model/all>,
        <https://brickschema.org/extension/brick_extension_interpret_223> ;
    owl:versionInfo "Created with TopBraid Composer" .

psm:BathroomExhaustFan a s223:Fan ;
    rdfs:label "Bathroom exhaust fan" ;
    s223:hasConnectionPoint psm:FanInletConnectionPoint,
        psm:FanOutletConnectionPoint ;
    s223:hasProperty psm:ExhaustFanStatus ;
    s223:hasRole s223:Role-Exhaust .

psm:BreakerPanel1 a s223:System ;
    rdfs:label "Breaker panel1" ;
    s223:hasMember psm:ElectricBreaker1,
        psm:ElectricBreaker2,
        psm:ElectricBreaker3,
        psm:ElectricBreaker4,
        psm:ElectricBreaker5 .

psm:CoolingCoilValveActuator a s223:Actuator ;
    rdfs:label "A5" ;
    s223:commandedByProperty psm:CoolingCoilValvePosition .

psm:DaylightSensor1 a s223:IlluminanceSensor ;
    rdfs:label "D1" ;
    s223:hasMeasurementLocation psm:LightingSpace1 ;
    s223:hasPhysicalLocation psm:OpenOffice ;
    s223:observes psm:OpenOfficeDaylightLevel .

psm:ElectricCircuit4 a s223:ElectricWire ;
    rdfs:label "Electric Circuit 4" ;
    s223:hasMedium s223:AC-120V-60Hz .

psm:ElectricCircuit5 a s223:ElectricWire ;
    rdfs:label "Electric Circuit 5" ;
    s223:hasMedium s223:AC-120V-60Hz .

psm:ExhaustAirDamperActuator a s223:Actuator ;
    rdfs:label "A1" ;
    s223:commandedByProperty psm:ExhaustAirDamperPosition .

psm:Floor1 a s223:PhysicalSpace ;
    rdfs:label "Floor1" ;
    s223:contains psm:Bathroom,
        psm:Corridor,
        psm:Kitchenette,
        psm:OpenOffice,
        psm:PrivateOffice .

psm:FlowSensor1 a s223:FlowSensor ;
    rdfs:label "S1" ;
    s223:hasMeasurementLocation psm:i00053 ;
    s223:observes psm:ReturnAirFlowRate .

psm:GridConnection a s223:ElectricWire ;
    rdfs:label "Grid connection" ;
    s223:hasMedium s223:AC-120V-240V-60Hz .

psm:HVACZone1 a s223:Zone ;
    rdfs:label "HVACZone1" ;
    s223:contains psm:HVACSpace1,
        psm:HVACSpace2,
        psm:HVACSpace3,
        psm:HVACSpace4 ;
    s223:hasDomain s223:Domain-HVAC .

psm:HVACZone1Thermostat a s223:TemperatureSensor ;
    rdfs:label "TH1" ;
    s223:hasMeasurementLocation psm:HVACSpace1 ;
    s223:hasPhysicalLocation psm:OpenOffice ;
    s223:observes psm:HVACZone1Temperature .

psm:HVACZone2Thermostat a s223:TemperatureSensor ;
    rdfs:label "TH2" ;
    s223:hasMeasurementLocation psm:HVACSpace5 ;
    s223:hasPhysicalLocation psm:Corridor ;
    s223:observes psm:HVACZone2Temperature .

psm:HeatingCoilValveActuator a s223:Actuator ;
    rdfs:label "A4" ;
    s223:commandedByProperty psm:HeatingCoilValvePosition .

psm:KitchenetteLightingSystem a s223:System ;
    rdfs:label "Kitchenette lighting system" ;
    s223:hasMember psm:Luminaire11,
        psm:Luminaire12,
        psm:OccSensor5 .

psm:LightingZone1 a s223:Zone ;
    rdfs:label "LightingZone1" ;
    s223:contains psm:LightingSpace1 ;
    s223:hasDomain s223:Domain-Lighting .

psm:LightingZone2 a s223:Zone ;
    rdfs:label "LightingZone2" ;
    s223:contains psm:LightingSpace2 ;
    s223:hasDomain s223:Domain-Lighting .

psm:LightingZone3 a s223:Zone ;
    rdfs:label "LightingZone3" ;
    s223:contains psm:LightingSpace3 ;
    s223:hasDomain s223:Domain-Lighting .

psm:LightingZone4 a s223:Zone ;
    rdfs:label "LightingZone4" ;
    s223:contains psm:LightingSpace4 ;
    s223:hasDomain s223:Domain-Lighting .

psm:LightingZone5 a s223:Zone ;
    rdfs:label "LightingZone5" ;
    s223:contains psm:LightingSpace5 ;
    s223:hasDomain s223:Domain-Lighting .

psm:LightingZone6 a s223:Zone ;
    rdfs:label "LightingZone6" ;
    s223:contains psm:LightingSpace6 ;
    s223:hasDomain s223:Domain-Lighting .

psm:Luminaire1 a s223:Luminaire ;
    rdfs:label "Luminaire1" ;
    s223:cnx psm:Luminaire1Inlet,
        psm:Luminaire1Outlet ;
    s223:contains psm:Driver1,
        psm:LightEngine1 .

psm:Luminaire10 a s223:Luminaire ;
    rdfs:label "Luminaire10" ;
    s223:hasConnectionPoint psm:Luminaire10Inlet,
        psm:Luminaire10Outlet ;
    s223:hasProperty psm:Luminaire10OnOffStatus .

psm:Luminaire1FunctionBlock a s223:FunctionBlock ;
    rdfs:label "Luminaire1function block" ;
    s223:hasInput psm:Luminaire1DaylightFunctionInput,
        psm:Luminaire1OccupancyFunctionInput ;
    s223:hasOutput psm:Luminaire1CCTSettingOutput,
        psm:Luminaire1IntensitySettingOutput,
        psm:Luminaire1OnOffSettingOutput .

psm:Luminaire2 a s223:Luminaire ;
    rdfs:label "Luminaire2" ;
    s223:commandedByProperty psm:Luminaire2CCT,
        psm:Luminaire2Intensity,
        psm:Luminaire2OnOff ;
    s223:hasConnectionPoint psm:Luminaire2Inlet,
        psm:Luminaire2Outlet ;
    s223:hasProperty psm:Luminaire2OnOffStatus .

psm:Luminaire2FunctionBlock a s223:FunctionBlock ;
    rdfs:label "Luminaire2 function block" ;
    s223:hasInput psm:Luminaire2DaylightFunctionInput,
        psm:Luminaire2OccupancyFunctionInput1 ;
    s223:hasOutput psm:Luminaire2CCTSettingOutput,
        psm:Luminaire2IntensitySettingOutput,
        psm:Luminaire2OnOffSettingOutput .

psm:Luminaire3 a s223:Luminaire ;
    rdfs:label "Luminaire3" ;
    s223:hasConnectionPoint psm:Luminaire3Inlet,
        psm:Luminaire3Outlet ;
    s223:hasProperty psm:Luminaire3OnOffStatus .

psm:Luminaire4 a s223:Luminaire ;
    rdfs:label "Luminaire4" ;
    s223:hasConnectionPoint psm:Luminaire4Inlet,
        psm:Luminaire4Outlet ;
    s223:hasProperty psm:Luminaire4OnOffStatus .

psm:Luminaire5 a s223:Luminaire ;
    rdfs:label "Luminaire5" ;
    s223:hasConnectionPoint psm:Luminaire5Inlet,
        psm:Luminaire5Outlet ;
    s223:hasProperty psm:Luminaire5OnOffStatus .

psm:Luminaire6 a s223:Luminaire ;
    rdfs:label "Luminaire6" ;
    s223:hasConnectionPoint psm:Luminaire6Inlet,
        psm:Luminaire6Outlet ;
    s223:hasProperty psm:Luminaire6OnOffStatus .

psm:Luminaire7 a s223:Luminaire ;
    rdfs:label "Luminaire7" ;
    s223:hasConnectionPoint psm:Luminaire7Inlet,
        psm:Luminaire7Outlet ;
    s223:hasProperty psm:Luminaire7OnOffStatus .

psm:Luminaire8 a s223:Luminaire ;
    rdfs:label "Luminaire8" ;
    s223:hasConnectionPoint psm:Luminaire8Inlet,
        psm:Luminaire8Outlet ;
    s223:hasProperty psm:Luminaire8OnOffStatus .

psm:Luminaire9 a s223:Luminaire ;
    rdfs:label "Luminaire9" ;
    s223:hasConnectionPoint psm:Luminaire9Inlet,
        psm:Luminaire9Outlet ;
    s223:hasProperty psm:Luminaire9OnOffStatus .

psm:MainBreaker a s223:ElectricBreaker ;
    rdfs:label "Main breaker" ;
    s223:hasConnectionPoint psm:MainBreakerInletCP,
        psm:MainBreakerOutCP1,
        psm:MainBreakerOutCP2,
        psm:MainBreakerOutCP3 .

psm:MixedAirDamperActuator a s223:Actuator ;
    rdfs:label "A2" ;
    s223:commandedByProperty psm:MixedAirDamperPosition .

psm:MixedAirPressureSensor a s223:PressureSensor ;
    rdfs:label "S5" ;
    s223:hasMeasurementLocation psm:i00024 ;
    s223:observes psm:MixedAirPressure .

psm:OccSensor1 a s223:OccupantCounter ;
    rdfs:label "O1" ;
    s223:hasMeasurementLocation psm:OccupancySpace1 ;
    s223:hasPhysicalLocation psm:OpenOffice ;
    s223:observes psm:OccupancyProp1 .

psm:OccSensor2 a s223:OccupantMotionSensor ;
    rdfs:label "O2" ;
    s223:hasMeasurementLocation psm:OccupancySpace2 ;
    s223:hasPhysicalLocation psm:Bathroom ;
    s223:observes psm:OccupancyProp2 .

psm:OccSensor3 a s223:OccupantPresenceSensor ;
    rdfs:label "O3" ;
    s223:hasMeasurementLocation psm:OccupancySpace3 ;
    s223:observes psm:OccupancyProp3 .

psm:OccSensor4 a s223:OccupantMotionSensor ;
    rdfs:label "O4" ;
    s223:hasMeasurementLocation psm:OccupancySpace4 ;
    s223:observes psm:OccupancyProp4 .

psm:OpeningCB a s223:Connection ;
    rdfs:label "Opening CB" ;
    s223:cnx psm:BathroomInletConnectionPoint,
        psm:CorridorOutletConnectionPointB ;
    s223:hasMedium s223:Medium-Air .

psm:OpeningCOO a s223:Connection ;
    rdfs:label "Opening COO" ;
    s223:cnx psm:CorridorOutletConnectionPointOO,
        psm:OpenOfficeInletConnectionPoint ;
    s223:hasMedium s223:Medium-Air .

psm:OpeningKC a s223:Connection ;
    rdfs:label "Opening KC" ;
    s223:cnx psm:CorridorInletConnectionPointK,
        psm:KitchenetteOutletConnectionPoint ;
    s223:hasMedium s223:Medium-Air .

psm:OpeningPOC a s223:Connection ;
    rdfs:label "Opening POC" ;
    s223:cnx psm:CorridorInletConnectionPointPO,
        psm:PrivateOfficeOutletConnectionPoint ;
    s223:hasMedium s223:Medium-Air .

psm:OutsideAirDamperActuator a s223:Actuator ;
    rdfs:label "A3" ;
    s223:commandedByProperty psm:OutsideAirDamperPosition .

psm:PipeFromBoiler a s223:Connection ;
    rdfs:label "Pipe from boiler" ;
    s223:cnx psm:i00032 ;
    s223:hasMedium s223:Water-HotWater .

psm:Resource_1 a rdfs:Resource ;
    rdfs:label "Resource 1" .

psm:ReturnFanActuator a s223:Actuator ;
    rdfs:label "A8" ;
    s223:commandedByProperty psm:ReturnFanSpeed .

psm:ReturnSystem a s223:System ;
    rdfs:label "Return System" ;
    s223:hasMember psm:i00051,
        psm:i00056 ;
    s223:hasRole s223:Role-Return .

psm:RoomSupply1 a s223:Connection ;
    rdfs:label "Room supply1" ;
    s223:cnx psm:PrivateOfficeInletConnectionPoint,
        psm:VAV1OuletReheatCoilCP ;
    s223:hasMedium s223:Medium-Air .

psm:RoomSupply2 a s223:Connection ;
    rdfs:label "Room supply2" ;
    s223:cnx psm:KitchenetteInletConnectionPoint,
        psm:VAV2OuletReheatCoilCP ;
    s223:hasMedium s223:Medium-Air .

psm:SupplyFanActuator a s223:Actuator ;
    rdfs:label "A9" ;
    s223:commandedByProperty psm:SupplyFanSpeed .

psm:SupplySystem a s223:System ;
    rdfs:label "Supply System" ;
    s223:hasMember psm:i00007,
        psm:i00011,
        psm:i00016,
        psm:i00021,
        psm:i00025,
        psm:i00036,
        psm:i00047 ;
    s223:hasRole s223:Role-Supply .

psm:TempSensor_1 a s223:TemperatureSensor ;
    rdfs:label "S7" ;
    s223:hasMeasurementLocation psm:i00050 ;
    s223:observes psm:CoolingCoilOutletTemperature .

psm:TempSensor_2 a s223:TemperatureSensor ;
    rdfs:label "S6" ;
    s223:hasMeasurementLocation psm:i00046 ;
    s223:observes psm:HeatingCoilOutletTemperature .

psm:VAV1InletTemperature a s223:QuantifiableObservableProperty ;
    rdfs:label "VAV1 Inlet Temperature" ;
    s223:hasValue 70.2 ;
    qudt:hasQuantityKind quantitykind:Temperature ;
    qudt:unit unit:DEG_F .

psm:VAV1InternalConnection a s223:Connection ;
    rdfs:label "VAV1Internal connection" ;
    s223:cnx psm:VAV1DamperOutletCP,
        psm:VAV1InletReheatCoilCP ;
    s223:hasMedium s223:Medium-Air .

psm:VAV2InternalConnection a s223:Connection ;
    rdfs:label "VAV2Internal connection" ;
    s223:cnx psm:VAV2DamperOutletCP,
        psm:VAV2InletReheatCoilCP ;
    s223:hasMedium s223:Medium-Air .

psm:VAV2OutletTemperature a s223:QuantifiableObservableProperty ;
    rdfs:label "VAV2 Outlet Temperature" ;
    s223:hasValue 71.2 ;
    qudt:hasQuantityKind quantitykind:Temperature ;
    qudt:unit unit:DEG_F .

psm:VAVBox1 a s223:VAVUnit ;
    rdfs:label "VAVBox1" ;
    s223:cnx psm:VAVBox1Inlet,
        psm:VAVBox1Outlet ;
    s223:contains psm:VAVBox1HeatingCoil,
        psm:VAVBox1InletFlowSensor,
        psm:VAVBox1MotorizedDamper,
        psm:VAVBox1OutletTemperatureSensor .

psm:VAVBox1DamperActuator a s223:Actuator ;
    rdfs:label "A10" ;
    s223:commandedByProperty psm:VAVBox1DamperPosition .

psm:VAVBox1ReheatValveActuator a s223:Actuator ;
    rdfs:label "A11" ;
    s223:commandedByProperty psm:VAVBox1ReheatValvePosition .

psm:VAVBox2 a s223:VAVUnit ;
    rdfs:label "VAVBox2" ;
    s223:contains psm:VAVBox2HeatingCoil,
        psm:VAVBox2InletFlowSensor,
        psm:VAVBox2MotorizedDamper,
        psm:VAVBox2OutletTemperatureSensor ;
    s223:hasConnectionPoint psm:VAVBox2Inlet,
        psm:VAVBox2Outlet ;
    s223:servesZone psm:HVACZone2 .

psm:VAVBox2DamperActuator a s223:Actuator ;
    rdfs:label "A6" ;
    s223:commandedByProperty psm:VAVBox2DamperPosition .

psm:VAVBox2ReheatValveActuator a s223:Actuator ;
    rdfs:label "A7" ;
    s223:commandedByProperty psm:VAVBox2ReheatValvePosition .

psm:i00001 a s223:AirHandlingUnit ;
    rdfs:label "AHU" ;
    s223:contains psm:i00007,
        psm:i00011,
        psm:i00016,
        psm:i00021,
        psm:i00025,
        psm:i00030,
        psm:i00036,
        psm:i00041,
        psm:i00047,
        psm:i00051,
        psm:i00056,
        psm:i00061 ;
    s223:hasConnectionPoint psm:AHUChilledWaterInlet,
        psm:AHUChilledWaterOutlet,
        psm:AHUExhaustOutlet,
        psm:AHUHotWaterInlet,
        psm:AHUHotWaterOutlet,
        psm:AHUOAInlet,
        psm:AHUReturnInlet,
        psm:AHUSupplyOutlet .

psm:i00070 a s223:Connection ;
    rdfs:label "Supply Air Duct" ;
    s223:hasMedium s223:Medium-Air ;
    s223:hasProperty psm:sap .

psm:masen a s223:Sensor ;
    rdfs:label "S4" ;
    s223:observes psm:mxtmp .

psm:oasen a s223:TemperatureSensor ;
    rdfs:label "S3" ;
    s223:hasMeasurementLocation psm:i00013 ;
    s223:observes psm:oatmp .

psm:rasen a s223:TemperatureSensor ;
    rdfs:label "S2" ;
    s223:hasMeasurementLocation psm:i00052 ;
    s223:observes psm:ratmp .

psm:sasen a s223:PressureSensor ;
    rdfs:label "S8" ;
    s223:hasMeasurementLocation psm:i00049 ;
    s223:observes psm:sap .

<http://data.ashrae.org/standard223/1.0/extension/function/shacl> rdfs:comment "This graph contains some SPARQLFunction definitions, which are part of SHACL Advanced Features (SHACL AF). Thus, they may not be supported by all SHACL implementations." ;
    owl:imports <http://data.ashrae.org/standard223/1.0/model/all>,
        sh: ;
    owl:versionInfo "Created with TopBraid Composer" .

g36:AirFlowStationAnnotation a sh:NodeShape ;
    sh:rule [ a sh:TripleRule ;
            sh:condition g36:AirFlowStationRule ;
            sh:object g36:AirFlowStation ;
            sh:predicate rdf:type ;
            sh:subject sh:this ] ;
    sh:targetClass s223:Sensor .

g36:BinaryOut a s223:Class,
        sh:NodeShape ;
    rdfs:label "Binary out" ;
    rdfs:subClassOf s223:EnumeratedActuatableProperty ;
    sh:rule [ a sh:TripleRule ;
            rdfs:comment "An instance of g36:BinaryOut has a value that is a member of the EnumerationKind g36:RunCommand." ;
            sh:object g36:RunCommand ;
            sh:predicate s223:hasEnumerationKind ;
            sh:subject sh:this ] .

g36:Damper a s223:Class,
        sh:Nodeshape ;
    rdfs:label "Damper" ;
    rdfs:subClassOf s223:Damper ;
    sh:node g36:DamperRule .

g36:Damper42 a s223:Class,
        sh:Nodeshape ;
    rdfs:label "Damper for VAV with Reheat" ;
    rdfs:subClassOf s223:Damper ;
    sh:node g36:DamperRule42 .

g36:RunCommand-Start a g36:RunCommand ;
    rdfs:label "Start" .

g36:RunCommand-Stop a g36:RunCommand ;
    rdfs:label "Stop" .

g36:RunStatus-Off a g36:RunStatus ;
    rdfs:label "Off" .

g36:RunStatus-On a g36:RunStatus ;
    rdfs:label "On" .

g36:RunStatus-Unknown a g36:RunStatus ;
    rdfs:label "Unknown" .

g36:TemperatureSensor a s223:Class,
        sh:NodeShape ;
    rdfs:label "Supply Air Temperature Sensor" ;
    rdfs:subClassOf s223:TemperatureSensor ;
    sh:property [ rdfs:comment "Supply air temperature sensor in a VAV with reheat" ;
            sh:path s223:observes ;
            sh:qualifiedMinCount 1 ;
            sh:qualifiedValueShape [ sh:class g36:AnalogIn ;
                    sh:node [ sh:property [ sh:hasValue quantitykind:Temperature ;
                                    sh:path qudt:hasQuantityKind ] ] ] ] .

g36:VAV_4-1 a s223:Class,
        sh:NodeShape ;
    rdfs:label "VAV with Cooling Only",
        "VAV_4-1" ;
    sh:class g36:VAV ;
    sh:property [ sh:class s223:DomainSpace ;
            sh:minCount 1 ;
            sh:node [ sh:property [ sh:class g36:Zone ;
                            sh:minCount 1 ;
                            sh:path [ sh:inversePath s223:contains ] ] ] ;
            sh:path s223:connectedTo ],
        [ sh:class s223:DomainSpace ;
            sh:minCount 1 ;
            sh:node [ sh:property [ sh:class g36:Zone ;
                            sh:minCount 1 ;
                            sh:path [ sh:inversePath s223:contains ] ] ] ;
            sh:path s223:connectedTo ] .

g36:VAV_4-2 a s223:Class,
        sh:NodeShape ;
    rdfs:label "VAV with reheat" ;
    rdfs:comment "This could just be a rule, rather than a subclass of VAVWithReheat. Not sure which pattern is more sensible" ;
    sh:class g36:VAVWithReheat ;
    sh:property [ sh:class s223:DomainSpace ;
            sh:minCount 1 ;
            sh:node [ sh:property [ sh:class g36:Zone ;
                            sh:minCount 1 ;
                            sh:path [ sh:inversePath s223:contains ] ] ] ;
            sh:path s223:connectedTo ;
            sh:severity s223:g36 ] .

<http://data.ashrae.org/standard223/1.0/extensions/settings> rdfs:comment """This file can be used to control which extensions are to be loaded with the 223 ontology by importing the appropriate graph(s). Options include:
For access to magic properties and other SPIN functions - http://data.ashraw.org/standard223/1.0/function/spin.  
For validation of the schema, model, or data - http://data.ashrae.org/standard223/1.0/validation/schema (or model or data).  
For inferred properties - http://data.ashrae.org/standard223/1.0/inference/model-rules (and/or schema-rules, data-rules)""" ;
    owl:imports <http://data.ashrae.org/standard223/1.0/extension/equipments>,
        <http://data.ashrae.org/standard223/1.0/extension/equipments-extensions-rules>,
        <http://data.ashrae.org/standard223/1.0/extension/g36>,
        <http://data.ashrae.org/standard223/1.0/inference/data-rules>,
        <http://data.ashrae.org/standard223/1.0/inference/model-rules>,
        <http://data.ashrae.org/standard223/1.0/inference/owl-subset>,
        <http://data.ashrae.org/standard223/1.0/validation/data>,
        <http://data.ashrae.org/standard223/1.0/validation/model>,
        <http://data.ashrae.org/standard223/1.0/validation/schema> ;
    owl:versionInfo "Created with TopBraid Composer" .

<http://data.ashrae.org/standard223/1.0/function/spin> owl:imports <http://spinrdf.org/spl> ;
    owl:versionInfo "Created with TopBraid Composer" .

<http://data.ashrae.org/standard223/1.0/model/core> owl:imports <http://data.ashrae.org/standard223/1.0/model/all> ;
    owl:versionInfo "Created with TopBraid Composer" .

<http://data.ashrae.org/standard223/1.0/model/device> owl:imports <http://data.ashrae.org/standard223/1.0/model/all> ;
    owl:versionInfo "Created with TopBraid Composer" .

<http://data.ashrae.org/standard223/1.0/model/fnblck> owl:imports <http://data.ashrae.org/standard223/1.0/model/all> .

<http://data.ashrae.org/standard223/1.0/vocab/enumeration> owl:imports <http://data.ashrae.org/standard223/1.0/model/all>,
        <http://data.ashrae.org/standard223/1.0/vocab/electricity> ;
    owl:versionInfo "Created with TopBraid Composer" .

spin:allProperties a spin:MagicProperty ;
    rdfs:label "Find all Properties" ;
    spin:body [ a sp:Select ;
            sp:resultVariables ( [ sp:varName "value" ] ) ;
            sp:where ( [ a sp:TriplePath ;
                        sp:object s223:hasProperty ;
                        sp:path [ a sp:ModPath ;
                                sp:modMax -2 ;
                                sp:modMin 0 ;
                                sp:subPath rdfs:subPropertyOf ] ;
                        sp:subject [ sp:varName "property" ] ] [ sp:object [ sp:varName "value" ] ;
                        sp:predicate [ sp:varName "property" ] ;
                        sp:subject spin:_arg1 ] ) ] ;
    spin:constraint [ a spl:Argument ;
            spl:optional false ;
            spl:predicate sp:arg1 ;
            rdfs:comment "The resource that has Properties" ] ;
    spin:returnType rdfs:Class ;
    rdfs:subClassOf spin:MagicProperties .

sh:AndConstraintComponent a sh:ConstraintComponent ;
    rdfs:label "And constraint component"@en ;
    rdfs:comment "A constraint component that can be used to test whether a value node conforms to all members of a provided list of shapes."@en ;
    rdfs:isDefinedBy sh: ;
    sh:parameter sh:AndConstraintComponent-and .

sh:ClassConstraintComponent a sh:ConstraintComponent ;
    rdfs:label "Class constraint component"@en ;
    rdfs:comment "A constraint component that can be used to verify that each value node is an instance of a given type."@en ;
    rdfs:isDefinedBy sh: ;
    sh:parameter sh:ClassConstraintComponent-class .

sh:ClosedConstraintComponent a sh:ConstraintComponent ;
    rdfs:label "Closed constraint component"@en ;
    rdfs:comment "A constraint component that can be used to indicate that focus nodes must only have values for those properties that have been explicitly enumerated via sh:property/sh:path."@en ;
    rdfs:isDefinedBy sh: ;
    sh:parameter sh:ClosedConstraintComponent-closed,
        sh:ClosedConstraintComponent-ignoredProperties .

sh:DatatypeConstraintComponent a sh:ConstraintComponent ;
    rdfs:label "Datatype constraint component"@en ;
    rdfs:comment "A constraint component that can be used to restrict the datatype of all value nodes."@en ;
    rdfs:isDefinedBy sh: ;
    sh:parameter sh:DatatypeConstraintComponent-datatype .

sh:DisjointConstraintComponent a sh:ConstraintComponent ;
    rdfs:label "Disjoint constraint component"@en ;
    rdfs:comment "A constraint component that can be used to verify that the set of value nodes is disjoint with the the set of nodes that have the focus node as subject and the value of a given property as predicate."@en ;
    rdfs:isDefinedBy sh: ;
    sh:parameter sh:DisjointConstraintComponent-disjoint .

sh:EqualsConstraintComponent a sh:ConstraintComponent ;
    rdfs:label "Equals constraint component"@en ;
    rdfs:comment "A constraint component that can be used to verify that the set of value nodes is equal to the set of nodes that have the focus node as subject and the value of a given property as predicate."@en ;
    rdfs:isDefinedBy sh: ;
    sh:parameter sh:EqualsConstraintComponent-equals .

sh:ExpressionConstraintComponent a sh:ConstraintComponent ;
    rdfs:label "Expression constraint component"@en ;
    rdfs:comment "A constraint component that can be used to verify that a given node expression produces true for all value nodes."@en ;
    rdfs:isDefinedBy sh: ;
    sh:parameter sh:ExpressionConstraintComponent-expression .

sh:HasValueConstraintComponent a sh:ConstraintComponent ;
    rdfs:label "Has-value constraint component"@en ;
    rdfs:comment "A constraint component that can be used to verify that one of the value nodes is a given RDF node."@en ;
    rdfs:isDefinedBy sh: ;
    sh:parameter sh:HasValueConstraintComponent-hasValue .

sh:InConstraintComponent a sh:ConstraintComponent ;
    rdfs:label "In constraint component"@en ;
    rdfs:comment "A constraint component that can be used to exclusively enumerate the permitted value nodes."@en ;
    rdfs:isDefinedBy sh: ;
    sh:parameter sh:InConstraintComponent-in .

sh:JSConstraintComponent a sh:ConstraintComponent ;
    rdfs:label "JavaScript constraint component"@en ;
    rdfs:comment "A constraint component with the parameter sh:js linking to a sh:JSConstraint containing a sh:script."@en ;
    rdfs:isDefinedBy sh: ;
    sh:parameter sh:JSConstraint-js .

sh:LanguageInConstraintComponent a sh:ConstraintComponent ;
    rdfs:label "Language-in constraint component"@en ;
    rdfs:comment "A constraint component that can be used to enumerate language tags that all value nodes must have."@en ;
    rdfs:isDefinedBy sh: ;
    sh:parameter sh:LanguageInConstraintComponent-languageIn .

sh:LessThanConstraintComponent a sh:ConstraintComponent ;
    rdfs:label "Less-than constraint component"@en ;
    rdfs:comment "A constraint component that can be used to verify that each value node is smaller than all the nodes that have the focus node as subject and the value of a given property as predicate."@en ;
    rdfs:isDefinedBy sh: ;
    sh:parameter sh:LessThanConstraintComponent-lessThan .

sh:LessThanOrEqualsConstraintComponent a sh:ConstraintComponent ;
    rdfs:label "less-than-or-equals constraint component"@en ;
    rdfs:comment "A constraint component that can be used to verify that every value node is smaller than all the nodes that have the focus node as subject and the value of a given property as predicate."@en ;
    rdfs:isDefinedBy sh: ;
    sh:parameter sh:LessThanOrEqualsConstraintComponent-lessThanOrEquals .

sh:MaxCountConstraintComponent a sh:ConstraintComponent ;
    rdfs:label "Max-count constraint component"@en ;
    rdfs:comment "A constraint component that can be used to restrict the maximum number of value nodes."@en ;
    rdfs:isDefinedBy sh: ;
    sh:parameter sh:MaxCountConstraintComponent-maxCount .

sh:MaxExclusiveConstraintComponent a sh:ConstraintComponent ;
    rdfs:label "Max-exclusive constraint component"@en ;
    rdfs:comment "A constraint component that can be used to restrict the range of value nodes with a maximum exclusive value."@en ;
    rdfs:isDefinedBy sh: ;
    sh:parameter sh:MaxExclusiveConstraintComponent-maxExclusive .

sh:MaxInclusiveConstraintComponent a sh:ConstraintComponent ;
    rdfs:label "Max-inclusive constraint component"@en ;
    rdfs:comment "A constraint component that can be used to restrict the range of value nodes with a maximum inclusive value."@en ;
    rdfs:isDefinedBy sh: ;
    sh:parameter sh:MaxInclusiveConstraintComponent-maxInclusive .

sh:MaxLengthConstraintComponent a sh:ConstraintComponent ;
    rdfs:label "Max-length constraint component"@en ;
    rdfs:comment "A constraint component that can be used to restrict the maximum string length of value nodes."@en ;
    rdfs:isDefinedBy sh: ;
    sh:parameter sh:MaxLengthConstraintComponent-maxLength .

sh:MinCountConstraintComponent a sh:ConstraintComponent ;
    rdfs:label "Min-count constraint component"@en ;
    rdfs:comment "A constraint component that can be used to restrict the minimum number of value nodes."@en ;
    rdfs:isDefinedBy sh: ;
    sh:parameter sh:MinCountConstraintComponent-minCount .

sh:MinExclusiveConstraintComponent a sh:ConstraintComponent ;
    rdfs:label "Min-exclusive constraint component"@en ;
    rdfs:comment "A constraint component that can be used to restrict the range of value nodes with a minimum exclusive value."@en ;
    rdfs:isDefinedBy sh: ;
    sh:parameter sh:MinExclusiveConstraintComponent-minExclusive .

sh:MinInclusiveConstraintComponent a sh:ConstraintComponent ;
    rdfs:label "Min-inclusive constraint component"@en ;
    rdfs:comment "A constraint component that can be used to restrict the range of value nodes with a minimum inclusive value."@en ;
    rdfs:isDefinedBy sh: ;
    sh:parameter sh:MinInclusiveConstraintComponent-minInclusive .

sh:MinLengthConstraintComponent a sh:ConstraintComponent ;
    rdfs:label "Min-length constraint component"@en ;
    rdfs:comment "A constraint component that can be used to restrict the minimum string length of value nodes."@en ;
    rdfs:isDefinedBy sh: ;
    sh:parameter sh:MinLengthConstraintComponent-minLength .

sh:NodeConstraintComponent a sh:ConstraintComponent ;
    rdfs:label "Node constraint component"@en ;
    rdfs:comment "A constraint component that can be used to verify that all value nodes conform to the given node shape."@en ;
    rdfs:isDefinedBy sh: ;
    sh:parameter sh:NodeConstraintComponent-node .

sh:NodeKindConstraintComponent a sh:ConstraintComponent ;
    rdfs:label "Node-kind constraint component"@en ;
    rdfs:comment "A constraint component that can be used to restrict the RDF node kind of each value node."@en ;
    rdfs:isDefinedBy sh: ;
    sh:parameter sh:NodeKindConstraintComponent-nodeKind .

sh:NotConstraintComponent a sh:ConstraintComponent ;
    rdfs:label "Not constraint component"@en ;
    rdfs:comment "A constraint component that can be used to verify that value nodes do not conform to a given shape."@en ;
    rdfs:isDefinedBy sh: ;
    sh:parameter sh:NotConstraintComponent-not .

sh:OrConstraintComponent a sh:ConstraintComponent ;
    rdfs:label "Or constraint component"@en ;
    rdfs:comment "A constraint component that can be used to restrict the value nodes so that they conform to at least one out of several provided shapes."@en ;
    rdfs:isDefinedBy sh: ;
    sh:parameter sh:OrConstraintComponent-or .

sh:PatternConstraintComponent a sh:ConstraintComponent ;
    rdfs:label "Pattern constraint component"@en ;
    rdfs:comment "A constraint component that can be used to verify that every value node matches a given regular expression."@en ;
    rdfs:isDefinedBy sh: ;
    sh:parameter sh:PatternConstraintComponent-flags,
        sh:PatternConstraintComponent-pattern .

sh:PropertyConstraintComponent a sh:ConstraintComponent ;
    rdfs:label "Property constraint component"@en ;
    rdfs:comment "A constraint component that can be used to verify that all value nodes conform to the given property shape."@en ;
    rdfs:isDefinedBy sh: ;
    sh:parameter sh:PropertyConstraintComponent-property .

sh:QualifiedMaxCountConstraintComponent a sh:ConstraintComponent ;
    rdfs:label "Qualified-max-count constraint component"@en ;
    rdfs:comment "A constraint component that can be used to verify that a specified maximum number of value nodes conforms to a given shape."@en ;
    rdfs:isDefinedBy sh: ;
    sh:parameter sh:QualifiedMaxCountConstraintComponent-qualifiedMaxCount,
        sh:QualifiedMaxCountConstraintComponent-qualifiedValueShape,
        sh:QualifiedMaxCountConstraintComponent-qualifiedValueShapesDisjoint .

sh:QualifiedMinCountConstraintComponent a sh:ConstraintComponent ;
    rdfs:label "Qualified-min-count constraint component"@en ;
    rdfs:comment "A constraint component that can be used to verify that a specified minimum number of value nodes conforms to a given shape."@en ;
    rdfs:isDefinedBy sh: ;
    sh:parameter sh:QualifiedMinCountConstraintComponent-qualifiedMinCount,
        sh:QualifiedMinCountConstraintComponent-qualifiedValueShape,
        sh:QualifiedMinCountConstraintComponent-qualifiedValueShapesDisjoint .

sh:SPARQLConstraintComponent a sh:ConstraintComponent ;
    rdfs:label "SPARQL constraint component"@en ;
    rdfs:comment "A constraint component that can be used to define constraints based on SPARQL queries."@en ;
    rdfs:isDefinedBy sh: ;
    sh:parameter sh:SPARQLConstraintComponent-sparql .

sh:UniqueLangConstraintComponent a sh:ConstraintComponent ;
    rdfs:label "Unique-languages constraint component"@en ;
    rdfs:comment "A constraint component that can be used to specify that no pair of value nodes may use the same language tag."@en ;
    rdfs:isDefinedBy sh: ;
    sh:parameter sh:UniqueLangConstraintComponent-uniqueLang .

sh:Violation a sh:Severity ;
    rdfs:label "Violation"@en ;
    rdfs:comment "The severity for a violation validation result."@en ;
    rdfs:isDefinedBy sh: .

sh:XoneConstraintComponent a sh:ConstraintComponent ;
    rdfs:label "Exactly one constraint component"@en ;
    rdfs:comment "A constraint component that can be used to restrict the value nodes so that they conform to exactly one out of several provided shapes."@en ;
    rdfs:isDefinedBy sh: ;
    sh:parameter sh:XoneConstraintComponent-xone .

sh:alternativePath a rdf:Property ;
    rdfs:label "alternative path"@en ;
    rdfs:comment "The (single) value of this property must be a list of path elements, representing the elements of alternative paths."@en ;
    rdfs:isDefinedBy sh: ;
    rdfs:range rdf:List .

sh:annotationProperty a rdf:Property ;
    rdfs:label "annotation property"@en ;
    rdfs:comment "The annotation property that shall be set."@en ;
    rdfs:domain sh:ResultAnnotation ;
    rdfs:isDefinedBy sh: ;
    rdfs:range rdf:Property .

sh:annotationValue a rdf:Property ;
    rdfs:label "annotation value"@en ;
    rdfs:comment "The (default) values of the annotation property."@en ;
    rdfs:domain sh:ResultAnnotation ;
    rdfs:isDefinedBy sh: .

sh:annotationVarName a rdf:Property ;
    rdfs:label "annotation variable name"@en ;
    rdfs:comment "The name of the SPARQL variable from the SELECT clause that shall be used for the values."@en ;
    rdfs:domain sh:ResultAnnotation ;
    rdfs:isDefinedBy sh: ;
    rdfs:range xsd:string .

sh:ask a rdf:Property ;
    rdfs:label "ask"@en ;
    rdfs:comment "The SPARQL ASK query to execute."@en ;
    rdfs:domain sh:SPARQLAskExecutable ;
    rdfs:isDefinedBy sh: ;
    rdfs:range xsd:string .

sh:condition a rdf:Property ;
    rdfs:label "condition"@en ;
    rdfs:comment "The shapes that the focus nodes need to conform to before a rule is executed on them."@en ;
    rdfs:domain sh:Rule ;
    rdfs:isDefinedBy sh: ;
    rdfs:range sh:Shape .

sh:conforms a rdf:Property ;
    rdfs:label "conforms"@en ;
    rdfs:comment "True if the validation did not produce any validation results, and false otherwise."@en ;
    rdfs:domain sh:ValidationReport ;
    rdfs:isDefinedBy sh: ;
    rdfs:range xsd:boolean .

sh:construct a rdf:Property ;
    rdfs:label "construct"@en ;
    rdfs:comment "The SPARQL CONSTRUCT query to execute."@en ;
    rdfs:domain sh:SPARQLConstructExecutable ;
    rdfs:isDefinedBy sh: ;
    rdfs:range xsd:string .

sh:deactivated a rdf:Property ;
    rdfs:label "deactivated"@en ;
    rdfs:comment "If set to true then all nodes conform to this."@en ;
    rdfs:isDefinedBy sh: ;
    rdfs:range xsd:boolean .

sh:declare a rdf:Property ;
    rdfs:label "declare"@en ;
    rdfs:comment "Links a resource with its namespace prefix declarations."@en ;
    rdfs:domain owl:Ontology ;
    rdfs:isDefinedBy sh: ;
    rdfs:range sh:PrefixDeclaration .

sh:defaultValue a rdf:Property ;
    rdfs:label "default value"@en ;
    rdfs:comment "A default value for a property, for example for user interface tools to pre-populate input fields."@en ;
    rdfs:domain sh:PropertyShape ;
    rdfs:isDefinedBy sh: .

sh:description a rdf:Property ;
    rdfs:label "description"@en ;
    rdfs:comment "Human-readable descriptions for the property in the context of the surrounding shape."@en ;
    rdfs:domain sh:PropertyShape ;
    rdfs:isDefinedBy sh: .

sh:detail a rdf:Property ;
    rdfs:label "detail"@en ;
    rdfs:comment "Links a result with other results that provide more details, for example to describe violations against nested shapes."@en ;
    rdfs:domain sh:AbstractResult ;
    rdfs:isDefinedBy sh: ;
    rdfs:range sh:AbstractResult .

sh:entailment a rdf:Property ;
    rdfs:label "entailment"@en ;
    rdfs:comment "An entailment regime that indicates what kind of inferencing is required by a shapes graph."@en ;
    rdfs:domain owl:Ontology ;
    rdfs:isDefinedBy sh: ;
    rdfs:range rdfs:Resource .

sh:filterShape a rdf:Property ;
    rdfs:label "filter shape"@en ;
    rdfs:comment "The shape that all input nodes of the expression need to conform to."@en ;
    rdfs:isDefinedBy sh: ;
    rdfs:range sh:Shape .

sh:focusNode a rdf:Property ;
    rdfs:label "focus node"@en ;
    rdfs:comment "The focus node that was validated when the result was produced."@en ;
    rdfs:domain sh:AbstractResult ;
    rdfs:isDefinedBy sh: .

sh:group a rdf:Property ;
    rdfs:label "group"@en ;
    rdfs:comment "Can be used to link to a property group to indicate that a property shape belongs to a group of related property shapes."@en ;
    rdfs:domain sh:PropertyShape ;
    rdfs:isDefinedBy sh: ;
    rdfs:range sh:PropertyGroup .

sh:intersection a rdf:Property ;
    rdfs:label "intersection"@en ;
    rdfs:comment "A list of node expressions that shall be intersected."@en ;
    rdfs:isDefinedBy sh: .

sh:inversePath a rdf:Property ;
    rdfs:label "inverse path"@en ;
    rdfs:comment "The (single) value of this property represents an inverse path (object to subject)."@en ;
    rdfs:isDefinedBy sh: ;
    rdfs:range rdfs:Resource .

sh:jsFunctionName a rdf:Property ;
    rdfs:label "JavaScript function name"@en ;
    rdfs:comment "The name of the JavaScript function to execute."@en ;
    rdfs:domain sh:JSExecutable ;
    rdfs:isDefinedBy sh: ;
    rdfs:range xsd:string .

sh:jsLibrary a rdf:Property ;
    rdfs:label "JavaScript library"@en ;
    rdfs:comment "Declares which JavaScript libraries are needed to execute this."@en ;
    rdfs:isDefinedBy sh: ;
    rdfs:range sh:JSLibrary .

sh:jsLibraryURL a rdf:Property ;
    rdfs:label "JavaScript library URL"@en ;
    rdfs:comment "Declares the URLs of a JavaScript library. This should be the absolute URL of a JavaScript file. Implementations may redirect those to local files."@en ;
    rdfs:domain sh:JSLibrary ;
    rdfs:isDefinedBy sh: ;
    rdfs:range xsd:anyURI .

sh:labelTemplate a rdf:Property ;
    rdfs:label "label template"@en ;
    rdfs:comment "Outlines how human-readable labels of instances of the associated Parameterizable shall be produced. The values can contain {?paramName} as placeholders for the actual values of the given parameter."@en ;
    rdfs:domain sh:Parameterizable ;
    rdfs:isDefinedBy sh: .

sh:message a rdf:Property ;
    rdfs:label "message"@en ;
    rdfs:comment "A human-readable message (possibly with placeholders for variables) explaining the cause of the result."@en ;
    rdfs:isDefinedBy sh: .

sh:name a rdf:Property ;
    rdfs:label "name"@en ;
    rdfs:comment "Human-readable labels for the property in the context of the surrounding shape."@en ;
    rdfs:domain sh:PropertyShape ;
    rdfs:isDefinedBy sh: .

sh:namespace a rdf:Property ;
    rdfs:label "namespace"@en ;
    rdfs:comment "The namespace associated with a prefix in a prefix declaration."@en ;
    rdfs:domain sh:PrefixDeclaration ;
    rdfs:isDefinedBy sh: ;
    rdfs:range xsd:anyURI .

sh:nodeValidator a rdf:Property ;
    rdfs:label "shape validator"@en ;
    rdfs:comment "The validator(s) used to evaluate a constraint in the context of a node shape."@en ;
    rdfs:domain sh:ConstraintComponent ;
    rdfs:isDefinedBy sh: ;
    rdfs:range sh:Validator .

sh:nodes a rdf:Property ;
    rdfs:label "nodes"@en ;
    rdfs:comment "The node expression producing the input nodes of a filter shape expression."@en ;
    rdfs:isDefinedBy sh: .

sh:object a rdf:Property ;
    rdfs:label "object"@en ;
    rdfs:comment "An expression producing the nodes that shall be inferred as objects."@en ;
    rdfs:domain sh:TripleRule ;
    rdfs:isDefinedBy sh: .

sh:oneOrMorePath a rdf:Property ;
    rdfs:label "one or more path"@en ;
    rdfs:comment "The (single) value of this property represents a path that is matched one or more times."@en ;
    rdfs:isDefinedBy sh: ;
    rdfs:range rdfs:Resource .

sh:optional a rdf:Property ;
    rdfs:label "optional"@en ;
    rdfs:comment "Indicates whether a parameter is optional."@en ;
    rdfs:domain sh:Parameter ;
    rdfs:isDefinedBy sh: ;
    rdfs:range xsd:boolean .

sh:order a rdf:Property ;
    rdfs:label "order"@en ;
    rdfs:comment "Specifies the relative order of this compared to its siblings. For example use 0 for the first, 1 for the second."@en ;
    rdfs:isDefinedBy sh: .

sh:parameter a rdf:Property ;
    rdfs:label "parameter"@en ;
    rdfs:comment "The parameters of a function or constraint component."@en ;
    rdfs:domain sh:Parameterizable ;
    rdfs:isDefinedBy sh: ;
    rdfs:range sh:Parameter .

sh:path a rdf:Property ;
    rdfs:label "path"@en ;
    rdfs:comment "Specifies the property path of a property shape."@en ;
    rdfs:domain sh:PropertyShape ;
    rdfs:isDefinedBy sh: ;
    rdfs:range rdfs:Resource .

sh:predicate a rdf:Property ;
    rdfs:label "predicate"@en ;
    rdfs:comment "An expression producing the properties that shall be inferred as predicates."@en ;
    rdfs:domain sh:TripleRule ;
    rdfs:isDefinedBy sh: .

sh:prefix a rdf:Property ;
    rdfs:label "prefix"@en ;
    rdfs:comment "The prefix of a prefix declaration."@en ;
    rdfs:domain sh:PrefixDeclaration ;
    rdfs:isDefinedBy sh: ;
    rdfs:range xsd:string .

sh:prefixes a rdf:Property ;
    rdfs:label "prefixes"@en ;
    rdfs:comment "The prefixes that shall be applied before parsing the associated SPARQL query."@en ;
    rdfs:domain sh:SPARQLExecutable ;
    rdfs:isDefinedBy sh: ;
    rdfs:range owl:Ontology .

sh:propertyValidator a rdf:Property ;
    rdfs:label "property validator"@en ;
    rdfs:comment "The validator(s) used to evaluate a constraint in the context of a property shape."@en ;
    rdfs:domain sh:ConstraintComponent ;
    rdfs:isDefinedBy sh: ;
    rdfs:range sh:Validator .

sh:result a rdf:Property ;
    rdfs:label "result"@en ;
    rdfs:comment "The validation results contained in a validation report."@en ;
    rdfs:domain sh:ValidationReport ;
    rdfs:isDefinedBy sh: ;
    rdfs:range sh:ValidationResult .

sh:resultAnnotation a rdf:Property ;
    rdfs:label "result annotation"@en ;
    rdfs:comment "Links a SPARQL validator with zero or more sh:ResultAnnotation instances, defining how to derive additional result properties based on the variables of the SELECT query."@en ;
    rdfs:domain sh:SPARQLSelectValidator ;
    rdfs:isDefinedBy sh: ;
    rdfs:range sh:ResultAnnotation .

sh:resultMessage a rdf:Property ;
    rdfs:label "result message"@en ;
    rdfs:comment "Human-readable messages explaining the cause of the result."@en ;
    rdfs:domain sh:AbstractResult ;
    rdfs:isDefinedBy sh: .

sh:resultPath a rdf:Property ;
    rdfs:label "result path"@en ;
    rdfs:comment "The path of a validation result, based on the path of the validated property shape."@en ;
    rdfs:domain sh:AbstractResult ;
    rdfs:isDefinedBy sh: ;
    rdfs:range rdfs:Resource .

sh:resultSeverity a rdf:Property ;
    rdfs:label "result severity"@en ;
    rdfs:comment "The severity of the result, e.g. warning."@en ;
    rdfs:domain sh:AbstractResult ;
    rdfs:isDefinedBy sh: ;
    rdfs:range sh:Severity .

sh:returnType a rdf:Property ;
    rdfs:label "return type"@en ;
    rdfs:comment "The expected type of values returned by the associated function."@en ;
    rdfs:domain sh:Function ;
    rdfs:isDefinedBy sh: ;
    rdfs:range rdfs:Class .

sh:rule a rdf:Property ;
    rdfs:label "rule"@en ;
    rdfs:comment "The rules linked to a shape."@en ;
    rdfs:domain sh:Shape ;
    rdfs:isDefinedBy sh: ;
    rdfs:range sh:Rule .

sh:select a rdf:Property ;
    rdfs:label "select"@en ;
    rdfs:comment "The SPARQL SELECT query to execute."@en ;
    rdfs:domain sh:SPARQLSelectExecutable ;
    rdfs:isDefinedBy sh: ;
    rdfs:range xsd:string .

sh:severity a rdf:Property ;
    rdfs:label "severity"@en ;
    rdfs:comment "Defines the severity that validation results produced by a shape must have. Defaults to sh:Violation."@en ;
    rdfs:domain sh:Shape ;
    rdfs:isDefinedBy sh: ;
    rdfs:range sh:Severity .

sh:shapesGraph a rdf:Property ;
    rdfs:label "shapes graph"@en ;
    rdfs:comment "Shapes graphs that should be used when validating this data graph."@en ;
    rdfs:domain owl:Ontology ;
    rdfs:isDefinedBy sh: ;
    rdfs:range owl:Ontology .

sh:shapesGraphWellFormed a rdf:Property ;
    rdfs:label "shapes graph well-formed"@en ;
    rdfs:comment "If true then the validation engine was certain that the shapes graph has passed all SHACL syntax requirements during the validation process."@en ;
    rdfs:domain sh:ValidationReport ;
    rdfs:isDefinedBy sh: ;
    rdfs:range xsd:boolean .

sh:sourceConstraint a rdf:Property ;
    rdfs:label "source constraint"@en ;
    rdfs:comment "The constraint that was validated when the result was produced."@en ;
    rdfs:domain sh:AbstractResult ;
    rdfs:isDefinedBy sh: .

sh:sourceConstraintComponent a rdf:Property ;
    rdfs:label "source constraint component"@en ;
    rdfs:comment "The constraint component that is the source of the result."@en ;
    rdfs:domain sh:AbstractResult ;
    rdfs:isDefinedBy sh: ;
    rdfs:range sh:ConstraintComponent .

sh:sourceShape a rdf:Property ;
    rdfs:label "source shape"@en ;
    rdfs:comment "The shape that is was validated when the result was produced."@en ;
    rdfs:domain sh:AbstractResult ;
    rdfs:isDefinedBy sh: ;
    rdfs:range sh:Shape .

sh:subject a rdf:Property ;
    rdfs:label "subject"@en ;
    rdfs:comment "An expression producing the resources that shall be inferred as subjects."@en ;
    rdfs:domain sh:TripleRule ;
    rdfs:isDefinedBy sh: .

sh:suggestedShapesGraph a rdf:Property ;
    rdfs:label "suggested shapes graph"@en ;
    rdfs:comment "Suggested shapes graphs for this ontology. The values of this property may be used in the absence of specific sh:shapesGraph statements."@en ;
    rdfs:domain owl:Ontology ;
    rdfs:isDefinedBy sh: ;
    rdfs:range owl:Ontology .

sh:target a rdf:Property ;
    rdfs:label "target"@en ;
    rdfs:comment "Links a shape to a target specified by an extension language, for example instances of sh:SPARQLTarget."@en ;
    rdfs:domain sh:Shape ;
    rdfs:isDefinedBy sh: ;
    rdfs:range sh:Target .

sh:targetClass a rdf:Property ;
    rdfs:label "target class"@en ;
    rdfs:comment "Links a shape to a class, indicating that all instances of the class must conform to the shape."@en ;
    rdfs:domain sh:Shape ;
    rdfs:isDefinedBy sh: ;
    rdfs:range rdfs:Class .

sh:targetNode a rdf:Property ;
    rdfs:label "target node"@en ;
    rdfs:comment "Links a shape to individual nodes, indicating that these nodes must conform to the shape."@en ;
    rdfs:domain sh:Shape ;
    rdfs:isDefinedBy sh: .

sh:targetObjectsOf a rdf:Property ;
    rdfs:label "target objects of"@en ;
    rdfs:comment "Links a shape to a property, indicating that all all objects of triples that have the given property as their predicate must conform to the shape."@en ;
    rdfs:domain sh:Shape ;
    rdfs:isDefinedBy sh: ;
    rdfs:range rdf:Property .

sh:targetSubjectsOf a rdf:Property ;
    rdfs:label "target subjects of"@en ;
    rdfs:comment "Links a shape to a property, indicating that all subjects of triples that have the given property as their predicate must conform to the shape."@en ;
    rdfs:domain sh:Shape ;
    rdfs:isDefinedBy sh: ;
    rdfs:range rdf:Property .

sh:union a rdf:Property ;
    rdfs:label "union"@en ;
    rdfs:comment "A list of node expressions that shall be used together."@en ;
    rdfs:isDefinedBy sh: .

sh:update a rdf:Property ;
    rdfs:label "update"@en ;
    rdfs:comment "The SPARQL UPDATE to execute."@en ;
    rdfs:domain sh:SPARQLUpdateExecutable ;
    rdfs:isDefinedBy sh: ;
    rdfs:range xsd:string .

sh:validator a rdf:Property ;
    rdfs:label "validator"@en ;
    rdfs:comment "The validator(s) used to evaluate constraints of either node or property shapes."@en ;
    rdfs:domain sh:ConstraintComponent ;
    rdfs:isDefinedBy sh: ;
    rdfs:range sh:Validator .

sh:value a rdf:Property ;
    rdfs:label "value"@en ;
    rdfs:comment "An RDF node that has caused the result."@en ;
    rdfs:domain sh:AbstractResult ;
    rdfs:isDefinedBy sh: .

sh:zeroOrMorePath a rdf:Property ;
    rdfs:label "zero or more path"@en ;
    rdfs:comment "The (single) value of this property represents a path that is matched zero or more times."@en ;
    rdfs:isDefinedBy sh: ;
    rdfs:range rdfs:Resource .

sh:zeroOrOnePath a rdf:Property ;
    rdfs:label "zero or one path"@en ;
    rdfs:comment "The (single) value of this property represents a path that is matched zero or one times."@en ;
    rdfs:isDefinedBy sh: ;
    rdfs:range rdfs:Resource .

s223:AirHandlingUnit a s223:Class,
        sh:NodeShape ;
    rdfs:label "Air handling unit" ;
    rdfs:comment "An assembly consisting of sections containing a fan or fans and other necessary equipment to perform one or more of the following functions: circulating, filtration, heating, cooling, heat recovery, humidifying, dehumidifying, and mixing of air. It is usually connected to an air-distribution system." ;
    rdfs:subClassOf s223:Equipment ;
    sh:property [ rdfs:comment "An AirHandlingUnit shall have at least one inlet using the medium Air." ;
            sh:minCount 2 ;
            sh:path s223:hasConnectionPoint ;
            sh:qualifiedMinCount 1 ;
            sh:qualifiedValueShape [ sh:class s223:InletConnectionPoint ;
                    sh:node [ sh:property [ sh:class s223:Medium-Air ;
                                    sh:path s223:hasMedium ] ] ] ],
        [ rdfs:comment "An AirHandlingUnit shall have at least one outlet using the medium Air." ;
            sh:path s223:hasConnectionPoint ;
            sh:qualifiedMinCount 1 ;
            sh:qualifiedValueShape [ sh:class s223:OutletConnectionPoint ;
                    sh:node [ sh:property [ sh:class s223:Medium-Air ;
                                    sh:path s223:hasMedium ] ] ] ] .

s223:Constant a s223:Class,
        sh:NodeShape ;
    rdfs:label "Constant" ;
    rdfs:comment "A constant is a parameter with constant value, used by the function block to produce one or more output (ex. pi)." ;
    rdfs:subClassOf s223:Concept,
        s223:Parameter ;
    sh:property [ rdfs:comment "An instance of Constant can be associated with any number of Property instances using the relation 'uses'." ;
            sh:class s223:Property ;
            sh:path s223:uses ] .

s223:CoolingCoil a s223:Class,
        sh:NodeShape ;
    rdfs:label "Cooling coil" ;
    rdfs:subClassOf s223:Coil ;
    sh:property [ rdfs:comment "A cooling coil must be related to the role 'Role-Cooling' using the relation 'hasRole'." ;
            sh:hasValue s223:Role-Cooling ;
            sh:minCount 1 ;
            sh:path s223:hasRole ] ;
    sh:rule [ a sh:TripleRule ;
            rdfs:comment "Cooling coils will always have the role Role-Cooling" ;
            sh:object s223:Role-Cooling ;
            sh:predicate s223:hasRole ;
            sh:subject sh:this ] .

s223:ElectricalPhaseIdentifier-A a s223:Attribute-ElectricalPhaseIdentifier ;
    rdfs:label "Electrical Phase Identifier A" ;
    rdfs:comment "The value of the associated Property identifies the electrical phase A of the Connection." .

s223:ElectricalPhaseIdentifier-B a s223:Attribute-ElectricalPhaseIdentifier ;
    rdfs:label "Electrical Phase Identifier B" ;
    rdfs:comment "The value of the associated Property identifies the electrical phase B of the Connection." .

s223:ElectricalPhaseIdentifier-BC a s223:Attribute-ElectricalPhaseIdentifier ;
    rdfs:label "Electrical Phase Identifier BC" ;
    rdfs:comment "The value of the associated Property identifies the electrical phase BC of the Connection." .

s223:HeatExchanger a s223:Class,
        sh:NodeShape ;
    rdfs:label "Heat exchanger" ;
    rdfs:comment "A component intended to transfer heat from one medium to another while keeping the two media separate" ;
    rdfs:subClassOf s223:Equipment ;
    sh:property [ rdfs:comment "A HeatExchanger shall have at least two inlets." ;
            sh:path s223:hasConnectionPoint ;
            sh:qualifiedMinCount 2 ;
            sh:qualifiedValueShape [ sh:class s223:InletConnectionPoint ] ],
        [ rdfs:comment "A HeatExchanger shall have at least two outlets." ;
            sh:path s223:hasConnectionPoint ;
            sh:qualifiedMinCount 2 ;
            sh:qualifiedValueShape [ sh:class s223:OutletConnectionPoint ] ],
        [ sh:minCount 4 ;
            sh:path s223:hasConnectionPoint ],
        [ rdfs:comment "A HeatExchanger can be associated with an EnumerationKind-Role using the relation hasRole" ;
            sh:class s223:EnumerationKind-Role ;
            sh:path s223:hasRole ] .

s223:IlluminanceSensor a s223:Class,
        sh:NodeShape ;
    rdfs:label "Illuminance sensor" ;
    rdfs:subClassOf s223:LightSensor ;
    sh:property [ rdfs:comment "A IlluminanceSensor will always observe a Property that has a QuantityKind of Illuminance." ;
            sh:path s223:observes ;
            sh:qualifiedMinCount 1 ;
            sh:qualifiedValueShape [ sh:class s223:Property ;
                    sh:node [ sh:property [ sh:hasValue quantitykind:Illuminance ;
                                    sh:path qudt:hasQuantityKind ] ] ] ] .

s223:OccupantCounter a s223:Class,
        sh:NodeShape ;
    rdfs:label "Occupant counter" ;
    rdfs:subClassOf s223:OccupancySensor ;
    sh:property [ rdfs:comment "A OccupantCounter will always observe a Property that has a QuantityKind of Population." ;
            sh:path s223:observes ;
            sh:qualifiedMinCount 1 ;
            sh:qualifiedValueShape [ sh:class s223:Property ;
                    sh:node [ sh:property [ sh:hasValue quantitykind:Population ;
                                    sh:path qudt:hasQuantityKind ] ] ] ] .

s223:Role-Exhaust a s223:EnumerationKind-Role ;
    rdfs:label "Role-Exhaust" .

s223:Role-Return a s223:EnumerationKind-Role ;
    rdfs:label "Role-Return" .

s223:Role-Supply a s223:EnumerationKind-Role ;
    rdfs:label "Role-Supply" .

s223:Setpoint a s223:Class,
        sh:NodeShape ;
    rdfs:label "Setpoint" ;
    rdfs:subClassOf s223:Property,
        qudt:Quantity ;
    sh:property [ rdfs:comment "A Setpoint can be associated with a decimal value using the relation hasDeadband" ;
            sh:datatype xsd:decimal ;
            sh:path s223:hasDeadband ],
        [ rdfs:comment "A Setpoint can be assicated with a decimal value using the relation hasValue" ;
            sh:datatype xsd:decimal ;
            sh:path s223:hasValue ] ;
    sh:rule [ a sh:SPARQLRule ;
            rdfs:comment "Infer the hasQuantityKind relationship for a Setpoint if it is unambiguous" ;
            sh:construct """
CONSTRUCT {$this qudt:hasQuantityKind ?qk .}
WHERE {
FILTER (NOT EXISTS {$this qudt:hasQuantityKind ?something}) .
$this ^s223:hasSetpoint ?property .
?property qudt:hasQuantityKind ?qk .
}
""" ;
            sh:prefixes s223: ] .

s223:Voltage-1.73kV a s223:Dimensioned-Voltage,
        s223:QuantifiableProperty ;
    rdfs:label "1.73kV Voltage" ;
    s223:hasValue 1.73 ;
    qudt:hasQuantityKind quantitykind:Voltage ;
    qudt:hasUnit unit:KiloV .

s223:Voltage-1.91kV a s223:Dimensioned-Voltage,
        s223:QuantifiableProperty ;
    rdfs:label "1.91kV Voltage" ;
    s223:hasValue 1.91 ;
    qudt:hasQuantityKind quantitykind:Voltage ;
    qudt:hasUnit unit:KiloV .

s223:Voltage-10.0kV a s223:Dimensioned-Voltage,
        s223:QuantifiableProperty ;
    rdfs:label "10.0kV Voltage" ;
    s223:hasValue 10.0 ;
    qudt:hasQuantityKind quantitykind:Voltage ;
    qudt:hasUnit unit:KiloV .

s223:Voltage-110.0V a s223:Dimensioned-Voltage,
        s223:QuantifiableProperty ;
    rdfs:label "110.0V Voltage" ;
    s223:hasValue 110.0 ;
    qudt:hasQuantityKind quantitykind:Voltage ;
    qudt:hasUnit unit:V .

s223:Voltage-120.0V a s223:Dimensioned-Voltage,
        s223:QuantifiableProperty ;
    rdfs:label "120.0V Voltage" ;
    s223:hasValue 120.0 ;
    qudt:hasQuantityKind quantitykind:Voltage ;
    qudt:hasUnit unit:V .

s223:Voltage-127.0V a s223:Dimensioned-Voltage,
        s223:QuantifiableProperty ;
    rdfs:label "127.0V Voltage" ;
    s223:hasValue 127.0 ;
    qudt:hasQuantityKind quantitykind:Voltage ;
    qudt:hasUnit unit:V .

s223:Voltage-139.0V a s223:Dimensioned-Voltage,
        s223:QuantifiableProperty ;
    rdfs:label "139.0V Voltage" ;
    s223:hasValue 139.0 ;
    qudt:hasQuantityKind quantitykind:Voltage ;
    qudt:hasUnit unit:V .

s223:Voltage-190.0V a s223:Dimensioned-Voltage,
        s223:QuantifiableProperty ;
    rdfs:label "190.0V Voltage" ;
    s223:hasValue 190.0 ;
    qudt:hasQuantityKind quantitykind:Voltage ;
    qudt:hasUnit unit:V .

s223:Voltage-2.4kV a s223:Dimensioned-Voltage,
        s223:QuantifiableProperty ;
    rdfs:label "2.4kV Voltage" ;
    s223:hasValue 2.4 ;
    qudt:hasQuantityKind quantitykind:Voltage ;
    qudt:hasUnit unit:KiloV .

s223:Voltage-219.0V a s223:Dimensioned-Voltage,
        s223:QuantifiableProperty ;
    rdfs:label "219.0V Voltage" ;
    s223:hasValue 219.0 ;
    qudt:hasQuantityKind quantitykind:Voltage ;
    qudt:hasUnit unit:V .

s223:Voltage-220.0V a s223:Dimensioned-Voltage,
        s223:QuantifiableProperty ;
    rdfs:label "220.0V Voltage" ;
    s223:hasValue 220.0 ;
    qudt:hasQuantityKind quantitykind:Voltage ;
    qudt:hasUnit unit:V .

s223:Voltage-231.0V a s223:Dimensioned-Voltage,
        s223:QuantifiableProperty ;
    rdfs:label "231.0V Voltage" ;
    s223:hasValue 231.0 ;
    qudt:hasQuantityKind quantitykind:Voltage ;
    qudt:hasUnit unit:V .

s223:Voltage-277.0V a s223:Dimensioned-Voltage,
        s223:QuantifiableProperty ;
    rdfs:label "277.0V Voltage" ;
    s223:hasValue 277.0 ;
    qudt:hasQuantityKind quantitykind:Voltage ;
    qudt:hasUnit unit:V .

s223:Voltage-3.0kV a s223:Dimensioned-Voltage,
        s223:QuantifiableProperty ;
    rdfs:label "3.0kV Voltage" ;
    s223:hasValue 3.0 ;
    qudt:hasQuantityKind quantitykind:Voltage ;
    qudt:hasUnit unit:KiloV .

s223:Voltage-3.3kV a s223:Dimensioned-Voltage,
        s223:QuantifiableProperty ;
    rdfs:label "3.3kV Voltage" ;
    s223:hasValue 3.3 ;
    qudt:hasQuantityKind quantitykind:Voltage ;
    qudt:hasUnit unit:KiloV .

s223:Voltage-3.46kV a s223:Dimensioned-Voltage,
        s223:QuantifiableProperty ;
    rdfs:label "3.46kV Voltage" ;
    s223:hasValue 3.46 ;
    qudt:hasQuantityKind quantitykind:Voltage ;
    qudt:hasUnit unit:KiloV .

s223:Voltage-3.81kV a s223:Dimensioned-Voltage,
        s223:QuantifiableProperty ;
    rdfs:label "3.81kV Voltage" ;
    s223:hasValue 3.81 ;
    qudt:hasQuantityKind quantitykind:Voltage ;
    qudt:hasUnit unit:KiloV .

s223:Voltage-347.0V a s223:Dimensioned-Voltage,
        s223:QuantifiableProperty ;
    rdfs:label "347.0V Voltage" ;
    s223:hasValue 347.0 ;
    qudt:hasQuantityKind quantitykind:Voltage ;
    qudt:hasUnit unit:V .

s223:Voltage-380.0V a s223:Dimensioned-Voltage,
        s223:QuantifiableProperty ;
    rdfs:label "380.0V Voltage" ;
    s223:hasValue 380.0 ;
    qudt:hasQuantityKind quantitykind:Voltage ;
    qudt:hasUnit unit:V .

s223:Voltage-4.16kV a s223:Dimensioned-Voltage,
        s223:QuantifiableProperty ;
    rdfs:label "4.16kV Voltage" ;
    s223:hasValue 4.16 ;
    qudt:hasQuantityKind quantitykind:Voltage ;
    qudt:hasUnit unit:KiloV .

s223:Voltage-400.0V a s223:Dimensioned-Voltage,
        s223:QuantifiableProperty ;
    rdfs:label "400.0V Voltage" ;
    s223:hasValue 400.0 ;
    qudt:hasQuantityKind quantitykind:Voltage ;
    qudt:hasUnit unit:V .

s223:Voltage-415.0V a s223:Dimensioned-Voltage,
        s223:QuantifiableProperty ;
    rdfs:label "415.0V Voltage" ;
    s223:hasValue 415.0 ;
    qudt:hasQuantityKind quantitykind:Voltage ;
    qudt:hasUnit unit:V .

s223:Voltage-480.0V a s223:Dimensioned-Voltage,
        s223:QuantifiableProperty ;
    rdfs:label "480.0V Voltage" ;
    s223:hasValue 480.0 ;
    qudt:hasQuantityKind quantitykind:Voltage ;
    qudt:hasUnit unit:V .

s223:Voltage-5.77kV a s223:Dimensioned-Voltage,
        s223:QuantifiableProperty ;
    rdfs:label "5.77kV Voltage" ;
    s223:hasValue 5.77 ;
    qudt:hasQuantityKind quantitykind:Voltage ;
    qudt:hasUnit unit:KiloV .

s223:Voltage-6.0kV a s223:Dimensioned-Voltage,
        s223:QuantifiableProperty ;
    rdfs:label "6.0kV Voltage" ;
    s223:hasValue 6.0 ;
    qudt:hasQuantityKind quantitykind:Voltage ;
    qudt:hasUnit unit:KiloV .

s223:Voltage-6.6kV a s223:Dimensioned-Voltage,
        s223:QuantifiableProperty ;
    rdfs:label "6.6kV Voltage" ;
    s223:hasValue 6.6 ;
    qudt:hasQuantityKind quantitykind:Voltage ;
    qudt:hasUnit unit:KiloV .

s223:Voltage-600.0V a s223:Dimensioned-Voltage,
        s223:QuantifiableProperty ;
    rdfs:label "600.0V Voltage" ;
    s223:hasValue 600.0 ;
    qudt:hasQuantityKind quantitykind:Voltage ;
    qudt:hasUnit unit:V .

s223:actuates a rdf:Property ;
    rdfs:label "actuates" ;
    rdfs:comment "The relation actuates binds an Actuator to the Equipment that it actuates. The Equipment will have the ActuatableProperty that commands the actuator (see `s223:commandedByProperty`)." .

s223:connectsFrom a rdf:Property ;
    rdfs:label "connects from" ;
    rdfs:comment "The relation connectsFrom binds a Connectable thing to a Connection with an implied directionality. B connectsFrom A indicates a flow from A to B." .

s223:connectsTo a rdf:Property ;
    rdfs:label "connects to" ;
    rdfs:comment "The connectsTo relation binds a specific ConnectionPoint to a Connection; See Figure x.y. The relation connectsTo binds a Connectable thing to a Connection with an implied directionality. A connectsTo B indicates a flow from A to B." .

s223:executes a rdf:Property ;
    rdfs:label "executes" ;
    rdfs:comment "The relation executes is used to specify that a controller (see `s223:Controller`) is responsible for the execution of a function block (see `s223:FunctionBlock`). " .

s223:hasAspect a rdf:Property ;
    rdfs:label "has aspect" ;
    rdfs:comment "hasAspect is used to establish the context of a Property. The value must be an instance of EnumerationKind. For example, if a Property has a Temperature value of 45.3, the hasAspect relation is used to state what that represents, such as a Temperature limit during working hours, etc. A Property can have any number of hasAspect relations, as needed to establish the context." .

s223:hasConstant a rdf:Property ;
    rdfs:label "has constant" ;
    rdfs:comment "The relation hasConstant is used to relate a constant (see `s223:Constant`) to a function block (see `s223:FunctionBlock`)." .

s223:hasDeadband a rdf:Property ;
    rdfs:label "has deadband" .

s223:hasMeasurementResolution a rdf:Property ;
    rdfs:label "has measurement resolution" ;
    rdfs:comment "The hasMeasurementResolution relation is used to link to a numerical property whose value indicates the smallest recognizable change in engineering units that the sensor can indicate. " .

s223:hasMember a rdf:Property ;
    rdfs:label "has member" .

s223:hasPhase a rdf:Property ;
    rdfs:label "has phase" ;
    rdfs:comment "The relation hasPhase is used to indicate the intended phase of the Medium inside a Connection." .

s223:hasPhysicalLocation a rdf:Property ;
    rdfs:label "has Physical Location" ;
    rdfs:comment "The relation hasPhysicalLocation is used to indicate the physical space (see `s223:PhysicalSpace`) where a piece of equipment (see `s223:Equipment`) is located." .

s223:hasSetpoint a rdf:Property ;
    rdfs:label "has setpoint" ;
    rdfs:comment "This relation binds a control setpoint to the quantifiable property indicating the desired value which the control process is trying to maintain." .

s223:ofMedium a rdf:Property ;
    rdfs:label "of medium" .

s223:produces a rdf:Property ;
    rdfs:label "produces" ;
    rdfs:comment "The relation produces is used to relate a function output (see `s223:FunctionOutput`) to a property (see `s223:Property`). This allows one to specify that the value of this property is produced by the function block output, allowing the users of the model to understand that the value of the property is the result of the algorithm defined by the function block. " .

s223:scp a rdf:Property .

psm:BR1InletConnectionPoint a s223:InletConnectionPoint ;
    rdfs:label "BR1Inlet connection point" ;
    s223:cnx psm:MainBreakerCircuit1 ;
    s223:hasMedium s223:AC-120V-60Hz .

psm:BR1OutletConnectionPoint a s223:OutletConnectionPoint ;
    rdfs:label "BR1Outlet connection point" ;
    s223:cnx psm:ElectricCircuit1 ;
    s223:hasMedium s223:AC-120V-60Hz .

psm:BR2InletConnectionPoint a s223:InletConnectionPoint ;
    rdfs:label "BR2Inlet connection point" ;
    s223:cnx psm:MainBreakerCircuit2 ;
    s223:hasMedium s223:AC-120V-60Hz .

psm:BR2OutletConnectionPoint a s223:OutletConnectionPoint ;
    rdfs:label "BR2Outlet connection point" ;
    s223:cnx psm:ElectricCircuit2 ;
    s223:hasMedium s223:AC-120V-60Hz .

psm:BR3OutletConnectionPoint a s223:OutletConnectionPoint ;
    rdfs:label "BR3Outlet connection point" ;
    s223:cnx psm:ElectricCircuit3 ;
    s223:hasMedium s223:AC-240V-60Hz .

psm:BR4InletConnectionPoint a s223:InletConnectionPoint ;
    rdfs:label "BR4Inlet connection point" ;
    s223:hasMedium s223:AC-120V-60Hz .

psm:BR4OutletConnectionPoint a s223:OutletConnectionPoint ;
    rdfs:label "BR4Outlet connection point" ;
    s223:hasMedium s223:AC-120V-60Hz .

psm:BR5InletConnectionPoint a s223:InletConnectionPoint ;
    rdfs:label "BR5Inlet connection point" ;
    s223:hasMedium s223:AC-120V-60Hz .

psm:BR5OutletConnectionPoint a s223:OutletConnectionPoint ;
    rdfs:label "BR5Outlet connection point" ;
    s223:hasMedium s223:AC-120V-60Hz .

psm:BathroomExhaustDuct a s223:Connection ;
    rdfs:label "Bathroom exhaust duct" ;
    s223:cnx psm:BathroomOutletConnectionPoint ;
    s223:hasMedium s223:Medium-Air .

psm:BreakerCP1Phase a s223:EnumerableProperty ;
    rdfs:label "BreakerCP1Phase" ;
    s223:hasEnumerationKind s223:Attribute-ElectricalPhaseIdentifier ;
    s223:hasValue s223:ElectricalPhaseIdentifier-A .

psm:BreakerCP2Phase a s223:EnumerableProperty ;
    rdfs:label "Breaker CP2Phase" ;
    s223:hasEnumerationKind s223:Attribute-ElectricalPhaseIdentifier ;
    s223:hasValue s223:ElectricalPhaseIdentifier-B .

psm:BreakerCP3Phase a s223:EnumerableProperty ;
    rdfs:label "Breaker CP3Phase" ;
    s223:hasEnumerationKind s223:Attribute-ElectricalPhaseIdentifier ;
    s223:hasValue s223:ElectricalPhaseIdentifier-BC .

psm:CoolingCoilOutletTemperature a s223:QuantifiableObservableProperty ;
    rdfs:label "Cooling coil outlet temperature" ;
    s223:hasValue 65.0 ;
    qudt:hasQuantityKind quantitykind:Temperature ;
    qudt:unit unit:DEG_F .

psm:CoolingCoilValvePosition a s223:QuantifiableActuatableProperty ;
    rdfs:label "Cooling coil valve position" ;
    s223:hasValue 50.0 ;
    qudt:hasQuantityKind quantitykind:Dimensionless ;
    qudt:unit unit:PERCENT .

psm:CorridorLightInletCP a s223:InletConnectionPoint ;
    rdfs:label "Corridor light inlet CP" ;
    s223:cnx psm:CorridorLight1 ;
    s223:hasMedium s223:Light-Visible .

psm:DLightPath1 a s223:Connection ;
    rdfs:label "DLight Path1" ;
    s223:hasMedium s223:Light-Visible .

psm:Driver1 a s223:Actuator ;
    rdfs:label "Driver1" ;
    s223:actuates psm:LightEngine1 ;
    s223:cnx psm:Driver1Inlet,
        psm:Driver1Outlet ;
    s223:commandedByProperty psm:Luminaire1CCT,
        psm:Luminaire1Intensity,
        psm:Luminaire1OnOff .

psm:Driver1Inlet a s223:InletConnectionPoint ;
    rdfs:label "Driver1Inlet" ;
    s223:cnx psm:ElectricCircuit1 ;
    s223:hasMedium s223:AC-120V-60Hz ;
    s223:mapsTo psm:Luminaire1Inlet .

psm:Driver1Outlet a s223:OutletConnectionPoint ;
    rdfs:label "Driver1Outlet" ;
    s223:cnx psm:Luminaire1InternalWire ;
    s223:hasMedium s223:Medium-Electricity .

psm:ElectricBreaker1 a s223:ElectricBreaker ;
    rdfs:label "Electric breaker1" ;
    s223:hasConnectionPoint psm:BR1InletConnectionPoint,
        psm:BR1OutletConnectionPoint .

psm:ElectricBreaker2 a s223:ElectricBreaker ;
    rdfs:label "Electric breaker2" ;
    s223:hasConnectionPoint psm:BR2InletConnectionPoint,
        psm:BR2OutletConnectionPoint .

psm:ElectricBreaker3 a s223:ElectricBreaker ;
    rdfs:label "Electric breaker3" ;
    s223:hasConnectionPoint psm:BR3InletConnectionPoint,
        psm:BR3OutletConnectionPoint .

psm:ElectricBreaker4 a s223:ElectricBreaker ;
    rdfs:label "Electric breaker4" ;
    s223:hasConnectionPoint psm:BR4InletConnectionPoint,
        psm:BR4OutletConnectionPoint .

psm:ElectricBreaker5 a s223:ElectricBreaker ;
    rdfs:label "Electric breaker5" ;
    s223:hasConnectionPoint psm:BR5InletConnectionPoint,
        psm:BR5OutletConnectionPoint .

psm:ExhaustAirDamperPosition a s223:QuantifiableActuatableProperty ;
    rdfs:label "Exhaust air damper position" ;
    s223:hasValue 50.0 ;
    qudt:hasQuantityKind quantitykind:Dimensionless ;
    qudt:unit unit:PERCENT .

psm:ExhaustFanStatus a s223:EnumeratedActuatableProperty ;
    rdfs:label "Exhaust fan status" ;
    s223:hasEnumerationKind s223:EnumerationKind-OnOff ;
    s223:hasValue s223:OnOff-On .

psm:FanInletConnectionPoint a s223:InletConnectionPoint ;
    rdfs:label "Fan inlet connection point" ;
    s223:cnx psm:BathroomExhaustDuct ;
    s223:hasMedium s223:Medium-Air .

psm:FanOutletConnectionPoint a s223:OutletConnectionPoint ;
    rdfs:label "Fan outlet connection point" ;
    s223:cnx psm:OutsideAir ;
    s223:hasMedium s223:Medium-Air .

psm:HVAC4-5Connection a s223:Connection ;
    rdfs:label "HVAC4-5Connection" ;
    s223:cnx psm:InletIntraCorridor4CP ;
    s223:hasMedium s223:Medium-Air .

psm:HVACZone1Temperature a s223:QuantifiableObservableProperty ;
    rdfs:label "HVACZone1Temperature" ;
    s223:hasValue 69.7 ;
    qudt:hasQuantityKind quantitykind:Temperature ;
    qudt:unit unit:DEG_F .

psm:HVACZone2 a s223:Zone ;
    rdfs:label "HVACZone2" ;
    s223:contains psm:HVACSpace5,
        psm:HVACSpace6 ;
    s223:hasDomain s223:Domain-HVAC .

psm:HVACZone2Temperature a s223:QuantifiableObservableProperty ;
    rdfs:label "HVACZone2Temperature" ;
    s223:hasValue 73.2 ;
    qudt:hasQuantityKind quantitykind:Temperature ;
    qudt:unit unit:DEG_F .

psm:HeatingCoilOutletTemperature a s223:QuantifiableObservableProperty ;
    rdfs:label "Heating coil outlet temperature" ;
    s223:hasValue 80.0 ;
    qudt:hasQuantityKind quantitykind:Temperature ;
    qudt:unit unit:DEG_F .

psm:HeatingCoilValvePosition a s223:QuantifiableActuatableProperty ;
    rdfs:label "Heating coil valve position" ;
    s223:hasValue 50.0 ;
    qudt:hasQuantityKind quantitykind:Dimensionless ;
    qudt:unit unit:PERCENT .

psm:InletIntraCorridor4CP a s223:InletConnectionPoint ;
    rdfs:label "Inlet intra corridor4CP" ;
    s223:hasMedium s223:Medium-Air ;
    s223:isConnectionPointOf psm:HVACSpace4 .

psm:KitchenetteLight1 a s223:Connection ;
    rdfs:label "Kitchenette light1" ;
    s223:cnx psm:KitchenetteLightInletCP,
        psm:Luminaire11Outlet ;
    s223:hasMedium s223:Light-Visible .

psm:LIghtingSpace1DLInlet a s223:InletConnectionPoint ;
    rdfs:label "Lighting Space1 DL Inlet" ;
    s223:cnx psm:DLightPath1 ;
    s223:hasMedium s223:Light-Visible .

psm:LightEngine1Outlet a s223:OutletConnectionPoint ;
    rdfs:label "Light Engine 1 Outlet" ;
    s223:cnx psm:ELightPath1 ;
    s223:hasMedium s223:Light-Visible ;
    s223:mapsTo psm:Luminaire1Outlet .

psm:Luminaire10Inlet a s223:InletConnectionPoint ;
    rdfs:label "Luminaire10Inlet" ;
    s223:cnx psm:ElectricCircuit2 ;
    s223:hasMedium s223:AC-120V-60Hz .

psm:Luminaire10OnOffStatus a s223:EnumerableProperty ;
    rdfs:label "Luminaire10On off status" ;
    s223:hasEnumerationKind s223:EnumerationKind-OnOff ;
    s223:hasValue s223:OnOff-Off .

psm:Luminaire10Outlet a s223:OutletConnectionPoint ;
    rdfs:label "Luminaire10Outlet" ;
    s223:cnx psm:CorridorLight1 ;
    s223:hasMedium s223:Light-Visible .

psm:Luminaire11 a s223:Luminaire ;
    rdfs:label "Luminaire11" ;
    s223:hasConnectionPoint psm:Luminaire11Inlet,
        psm:Luminaire11Outlet ;
    s223:hasPhysicalLocation psm:Kitchenette ;
    s223:hasProperty psm:Luminaire11OnOffStatus .

psm:Luminaire11Inlet a s223:InletConnectionPoint ;
    rdfs:label "Luminaire11Inlet" ;
    s223:cnx psm:ElectricCircuit2 ;
    s223:hasMedium s223:AC-120V-60Hz .

psm:Luminaire11OnOffStatus a s223:EnumerableProperty ;
    rdfs:label "Luminaire11On off status" ;
    s223:hasEnumerationKind s223:EnumerationKind-OnOff ;
    s223:hasValue s223:OnOff-Off .

psm:Luminaire12 a s223:Luminaire ;
    rdfs:label "Luminaire12" ;
    s223:hasConnectionPoint psm:Luminaire12Inlet,
        psm:Luminaire12Outlet ;
    s223:hasPhysicalLocation psm:Kitchenette ;
    s223:hasProperty psm:Luminaire12OnOffStatus .

psm:Luminaire12Inlet a s223:InletConnectionPoint ;
    rdfs:label "Luminaire12Inlet" ;
    s223:cnx psm:ElectricCircuit2 ;
    s223:hasMedium s223:AC-120V-60Hz .

psm:Luminaire12OnOffStatus a s223:EnumerableProperty ;
    rdfs:label "Luminaire12On off status" ;
    s223:hasEnumerationKind s223:EnumerationKind-OnOff ;
    s223:hasValue s223:OnOff-Off .

psm:Luminaire12Outlet a s223:OutletConnectionPoint ;
    rdfs:label "Luminaire12Outlet" ;
    s223:cnx psm:KitchenetteLight1 ;
    s223:hasMedium s223:Light-Visible .

psm:Luminaire1CCTSettingOutput a s223:FunctionOutput ;
    rdfs:label "Luminaire1CCTSettingOutput" ;
    s223:produces psm:Luminaire1CCT .

psm:Luminaire1DaylightFunctionInput a s223:FunctionInput ;
    rdfs:label "Luminaire1Daylight function input" ;
    s223:uses psm:OpenOfficeDaylightLevel .

psm:Luminaire1IntensitySettingOutput a s223:FunctionOutput ;
    rdfs:label "Luminaire1Intensity setting output" ;
    s223:produces psm:Luminaire1Intensity .

psm:Luminaire1InternalWire a s223:ElectricWire ;
    rdfs:label "Luminaire1Internal wire" ;
    s223:cnx psm:LightEngine1Inlet ;
    s223:hasMedium s223:Medium-Electricity .

psm:Luminaire1OccupancyFunctionInput a s223:FunctionInput ;
    rdfs:label "Luminaire1Occupancy function input" ;
    s223:uses psm:OccupancyProp1 .

psm:Luminaire1OnOffSettingOutput a s223:FunctionOutput ;
    rdfs:label "Luminaire1On off setting output" ;
    s223:produces psm:Luminaire1OnOff .

psm:Luminaire2CCTSettingOutput a s223:FunctionOutput ;
    rdfs:label "Luminaire2CCTSettingOutput" ;
    s223:produces psm:Luminaire2CCT .

psm:Luminaire2DaylightFunctionInput a s223:FunctionInput ;
    rdfs:label "Luminaire2DaylightFunctionInput" ;
    s223:uses psm:OpenOfficeDaylightLevel .

psm:Luminaire2Inlet a s223:InletConnectionPoint ;
    rdfs:label "Luminaire2Inlet" ;
    s223:cnx psm:ElectricCircuit1 ;
    s223:hasMedium s223:AC-120V-60Hz .

psm:Luminaire2IntensitySettingOutput a s223:FunctionOutput ;
    rdfs:label "Luminaire2Intensity setting output" ;
    s223:produces psm:Luminaire2Intensity .

psm:Luminaire2OccupancyFunctionInput1 a s223:FunctionInput ;
    rdfs:label "Luminaire2 occupancy function input1" ;
    s223:uses psm:OccupancyProp1 .

psm:Luminaire2OnOffSettingOutput a s223:FunctionOutput ;
    rdfs:label "Luminaire2On off setting output" ;
    s223:produces psm:Luminaire2OnOff .

psm:Luminaire2OnOffStatus a s223:EnumerableProperty ;
    rdfs:label "Luminaire2On off status" ;
    s223:hasEnumerationKind s223:EnumerationKind-OnOff ;
    s223:hasValue s223:OnOff-Off .

psm:Luminaire2Outlet a s223:OutletConnectionPoint ;
    rdfs:label "Luminaire2Outlet" ;
    s223:cnx psm:ELightPath1 ;
    s223:hasMedium s223:Light-Visible .

psm:Luminaire3Inlet a s223:InletConnectionPoint ;
    rdfs:label "Luminaire3Inlet" ;
    s223:cnx psm:ElectricCircuit1 ;
    s223:hasMedium s223:AC-120V-60Hz .

psm:Luminaire3OnOffStatus a s223:EnumerableProperty ;
    rdfs:label "Luminaire3On off status" ;
    s223:hasEnumerationKind s223:EnumerationKind-OnOff ;
    s223:hasValue s223:OnOff-Off .

psm:Luminaire3Outlet a s223:OutletConnectionPoint ;
    rdfs:label "Luminaire3Outlet" ;
    s223:cnx psm:ELightPath2 ;
    s223:hasMedium s223:Light-Visible .

psm:Luminaire4Inlet a s223:InletConnectionPoint ;
    rdfs:label "Luminaire4Inlet" ;
    s223:cnx psm:ElectricCircuit1 ;
    s223:hasMedium s223:AC-120V-60Hz .

psm:Luminaire4OnOffStatus a s223:EnumerableProperty ;
    rdfs:label "Luminaire4On off status" ;
    s223:hasEnumerationKind s223:EnumerationKind-OnOff ;
    s223:hasValue s223:OnOff-Off .

psm:Luminaire4Outlet a s223:OutletConnectionPoint ;
    rdfs:label "Luminaire4Outlet" ;
    s223:cnx psm:ELightPath2 ;
    s223:hasMedium s223:Light-Visible .

psm:Luminaire5Inlet a s223:InletConnectionPoint ;
    rdfs:label "Luminaire5Inlet" ;
    s223:cnx psm:ElectricCircuit2 ;
    s223:hasMedium s223:AC-120V-60Hz .

psm:Luminaire5OnOffStatus a s223:EnumerableProperty ;
    rdfs:label "Luminaire5On off status" ;
    s223:hasEnumerationKind s223:EnumerationKind-OnOff ;
    s223:hasValue s223:OnOff-Off .

psm:Luminaire5Outlet a s223:OutletConnectionPoint ;
    rdfs:label "Luminaire5Outlet" ;
    s223:cnx psm:BathroomLight1 ;
    s223:hasMedium s223:Light-Visible .

psm:Luminaire6Inlet a s223:InletConnectionPoint ;
    rdfs:label "Luminaire6Inlet" ;
    s223:cnx psm:ElectricCircuit2 ;
    s223:hasMedium s223:AC-120V-60Hz .

psm:Luminaire6OnOffStatus a s223:EnumerableProperty ;
    rdfs:label "Luminaire6On off status" ;
    s223:hasEnumerationKind s223:EnumerationKind-OnOff ;
    s223:hasValue s223:OnOff-Off .

psm:Luminaire6Outlet a s223:OutletConnectionPoint ;
    rdfs:label "Luminaire6Outlet" ;
    s223:cnx psm:BathroomLight1 ;
    s223:hasMedium s223:Light-Visible .

psm:Luminaire7Inlet a s223:InletConnectionPoint ;
    rdfs:label "Luminaire7Inlet" ;
    s223:cnx psm:ElectricCircuit2 ;
    s223:hasMedium s223:AC-120V-60Hz .

psm:Luminaire7OnOffStatus a s223:EnumerableProperty ;
    rdfs:label "Luminaire7On off status" ;
    s223:hasEnumerationKind s223:EnumerationKind-OnOff ;
    s223:hasValue s223:OnOff-Off .

psm:Luminaire7Outlet a s223:OutletConnectionPoint ;
    rdfs:label "Luminaire7Outlet" ;
    s223:cnx psm:PrivateOfficeLight1 ;
    s223:hasMedium s223:Light-Visible .

psm:Luminaire8Inlet a s223:InletConnectionPoint ;
    rdfs:label "Luminaire8Inlet" ;
    s223:cnx psm:ElectricCircuit2 ;
    s223:hasMedium s223:AC-120V-60Hz .

psm:Luminaire8OnOffStatus a s223:EnumerableProperty ;
    rdfs:label "Luminaire8On off status" ;
    s223:hasEnumerationKind s223:EnumerationKind-OnOff ;
    s223:hasValue s223:OnOff-Off .

psm:Luminaire8Outlet a s223:OutletConnectionPoint ;
    rdfs:label "Luminaire8Outlet" ;
    s223:cnx psm:PrivateOfficeLight1 ;
    s223:hasMedium s223:Light-Visible .

psm:Luminaire9Inlet a s223:InletConnectionPoint ;
    rdfs:label "Luminaire9Inlet" ;
    s223:cnx psm:ElectricCircuit2 ;
    s223:hasMedium s223:AC-120V-60Hz .

psm:Luminaire9OnOffStatus a s223:EnumerableProperty ;
    rdfs:label "Luminaire9On off status" ;
    s223:hasEnumerationKind s223:EnumerationKind-OnOff ;
    s223:hasValue s223:OnOff-Off .

psm:Luminaire9Outlet a s223:OutletConnectionPoint ;
    rdfs:label "Luminaire9Outlet" ;
    s223:cnx psm:CorridorLight1 ;
    s223:hasMedium s223:Light-Visible .

psm:MainBreakerCircuit3 a s223:ElectricWire ;
    rdfs:label "Main breaker circuit3" ;
    s223:cnx psm:BR3InletConnectionPoint ;
    s223:hasMedium s223:AC-240V-60Hz .

psm:MainBreakerInletCP a s223:InletConnectionPoint ;
    rdfs:label "Main breaker inlet CP" ;
    s223:hasMedium s223:AC-120V-240V-60Hz .

psm:MainBreakerOutCP1 a s223:OutletConnectionPoint ;
    rdfs:label "Main breaker out CP1" ;
    s223:cnx psm:MainBreakerCircuit1 ;
    s223:hasMedium s223:AC-120V-60Hz ;
    s223:hasProperty psm:BreakerCP1Phase .

psm:MainBreakerOutCP2 a s223:OutletConnectionPoint ;
    rdfs:label "Main breaker out CP2" ;
    s223:cnx psm:MainBreakerCircuit2 ;
    s223:hasMedium s223:AC-120V-60Hz ;
    s223:hasProperty psm:BreakerCP2Phase .

psm:MainBreakerOutCP3 a s223:OutletConnectionPoint ;
    rdfs:label "Main breaker out CP3" ;
    s223:cnx psm:MainBreakerCircuit3 ;
    s223:hasMedium s223:AC-240V-60Hz ;
    s223:hasProperty psm:BreakerCP3Phase .

psm:MixedAirDamperPosition a s223:QuantifiableActuatableProperty ;
    rdfs:label "Mixed air damper position" ;
    s223:hasValue 50.0 ;
    qudt:hasQuantityKind quantitykind:Dimensionless ;
    qudt:unit unit:PERCENT .

psm:MixedAirPressure a s223:QuantifiableObservableProperty ;
    rdfs:label "Mixed air pressure" ;
    s223:hasValue 15.5 ;
    qudt:hasQuantityKind quantitykind:Pressure ;
    qudt:unit unit:PSI .

psm:OccSensor5 a s223:OccupantPresenceSensor ;
    rdfs:label "O5" ;
    s223:hasMeasurementLocation psm:OccupancySpace5 ;
    s223:observes psm:OccupancyProp5 .

psm:OccupancyProp2 a s223:EnumeratedObservableProperty ;
    rdfs:label "Occupancy prop2" ;
    s223:hasEnumerationKind s223:Occupancy-Motion ;
    s223:hasValue s223:Motion-True .

psm:OccupancyProp3 a s223:EnumeratedObservableProperty ;
    rdfs:label "Occupancy prop3" ;
    s223:hasEnumerationKind s223:Occupancy-Presence ;
    s223:hasValue s223:Presence-True .

psm:OccupancyProp4 a s223:EnumeratedObservableProperty ;
    rdfs:label "Occupancy prop4" ;
    s223:hasEnumerationKind s223:Occupancy-Motion ;
    s223:hasValue s223:Motion-True .

psm:OccupancyProp5 a s223:EnumeratedObservableProperty ;
    rdfs:label "Occupancy prop5" ;
    s223:hasEnumerationKind s223:Occupancy-Presence ;
    s223:hasValue s223:Presence-True .

psm:OpenOfficeOutletConnectionPoint a s223:OutletConnectionPoint ;
    rdfs:label "Open office outlet connection point" ;
    s223:cnx psm:ReturnDuct ;
    s223:hasMedium s223:Medium-Air .

psm:OutletIntraCorridor5CP a s223:OutletConnectionPoint ;
    rdfs:label "Outlet intra corridor5CP" ;
    s223:cnx psm:HVAC4-5Connection ;
    s223:hasMedium s223:Medium-Air .

psm:OutsideAir a s223:Connection ;
    rdfs:label "Outside air" ;
    s223:hasMedium s223:Medium-Air .

psm:OutsideAirDamperPosition a s223:QuantifiableActuatableProperty ;
    rdfs:label "Outside air damper position" ;
    s223:hasValue 50.0 ;
    qudt:hasQuantityKind quantitykind:Dimensionless ;
    qudt:unit unit:PERCENT .

psm:PipeFromChiller a s223:Connection ;
    rdfs:label "Pipe from chiller" ;
    s223:hasMedium s223:Water-ChilledWater .

psm:PipeToBoiler a s223:Connection ;
    rdfs:label "Pipe to boiler" ;
    s223:hasMedium s223:Water-HotWater .

psm:PipeToChiller a s223:Connection ;
    rdfs:label "Pipe to chiller" ;
    s223:hasMedium s223:Water-ChilledWater .

psm:PrivateOffice a s223:PhysicalSpace ;
    rdfs:label "Private office" ;
    s223:encloses psm:HVACSpace3,
        psm:LightingSpace4,
        psm:OccupancySpace3 .

psm:PrivateOfficeLightInletCP a s223:InletConnectionPoint ;
    rdfs:label "Private office light inlet CP" ;
    s223:cnx psm:PrivateOfficeLight1 ;
    s223:hasMedium s223:Light-Visible .

psm:ReturnAirFlowRate a g36:AnalogIn ;
    rdfs:label "Return air flow rate" ;
    s223:hasValue 129.3 ;
    qudt:hasQuantityKind quantitykind:VolumeFlowRate ;
    qudt:unit unit:FT3-PER-MIN .

psm:ReturnDuct a s223:Connection ;
    rdfs:label "Return duct" ;
    s223:cnx psm:i00052 ;
    s223:hasMedium s223:Medium-Air ;
    s223:hasProperty psm:ratmp .

psm:ReturnFanSpeed a s223:QuantifiableActuatableProperty ;
    rdfs:label "Return fan speed" ;
    s223:hasValue 70.0 ;
    qudt:hasQuantityKind quantitykind:Dimensionless ;
    qudt:unit unit:PERCENT .

psm:ReturnFanStatus a s223:EnumeratedActuatableProperty ;
    rdfs:label "Return fan status" ;
    s223:hasEnumerationKind s223:EnumerationKind-OnOff ;
    s223:hasValue s223:OnOff-On .

psm:SupplyFanElectricInCP a s223:InletConnectionPoint ;
    rdfs:label "Supply fan electric in CP" ;
    s223:cnx psm:ElectricCircuit3 ;
    s223:hasMedium s223:AC-240V-60Hz .

psm:SupplyFanSpeed a s223:QuantifiableActuatableProperty ;
    rdfs:label "Supply fan speed" ;
    s223:hasValue 80.0 ;
    qudt:hasQuantityKind quantitykind:Dimensionless ;
    qudt:unit unit:PERCENT .

psm:SupplyFanStatus a s223:EnumeratedActuatableProperty ;
    rdfs:label "Supply fan status" ;
    s223:hasEnumerationKind s223:EnumerationKind-OnOff ;
    s223:hasValue s223:OnOff-On .

psm:VAV1InletFlow a s223:QuantifiableObservableProperty ;
    rdfs:label "VAV1Inlet flow" ;
    s223:hasValue 135.0 ;
    qudt:hasQuantityKind quantitykind:VolumeFlowRate ;
    qudt:unit unit:FT3-PER-MIN .

psm:VAV1OutletTemperature a s223:QuantifiableObservableProperty ;
    rdfs:label "VAV1 Outlet Temperature" ;
    s223:hasValue 72.3 ;
    qudt:hasQuantityKind quantitykind:Temperature ;
    qudt:unit unit:DEG_F .

psm:VAV1ReheatCoilSupplyFluidInlet a s223:InletConnectionPoint ;
    rdfs:label "VAV1Reheat coil supply fluid inlet" ;
    s223:hasMedium s223:Water-HotWater .

psm:VAV1ReheatCoilSupplyFluidOutlet a s223:OutletConnectionPoint ;
    rdfs:label "VAV1Reheat coil supply fluid outlet" ;
    s223:hasMedium s223:Water-HotWater .

psm:VAV2InletFlow a s223:QuantifiableObservableProperty ;
    rdfs:label "VAV2Inlet flow" ;
    s223:hasValue 250.0 ;
    qudt:hasQuantityKind quantitykind:VolumeFlowRate ;
    qudt:unit unit:FT3-PER-MIN .

psm:VAV2OutletTemperatureProperty a s223:QuantifiableObservableProperty ;
    rdfs:label "VAV2Outlet temperature property" ;
    s223:hasValue 70.0 ;
    qudt:hasQuantityKind quantitykind:Temperature ;
    qudt:unit unit:DEG_F .

psm:VAV2ReheatCoilSupplyFluidInlet a s223:InletConnectionPoint ;
    rdfs:label "VAV2Reheat coil supply fluid inlet" ;
    s223:hasMedium s223:Water-HotWater .

psm:VAV2ReheatCoilSupplyFluidOutlet a s223:OutletConnectionPoint ;
    rdfs:label "VAV2Reheat coil supply fluid outlet" ;
    s223:hasMedium s223:Water-HotWater .

psm:VAVBox1DamperPosition a s223:QuantifiableActuatableProperty ;
    rdfs:label "VAVBox1Damper position" ;
    s223:hasValue 50.0 ;
    qudt:hasQuantityKind quantitykind:Dimensionless ;
    qudt:unit unit:PERCENT .

psm:VAVBox1HeatingCoil a s223:HeatingCoil ;
    rdfs:label "VAVBox1Heating coil" ;
    s223:hasConnectionPoint psm:VAV1InletReheatCoilCP,
        psm:VAV1OuletReheatCoilCP,
        psm:VAV1ReheatCoilSupplyFluidInlet,
        psm:VAV1ReheatCoilSupplyFluidOutlet .

psm:VAVBox1InletFlowSensor a s223:FlowSensor ;
    rdfs:label "S9" ;
    s223:hasMeasurementLocation psm:VAV2DamperInletCP ;
    s223:observes psm:VAV1InletFlow .

psm:VAVBox1MotorizedDamper a s223:MotorizedDamper ;
    rdfs:label "VAVBox1Motorized damper " ;
    s223:hasConnectionPoint psm:VAV1DamperInletCP,
        psm:VAV1DamperOutletCP .

psm:VAVBox1OutletTemperatureSensor a s223:TemperatureSensor ;
    rdfs:label "S10" ;
    s223:hasMeasurementLocation psm:VAV1OuletReheatCoilCP ;
    s223:observes psm:VAV1OutletTemperature .

psm:VAVBox1ReheatValvePosition a s223:QuantifiableActuatableProperty ;
    rdfs:label "VAVBox1Reheat valve position" ;
    s223:hasValue 50.0 ;
    qudt:hasQuantityKind quantitykind:Dimensionless ;
    qudt:unit unit:PERCENT .

psm:VAVBox2DamperPosition a s223:QuantifiableActuatableProperty ;
    rdfs:label "VAVBox2Damper position" ;
    s223:hasValue 50.0 ;
    qudt:hasQuantityKind quantitykind:Dimensionless ;
    qudt:unit unit:PERCENT .

psm:VAVBox2HeatingCoil a s223:HeatingCoil ;
    rdfs:label "VAVBox2Heating coil" ;
    s223:hasConnectionPoint psm:VAV2InletReheatCoilCP,
        psm:VAV2OuletReheatCoilCP,
        psm:VAV2ReheatCoilSupplyFluidInlet,
        psm:VAV2ReheatCoilSupplyFluidOutlet .

psm:VAVBox2InletFlowSensor a s223:FlowSensor ;
    rdfs:label "S11" ;
    s223:hasMeasurementLocation psm:VAV2DamperInletCP ;
    s223:observes psm:VAV2InletFlow .

psm:VAVBox2MotorizedDamper a s223:MotorizedDamper ;
    rdfs:label "VAVBox2Motorized damper" ;
    s223:hasConnectionPoint psm:VAV2DamperInletCP,
        psm:VAV2DamperOutletCP .

psm:VAVBox2OutletTemperatureSensor a s223:TemperatureSensor ;
    rdfs:label "S12" ;
    s223:hasMeasurementLocation psm:VAV2OuletReheatCoilCP ;
    s223:observes psm:VAV2OutletTemperatureProperty .

psm:VAVBox2ReheatValvePosition a s223:QuantifiableActuatableProperty ;
    rdfs:label "VAVBox2Reheat valve position" ;
    s223:hasValue 50.0 ;
    qudt:hasQuantityKind quantitykind:Dimensionless ;
    qudt:unit unit:PERCENT .

psm:VAVSupply a s223:Connection ;
    rdfs:label "VAVSupply" ;
    s223:cnx psm:VAV1DamperInletCP,
        psm:VAV2DamperInletCP ;
    s223:hasMedium s223:Medium-Air .

psm:i00008 a s223:Property,
        g36:AnalogOut ;
    rdfs:label "Minimum outdoor air damper command" ;
    qudt:hasQuantityKind quantitykind:Dimensionless ;
    qudt:unit unit:PERCENT .

psm:i00012 a s223:Property,
        g36:AnalogIn ;
    rdfs:label "Outdoor air flow" ;
    qudt:hasQuantityKind quantitykind:VolumeFlowRate ;
    qudt:unit unit:FT3-PER-MIN .

psm:i00017 a s223:Property,
        g36:AnalogOut ;
    rdfs:label "Economizer outside air damper command" ;
    qudt:hasQuantityKind quantitykind:Dimensionless ;
    qudt:unit unit:PERCENT .

psm:i00022 a s223:Property,
        g36:AnalogIn ;
    rdfs:label "Mixed air temperature" ;
    qudt:hasQuantityKind quantitykind:Temperature ;
    qudt:unit unit:DEG_F .

psm:i00029 a s223:OutletConnectionPoint ;
    rdfs:label "A-9.hot_water_coil.hotWaterOutlet" ;
    s223:cnx psm:PipeToBoiler,
        psm:i00025 ;
    s223:hasMedium s223:Water-HotWater ;
    s223:mapsTo psm:AHUHotWaterOutlet .

psm:i00031 a s223:Property,
        g36:AnalogOut ;
    rdfs:label "Hot water valve command" ;
    qudt:hasQuantityKind quantitykind:Dimensionless ;
    qudt:unit unit:PERCENT .

psm:i00040 a s223:OutletConnectionPoint ;
    rdfs:label "A-9.chilled_water_coil.chilledWaterReturn" ;
    s223:cnx psm:PipeToChiller,
        psm:i00036 ;
    s223:hasMedium s223:Water-ChilledWater ;
    s223:mapsTo psm:AHUChilledWaterOutlet .

psm:i00042 a s223:Property,
        g36:AnalogOut ;
    rdfs:label "Chilled water valve command" ;
    qudt:hasQuantityKind quantitykind:Dimensionless ;
    qudt:unit unit:PERCENT .

psm:i00043 a s223:InletConnectionPoint ;
    rdfs:label "A-9.chilled_water_coil.chilled_water_valve.chilledWaterInlet" ;
    s223:cnx psm:PipeFromChiller,
        psm:i00041 ;
    s223:hasMedium s223:Water-ChilledWater ;
    s223:mapsTo psm:AHUChilledWaterInlet .

psm:i00057 a s223:Property,
        g36:AnalogOut ;
    rdfs:label "Exhaust air damper command" ;
    qudt:hasQuantityKind quantitykind:Dimensionless ;
    qudt:unit unit:PERCENT .

psm:i00060 a s223:Connection ;
    s223:cnx psm:i00059 ;
    s223:hasMedium s223:Medium-Air .

psm:i00062 a s223:Property,
        g36:AnalogOut ;
    rdfs:label "Return air damper command" ;
    qudt:hasQuantityKind quantitykind:Dimensionless ;
    qudt:unit unit:PERCENT .

<http://data.ashrae.org/standard223/1.0/extension/g36> owl:imports <http://data.ashrae.org/standard223/1.0/extension/g36-rules>,
        <http://data.ashrae.org/standard223/1.0/model/all> ;
    owl:versionInfo "Created with TopBraid Composer" .

g36:AirFlowStation a s223:Class,
        sh:NodeShape ;
    rdfs:label "Air Flow Station" ;
    rdfs:subClassOf s223:Sensor ;
    sh:node g36:AirFlowStationRule .

g36:DamperRule a sh:NodeShape ;
    sh:class s223:Damper ;
    sh:property [ rdfs:comment "The damper inlet connection point must map to exactly one VAV inlet connection point" ;
            sh:path s223:hasConnectionPoint ;
            sh:qualifiedMinCount 1 ;
            sh:qualifiedValueShape [ sh:class s223:InletConnectionPoint ;
                    sh:node [ sh:property [ sh:class s223:InletConnectionPoint ;
                                    sh:maxCount 1 ;
                                    sh:minCount 1 ;
                                    sh:node [ sh:property [ sh:class g36:VAV ;
                                                    sh:minCount 1 ;
                                                    sh:path [ sh:inversePath s223:hasConnectionPoint ] ] ] ;
                                    sh:path s223:mapsTo ] ] ] ],
        [ rdfs:comment "The damper outlet connection point must map to exactly one VAV outlet connection point" ;
            sh:path s223:hasConnectionPoint ;
            sh:qualifiedMinCount 1 ;
            sh:qualifiedValueShape [ sh:class s223:OutletConnectionPoint ;
                    sh:node [ sh:property [ sh:class s223:OutletConnectionPoint ;
                                    sh:maxCount 1 ;
                                    sh:minCount 1 ;
                                    sh:node [ sh:property [ sh:class g36:VAV ;
                                                    sh:minCount 1 ;
                                                    sh:path [ sh:inversePath s223:hasConnectionPoint ] ] ] ;
                                    sh:path s223:mapsTo ] ] ] ],
        [ sh:path s223:hasProperty ;
            sh:qualifiedMinCount 1 ;
            sh:qualifiedValueShape [ sh:class g36:AnalogOut ;
                    sh:node [ sh:property [ sh:hasValue s223:QuantityKind-RelativePosition ;
                                    sh:path qudt:hasQuantityKind ] ] ] ],
        [ sh:path s223:hasProperty ;
            sh:qualifiedMinCount 1 ;
            sh:qualifiedValueShape [ sh:class g36:AnalogOut ;
                    sh:property [ sh:hasValue s223:QuantityKind-RelativePosition ;
                            sh:path qudt:hasQuantityKind ] ] ] .

g36:DamperRule42 a sh:NodeShape ;
    sh:class s223:Damper ;
    sh:property [ rdfs:comment "The damper  must connectedTo at least one piece of equipment that is a Hot Water Coil." ;
            sh:path s223:connectedTo ;
            sh:qualifiedMinCount 1 ;
            sh:qualifiedValueShape [ sh:class g36:HotWaterCoil ] ],
        [ rdfs:comment "The damper inlet connection point must map to exactly one VAV inlet connection point" ;
            sh:path s223:hasConnectionPoint ;
            sh:qualifiedMinCount 1 ;
            sh:qualifiedValueShape [ sh:class s223:InletConnectionPoint ;
                    sh:node [ sh:property [ sh:class s223:InletConnectionPoint ;
                                    sh:maxCount 1 ;
                                    sh:minCount 1 ;
                                    sh:node [ sh:property [ sh:class g36:VAVWithReheat ;
                                                    sh:minCount 1 ;
                                                    sh:path [ sh:inversePath s223:hasConnectionPoint ] ] ] ;
                                    sh:path s223:mapsTo ] ] ] ],
        [ sh:path s223:hasProperty ;
            sh:qualifiedMinCount 1 ;
            sh:qualifiedValueShape [ sh:class g36:AnalogOut ;
                    sh:node [ sh:property [ sh:hasValue s223:QuantityKind-RelativePosition ;
                                    sh:path qudt:hasQuantityKind ] ] ] ] .

g36:EnumerationKind-Position a s223:Class,
        g36:EnumerationKind-Position,
        sh:NodeShape ;
    rdfs:label "For properties related to position" ;
    rdfs:comment "Would like to move this to vocab with other property enumeration kinds" ;
    rdfs:subClassOf s223:EnumerationKind .

g36:VAVRule a sh:NodeShape ;
    sh:class s223:SingleDuctTerminal ;
    sh:property [ sh:class s223:Damper ;
            sh:path s223:contains ],
        [ sh:path s223:contains ;
            sh:qualifiedMaxCount 1 ;
            sh:qualifiedMinCount 1 ;
            sh:qualifiedValueShape [ sh:class s223:Damper ] ;
            sh:qualifiedValueShapesDisjoint true ],
        [ sh:path s223:hasProperty ;
            sh:qualifiedMinCount 1 ;
            sh:qualifiedValueShape [ sh:class g36:AnalogIn ;
                    sh:node [ sh:property [ sh:hasValue quantitykind:VolumeFlowRate ;
                                    sh:path qudt:hasQuantityKind ] ] ] ],
        [ sh:path s223:hasProperty ;
            sh:qualifiedMinCount 1 ;
            sh:qualifiedValueShape [ sh:class g36:AnalogIn ;
                    sh:property [ sh:hasValue quantitykind:VolumeFlowRate ;
                            sh:path qudt:hasQuantityKind ] ] ] ;
    sh:severity sh:Info .

g36:ZoneRule a sh:NodeShape ;
    sh:class s223:Zone ;
    sh:property [ rdfs:comment "Window Switch (Should there be an Open/Close Enumeratable property?) " ;
            sh:path s223:contains ;
            sh:qualifiedMinCount 1 ;
            sh:qualifiedValueShape [ sh:class s223:DomainSpace ;
                    sh:node [ sh:property [ sh:class s223:Window ;
                                    sh:node [ sh:property [ sh:class s223:Sensor ;
                                                    sh:path [ sh:inversePath s223:hasObservationLocation ] ] ] ;
                                    sh:path s223:connectedTo ] ] ] ],
        [ sh:hasValue s223:Domain-HVAC ;
            sh:minCount 1 ;
            sh:path s223:hasDomain ],
        [ sh:hasValue s223:Domain-HVAC ;
            sh:minCount 1 ;
            sh:path s223:hasDomain ],
        [ rdfs:comment "Window Switch Property" ;
            sh:path s223:hasProperty ;
            sh:qualifiedMinCount 1 ;
            sh:qualifiedValueShape [ sh:class g36:BinaryIn ] ],
        [ rdfs:comment "Zone CO2" ;
            sh:path s223:hasProperty ;
            sh:qualifiedMinCount 1 ;
            sh:qualifiedValueShape [ sh:class g36:AnalogIn ;
                    sh:node [ sh:property [ sh:hasValue s223:Substance-CO2 ;
                                    sh:path s223:ofSubstance ],
                                [ sh:hasValue quantitykind:Concentration ;
                                    sh:path qudt:hasQuantityKind ] ] ] ],
        [ rdfs:comment "Zone CO2" ;
            sh:path s223:hasProperty ;
            sh:qualifiedMinCount 1 ;
            sh:qualifiedValueShape [ sh:class g36:AnalogIn ;
                    sh:node [ sh:property [ sh:hasValue s223:Substance-CO2 ;
                                    sh:path s223:ofSubstance ],
                                [ sh:hasValue quantitykind:Concentration ;
                                    sh:path qudt:hasQuantityKind ] ] ] ],
        [ rdfs:comment "Zone Occupancy" ;
            sh:path s223:hasProperty ;
            sh:qualifiedMinCount 1 ;
            sh:qualifiedValueShape [ sh:class g36:AnalogIn ;
                    sh:node [ sh:property [ sh:class s223:QuantityKind-Occupancy ;
                                    sh:path qudt:QuantityKind ] ] ] ],
        [ rdfs:comment "Zone Occupancy" ;
            sh:path s223:hasProperty ;
            sh:qualifiedMinCount 1 ;
            sh:qualifiedValueShape [ sh:class g36:BinaryIn ] ],
        [ rdfs:comment "Zone Temp" ;
            sh:path s223:hasProperty ;
            sh:qualifiedMinCount 1 ;
            sh:qualifiedValueShape [ sh:class g36:AnalogIn ;
                    sh:node [ sh:property [ sh:hasValue quantitykind:Temperature ;
                                    sh:path qudt:hasQuantityKind ] ] ] ],
        [ rdfs:comment "Zone Temp" ;
            sh:path s223:hasProperty ;
            sh:qualifiedMinCount 1 ;
            sh:qualifiedValueShape [ sh:class g36:AnalogIn ;
                    sh:node [ sh:property [ sh:hasValue quantitykind:Temperature ;
                                    sh:path qudt:hasQuantityKind ] ] ] ],
        [ rdfs:comment "Window Switch (Should there be an Open/Close Enumeratable property?) " ;
            sh:path s223:contains ;
            sh:qualifiedMinCount 1 ;
            sh:qualifiedValueShape [ sh:class s223:DomainSpace ;
                    sh:node [ sh:property [ sh:class s223:Window ;
                                    sh:node [ sh:property [ sh:class s223:Sensor ;
                                                    sh:path [ sh:inversePath s223:hasObservationLocation ] ] ] ;
                                    sh:path s223:connectedTo ] ] ] ] .

<http://data.ashrae.org/standard223/1.0/extension/g36-rules> owl:imports <http://data.ashrae.org/standard223/1.0/model/all> ;
    owl:versionInfo "Created with TopBraid Composer" .

<http://data.ashrae.org/standard223/1.0/inference/data-rules> owl:imports <http://data.ashrae.org/standard223/1.0/model/all> ;
    owl:versionInfo "Created with TopBraid Composer" .

<http://data.ashrae.org/standard223/1.0/inference/model-rules> owl:imports <http://data.ashrae.org/standard223/1.0/model/all> ;
    owl:versionInfo "Created with TopBraid Composer" .

<http://data.ashrae.org/standard223/1.0/inference/owl-subset> owl:imports <http://data.ashrae.org/standard223/1.0/model/all> ;
    owl:versionInfo "Created with TopBraid Composer" .

<http://data.ashrae.org/standard223/1.0/validation/data> owl:imports <http://data.ashrae.org/standard223/1.0/model/all> ;
    owl:versionInfo "Created with TopBraid Composer" .

<http://data.ashrae.org/standard223/1.0/validation/model> owl:imports <http://data.ashrae.org/standard223/1.0/model/all> ;
    owl:versionInfo "Created with TopBraid Composer" .

<http://data.ashrae.org/standard223/1.0/validation/schema> owl:imports <http://data.ashrae.org/standard223/1.0/model/all> ;
    owl:versionInfo "Created with TopBraid Composer" .

<http://data.ashrae.org/standard223/1.0/vocab/electricity> owl:imports <http://data.ashrae.org/standard223/1.0/model/all> .

rdfs:comment a rdf:Property ;
    rdfs:label "Description of constraints for s223" ;
    rdfs:subPropertyOf rdfs:comment .

sh:AndConstraintComponent-and a sh:Parameter ;
    rdfs:isDefinedBy sh: ;
    sh:path sh:and .

sh:BlankNode a sh:NodeKind ;
    rdfs:label "Blank node"@en ;
    rdfs:comment "The node kind of all blank nodes."@en ;
    rdfs:isDefinedBy sh: .

sh:BlankNodeOrIRI a sh:NodeKind ;
    rdfs:label "Blank node or IRI"@en ;
    rdfs:comment "The node kind of all blank nodes or IRIs."@en ;
    rdfs:isDefinedBy sh: .

sh:BlankNodeOrLiteral a sh:NodeKind ;
    rdfs:label "Blank node or literal"@en ;
    rdfs:comment "The node kind of all blank nodes or literals."@en ;
    rdfs:isDefinedBy sh: .

sh:ClassConstraintComponent-class a sh:Parameter ;
    rdfs:isDefinedBy sh: ;
    sh:nodeKind sh:IRI ;
    sh:path sh:class .

sh:ClosedConstraintComponent-closed a sh:Parameter ;
    rdfs:isDefinedBy sh: ;
    sh:datatype xsd:boolean ;
    sh:path sh:closed .

sh:ClosedConstraintComponent-ignoredProperties a sh:Parameter ;
    rdfs:isDefinedBy sh: ;
    sh:optional true ;
    sh:path sh:ignoredProperties .

sh:DatatypeConstraintComponent-datatype a sh:Parameter ;
    rdfs:isDefinedBy sh: ;
    sh:maxCount 1 ;
    sh:nodeKind sh:IRI ;
    sh:path sh:datatype .

sh:DisjointConstraintComponent-disjoint a sh:Parameter ;
    rdfs:isDefinedBy sh: ;
    sh:nodeKind sh:IRI ;
    sh:path sh:disjoint .

sh:EqualsConstraintComponent-equals a sh:Parameter ;
    rdfs:isDefinedBy sh: ;
    sh:nodeKind sh:IRI ;
    sh:path sh:equals .

sh:ExpressionConstraintComponent-expression a sh:Parameter ;
    rdfs:isDefinedBy sh: ;
    sh:path sh:expression .

sh:HasValueConstraintComponent-hasValue a sh:Parameter ;
    rdfs:isDefinedBy sh: ;
    sh:path sh:hasValue .

sh:IRIOrLiteral a sh:NodeKind ;
    rdfs:label "IRI or literal"@en ;
    rdfs:comment "The node kind of all IRIs or literals."@en ;
    rdfs:isDefinedBy sh: .

sh:InConstraintComponent-in a sh:Parameter ;
    rdfs:isDefinedBy sh: ;
    sh:maxCount 1 ;
    sh:path sh:in .

sh:JSConstraint-js a sh:Parameter ;
    rdfs:isDefinedBy sh: ;
    sh:path sh:js .

sh:LanguageInConstraintComponent-languageIn a sh:Parameter ;
    rdfs:isDefinedBy sh: ;
    sh:maxCount 1 ;
    sh:path sh:languageIn .

sh:LessThanConstraintComponent-lessThan a sh:Parameter ;
    rdfs:isDefinedBy sh: ;
    sh:nodeKind sh:IRI ;
    sh:path sh:lessThan .

sh:LessThanOrEqualsConstraintComponent-lessThanOrEquals a sh:Parameter ;
    rdfs:isDefinedBy sh: ;
    sh:nodeKind sh:IRI ;
    sh:path sh:lessThanOrEquals .

sh:MaxCountConstraintComponent-maxCount a sh:Parameter ;
    rdfs:isDefinedBy sh: ;
    sh:datatype xsd:integer ;
    sh:maxCount 1 ;
    sh:path sh:maxCount .

sh:MaxExclusiveConstraintComponent-maxExclusive a sh:Parameter ;
    rdfs:isDefinedBy sh: ;
    sh:maxCount 1 ;
    sh:nodeKind sh:Literal ;
    sh:path sh:maxExclusive .

sh:MaxInclusiveConstraintComponent-maxInclusive a sh:Parameter ;
    rdfs:isDefinedBy sh: ;
    sh:maxCount 1 ;
    sh:nodeKind sh:Literal ;
    sh:path sh:maxInclusive .

sh:MaxLengthConstraintComponent-maxLength a sh:Parameter ;
    rdfs:isDefinedBy sh: ;
    sh:datatype xsd:integer ;
    sh:maxCount 1 ;
    sh:path sh:maxLength .

sh:MinCountConstraintComponent-minCount a sh:Parameter ;
    rdfs:isDefinedBy sh: ;
    sh:datatype xsd:integer ;
    sh:maxCount 1 ;
    sh:path sh:minCount .

sh:MinExclusiveConstraintComponent-minExclusive a sh:Parameter ;
    rdfs:isDefinedBy sh: ;
    sh:maxCount 1 ;
    sh:nodeKind sh:Literal ;
    sh:path sh:minExclusive .

sh:MinInclusiveConstraintComponent-minInclusive a sh:Parameter ;
    rdfs:isDefinedBy sh: ;
    sh:maxCount 1 ;
    sh:nodeKind sh:Literal ;
    sh:path sh:minInclusive .

sh:MinLengthConstraintComponent-minLength a sh:Parameter ;
    rdfs:isDefinedBy sh: ;
    sh:datatype xsd:integer ;
    sh:maxCount 1 ;
    sh:path sh:minLength .

sh:NodeConstraintComponent-node a sh:Parameter ;
    rdfs:isDefinedBy sh: ;
    sh:path sh:node .

sh:NodeKindConstraintComponent-nodeKind a sh:Parameter ;
    rdfs:isDefinedBy sh: ;
    sh:in ( sh:BlankNode sh:IRI sh:Literal sh:BlankNodeOrIRI sh:BlankNodeOrLiteral sh:IRIOrLiteral ) ;
    sh:maxCount 1 ;
    sh:path sh:nodeKind .

sh:NotConstraintComponent-not a sh:Parameter ;
    rdfs:isDefinedBy sh: ;
    sh:path sh:not .

sh:OrConstraintComponent-or a sh:Parameter ;
    rdfs:isDefinedBy sh: ;
    sh:path sh:or .

sh:PatternConstraintComponent-flags a sh:Parameter ;
    rdfs:isDefinedBy sh: ;
    sh:datatype xsd:string ;
    sh:optional true ;
    sh:path sh:flags .

sh:PatternConstraintComponent-pattern a sh:Parameter ;
    rdfs:isDefinedBy sh: ;
    sh:datatype xsd:string ;
    sh:path sh:pattern .

sh:PropertyConstraintComponent-property a sh:Parameter ;
    rdfs:isDefinedBy sh: ;
    sh:path sh:property .

sh:QualifiedMaxCountConstraintComponent-qualifiedMaxCount a sh:Parameter ;
    rdfs:isDefinedBy sh: ;
    sh:datatype xsd:integer ;
    sh:path sh:qualifiedMaxCount .

sh:QualifiedMaxCountConstraintComponent-qualifiedValueShape a sh:Parameter ;
    rdfs:isDefinedBy sh: ;
    sh:path sh:qualifiedValueShape .

sh:QualifiedMaxCountConstraintComponent-qualifiedValueShapesDisjoint a sh:Parameter ;
    rdfs:isDefinedBy sh: ;
    sh:datatype xsd:boolean ;
    sh:optional true ;
    sh:path sh:qualifiedValueShapesDisjoint .

sh:QualifiedMinCountConstraintComponent-qualifiedMinCount a sh:Parameter ;
    rdfs:isDefinedBy sh: ;
    sh:datatype xsd:integer ;
    sh:path sh:qualifiedMinCount .

sh:QualifiedMinCountConstraintComponent-qualifiedValueShape a sh:Parameter ;
    rdfs:isDefinedBy sh: ;
    sh:path sh:qualifiedValueShape .

sh:QualifiedMinCountConstraintComponent-qualifiedValueShapesDisjoint a sh:Parameter ;
    rdfs:isDefinedBy sh: ;
    sh:datatype xsd:boolean ;
    sh:optional true ;
    sh:path sh:qualifiedValueShapesDisjoint .

sh:SPARQLConstraintComponent-sparql a sh:Parameter ;
    rdfs:isDefinedBy sh: ;
    sh:path sh:sparql .

sh:UniqueLangConstraintComponent-uniqueLang a sh:Parameter ;
    rdfs:isDefinedBy sh: ;
    sh:datatype xsd:boolean ;
    sh:maxCount 1 ;
    sh:path sh:uniqueLang .

sh:XoneConstraintComponent-xone a sh:Parameter ;
    rdfs:isDefinedBy sh: ;
    sh:path sh:xone .

sh:and a rdf:Property ;
    rdfs:label "and"@en ;
    rdfs:comment "RDF list of shapes to validate the value nodes against."@en ;
    rdfs:isDefinedBy sh: ;
    rdfs:range rdf:List .

sh:class a rdf:Property ;
    rdfs:label "class"@en ;
    rdfs:comment "The type that all value nodes must have."@en ;
    rdfs:isDefinedBy sh: ;
    rdfs:range rdfs:Class .

sh:closed a rdf:Property ;
    rdfs:label "closed"@en ;
    rdfs:comment "If set to true then the shape is closed."@en ;
    rdfs:isDefinedBy sh: ;
    rdfs:range xsd:boolean .

sh:datatype a rdf:Property ;
    rdfs:label "datatype"@en ;
    rdfs:comment "Specifies an RDF datatype that all value nodes must have."@en ;
    rdfs:isDefinedBy sh: ;
    rdfs:range rdfs:Datatype .

sh:disjoint a rdf:Property ;
    rdfs:label "disjoint"@en ;
    rdfs:comment "Specifies a property where the set of values must be disjoint with the value nodes."@en ;
    rdfs:isDefinedBy sh: ;
    rdfs:range rdf:Property .

sh:equals a rdf:Property ;
    rdfs:label "equals"@en ;
    rdfs:comment "Specifies a property that must have the same values as the value nodes."@en ;
    rdfs:isDefinedBy sh: ;
    rdfs:range rdf:Property .

sh:expression a rdf:Property ;
    rdfs:label "expression"@en ;
    rdfs:comment "The node expression that must return true for the value nodes."@en ;
    rdfs:isDefinedBy sh: .

sh:flags a rdf:Property ;
    rdfs:label "flags"@en ;
    rdfs:comment "An optional flag to be used with regular expression pattern matching."@en ;
    rdfs:isDefinedBy sh: ;
    rdfs:range xsd:string .

sh:hasValue a rdf:Property ;
    rdfs:label "has value"@en ;
    rdfs:comment "Specifies a value that must be among the value nodes."@en ;
    rdfs:isDefinedBy sh: .

sh:ignoredProperties a rdf:Property ;
    rdfs:label "ignored properties"@en ;
    rdfs:comment "An optional RDF list of properties that are also permitted in addition to those explicitly enumerated via sh:property/sh:path."@en ;
    rdfs:isDefinedBy sh: ;
    rdfs:range rdf:List .

sh:in a rdf:Property ;
    rdfs:label "in"@en ;
    rdfs:comment "Specifies a list of allowed values so that each value node must be among the members of the given list."@en ;
    rdfs:isDefinedBy sh: ;
    rdfs:range rdf:List .

sh:js a rdf:Property ;
    rdfs:label "JavaScript constraint"@en ;
    rdfs:comment "Constraints expressed in JavaScript." ;
    rdfs:isDefinedBy sh: ;
    rdfs:range sh:JSConstraint .

sh:languageIn a rdf:Property ;
    rdfs:label "language in"@en ;
    rdfs:comment "Specifies a list of language tags that all value nodes must have."@en ;
    rdfs:isDefinedBy sh: ;
    rdfs:range rdf:List .

sh:lessThan a rdf:Property ;
    rdfs:label "less than"@en ;
    rdfs:comment "Specifies a property that must have smaller values than the value nodes."@en ;
    rdfs:isDefinedBy sh: ;
    rdfs:range rdf:Property .

sh:lessThanOrEquals a rdf:Property ;
    rdfs:label "less than or equals"@en ;
    rdfs:comment "Specifies a property that must have smaller or equal values than the value nodes."@en ;
    rdfs:isDefinedBy sh: ;
    rdfs:range rdf:Property .

sh:maxCount a rdf:Property ;
    rdfs:label "max count"@en ;
    rdfs:comment "Specifies the maximum number of values in the set of value nodes."@en ;
    rdfs:isDefinedBy sh: ;
    rdfs:range xsd:integer .

sh:maxExclusive a rdf:Property ;
    rdfs:label "max exclusive"@en ;
    rdfs:comment "Specifies the maximum exclusive value of each value node."@en ;
    rdfs:isDefinedBy sh: .

sh:maxInclusive a rdf:Property ;
    rdfs:label "max inclusive"@en ;
    rdfs:comment "Specifies the maximum inclusive value of each value node."@en ;
    rdfs:isDefinedBy sh: .

sh:maxLength a rdf:Property ;
    rdfs:label "max length"@en ;
    rdfs:comment "Specifies the maximum string length of each value node."@en ;
    rdfs:isDefinedBy sh: ;
    rdfs:range xsd:integer .

sh:minCount a rdf:Property ;
    rdfs:label "min count"@en ;
    rdfs:comment "Specifies the minimum number of values in the set of value nodes."@en ;
    rdfs:isDefinedBy sh: ;
    rdfs:range xsd:integer .

sh:minExclusive a rdf:Property ;
    rdfs:label "min exclusive"@en ;
    rdfs:comment "Specifies the minimum exclusive value of each value node."@en ;
    rdfs:isDefinedBy sh: .

sh:minInclusive a rdf:Property ;
    rdfs:label "min inclusive"@en ;
    rdfs:comment "Specifies the minimum inclusive value of each value node."@en ;
    rdfs:isDefinedBy sh: .

sh:minLength a rdf:Property ;
    rdfs:label "min length"@en ;
    rdfs:comment "Specifies the minimum string length of each value node."@en ;
    rdfs:isDefinedBy sh: ;
    rdfs:range xsd:integer .

sh:node a rdf:Property ;
    rdfs:label "node"@en ;
    rdfs:comment "Specifies the node shape that all value nodes must conform to."@en ;
    rdfs:isDefinedBy sh: ;
    rdfs:range sh:NodeShape .

sh:nodeKind a rdf:Property ;
    rdfs:label "node kind"@en ;
    rdfs:comment "Specifies the node kind (e.g. IRI or literal) each value node."@en ;
    rdfs:isDefinedBy sh: ;
    rdfs:range sh:NodeKind .

sh:not a rdf:Property ;
    rdfs:label "not"@en ;
    rdfs:comment "Specifies a shape that the value nodes must not conform to."@en ;
    rdfs:isDefinedBy sh: ;
    rdfs:range sh:Shape .

sh:or a rdf:Property ;
    rdfs:label "or"@en ;
    rdfs:comment "Specifies a list of shapes so that the value nodes must conform to at least one of the shapes."@en ;
    rdfs:isDefinedBy sh: ;
    rdfs:range rdf:List .

sh:pattern a rdf:Property ;
    rdfs:label "pattern"@en ;
    rdfs:comment "Specifies a regular expression pattern that the string representations of the value nodes must match."@en ;
    rdfs:isDefinedBy sh: ;
    rdfs:range xsd:string .

sh:property a rdf:Property ;
    rdfs:label "property"@en ;
    rdfs:comment "Links a shape to its property shapes."@en ;
    rdfs:domain sh:Shape ;
    rdfs:isDefinedBy sh: ;
    rdfs:range sh:PropertyShape .

sh:qualifiedMaxCount a rdf:Property ;
    rdfs:label "qualified max count"@en ;
    rdfs:comment "The maximum number of value nodes that can conform to the shape."@en ;
    rdfs:isDefinedBy sh: ;
    rdfs:range xsd:integer .

sh:qualifiedMinCount a rdf:Property ;
    rdfs:label "qualified min count"@en ;
    rdfs:comment "The minimum number of value nodes that must conform to the shape."@en ;
    rdfs:isDefinedBy sh: ;
    rdfs:range xsd:integer .

sh:sparql a rdf:Property ;
    rdfs:label "constraint (in SPARQL)"@en ;
    rdfs:comment "Links a shape with SPARQL constraints."@en ;
    rdfs:domain sh:Shape ;
    rdfs:isDefinedBy sh: ;
    rdfs:range sh:SPARQLConstraint .

sh:uniqueLang a rdf:Property ;
    rdfs:label "unique languages"@en ;
    rdfs:comment "Specifies whether all node values must have a unique (or no) language tag."@en ;
    rdfs:isDefinedBy sh: ;
    rdfs:range xsd:boolean .

sh:xone a rdf:Property ;
    rdfs:label "exactly one"@en ;
    rdfs:comment "Specifies a list of shapes so that the value nodes must conform to exactly one of the shapes."@en ;
    rdfs:isDefinedBy sh: ;
    rdfs:range rdf:List .

s223:AbstractSensor a s223:Class,
        sh:NodeShape ;
    rdfs:label "Abstract sensor" ;
    s223:abstract true ;
    rdfs:comment "This is an abstract class that represents properties that are common to all sensor types." ;
    rdfs:subClassOf s223:Equipment ;
    sh:property [ rdfs:comment "A Sensor can be associated with a QuantifiableProperty using the relation hasMeasurementResolution" ;
            sh:class s223:QuantifiableProperty ;
            sh:path s223:hasMeasurementResolution ],
        [ rdfs:comment "A Sensor must be associated with exactly 1 ObservableProperty using the relation observes" ;
            sh:class s223:ObservableProperty ;
            sh:maxCount 1 ;
            sh:minCount 1 ;
            sh:path s223:observes ],
        [ sh:name "Test for compatible declared Substances" ;
            sh:path s223:measuresSubstance ;
            sh:sparql [ a sh:SPARQLConstraint ;
                    rdfs:comment "Ensure that the Substance identified by a sensor via the s223:measuresSubstance relation is compatible with the Substance identified by the Property being measured via the s223:ofSubstance relation." ;
                    sh:message "Sensor {$this} measures substance {?a}, but the measured Property identifies an incompatible substance of {?b} via the s223:ofSubstance relation." ;
                    sh:prefixes s223: ;
                    sh:select """
SELECT DISTINCT $this ?a ?b
WHERE {
$this s223:measuresSubstance ?a .
$this s223:observes/s223:ofSubstance ?b .
?a a/rdfs:subClassOf* s223:EnumerationKind .
?b a/rdfs:subClassOf* s223:EnumerationKind .
FILTER (?a != ?b ) .
FILTER (NOT EXISTS {?b a/rdfs:subClassOf* ?a}) .
FILTER (NOT EXISTS {?a a/rdfs:subClassOf* ?b}) .
}
""" ] ] .

s223:Attribute-Effectiveness a s223:Attribute-Effectiveness,
        s223:Class,
        sh:NodeShape ;
    rdfs:label "Attribute-Effectiveness" ;
    rdfs:subClassOf s223:Context-Attribute .

s223:Junction a s223:Class,
        sh:NodeShape ;
    rdfs:label "Junction" ;
    rdfs:comment "A Junction is used to join two or more Segments together. This might be where a duct splits or joins." ;
    rdfs:subClassOf s223:Concept ;
    sh:property [ rdfs:comment "A Junction should be associated with at least two Segments using the relation lnx" ;
            sh:class s223:Segment ;
            sh:message "Junction is missing one or more Segments" ;
            sh:minCount 2 ;
            sh:path s223:lnx ;
            sh:severity sh:Info ] .

s223:LineNeutralVoltage-208.0V a s223:Dimensioned-LineNeutralVoltage ;
    rdfs:label "208.0V Line-Neutral Voltage" ;
    s223:hasVoltage s223:Voltage-208.0V .

s223:ManualValve a s223:Class,
        sh:NodeShape ;
    rdfs:label "Manual Valve" ;
    rdfs:subClassOf s223:Valve .

s223:Medium-NaturalGas a s223:Class,
        s223:Medium-NaturalGas ;
    rdfs:label "Medium-NaturalGas" ;
    rdfs:subClassOf s223:EnumerationKind-Medium .

s223:Motion-True a s223:Occupancy-Motion ;
    rdfs:label "Motion-True" .

s223:MotorizedValve a s223:Class,
        sh:NodeShape ;
    rdfs:label "Motorized Valve" ;
    rdfs:subClassOf s223:Valve .

s223:OccupantMotionSensor a s223:Class,
        sh:NodeShape ;
    rdfs:label "Occupant motion sensor" ;
    rdfs:subClassOf s223:OccupancySensor ;
    sh:property [ rdfs:comment "A OccupantMotionSensor will always observe a Property that has an EnumerationKind of Occupancy-Motion." ;
            sh:path s223:observes ;
            sh:qualifiedMinCount 1 ;
            sh:qualifiedValueShape [ sh:class s223:Property ;
                    sh:node [ sh:property [ sh:hasValue s223:Occupancy-Motion ;
                                    sh:path s223:hasEnumerationKind ] ] ] ] .

s223:OccupantPresenceSensor a s223:Class,
        sh:NodeShape ;
    rdfs:label "Occupant presence sensor" ;
    rdfs:subClassOf s223:OccupancySensor ;
    sh:property [ rdfs:comment "A OccupantPresenceSensor will always observe a Property that has an EnumerationKind of Occupancy-Presence." ;
            sh:path s223:observes ;
            sh:qualifiedMinCount 1 ;
            sh:qualifiedValueShape [ sh:class s223:Property ;
                    sh:node [ sh:property [ sh:hasValue s223:Occupancy-Presence ;
                                    sh:path s223:hasEnumerationKind ] ] ] ] .

s223:Parameter a s223:Class,
        sh:NodeShape ;
    rdfs:label "Parameter" ;
    rdfs:comment "A parameter belongs to exactly one Function Block." ;
    rdfs:subClassOf s223:Concept ;
    sh:property [ rdfs:comment "An instance of Parameter can be associated with any number of Property instances using the relation 'uses'." ;
            sh:class s223:Property ;
            sh:path s223:uses ],
        [ sh:class s223:FunctionBlock ;
            sh:maxCount 1 ;
            sh:message "This Parameter must be associated with exactly one FunctionBlock." ;
            sh:minCount 1 ;
            sh:path [ sh:inversePath s223:hasParameter ] ] .

s223:Phase-Gas a s223:Class,
        s223:Phase-Gas,
        sh:NodeShape ;
    rdfs:label "Phase-Gas" ;
    rdfs:subClassOf s223:EnumerationKind-Phase .

s223:Phase-Liquid a s223:Class,
        s223:Phase-Liquid,
        sh:NodeShape ;
    rdfs:label "Phase-Liquid" ;
    rdfs:subClassOf s223:EnumerationKind-Phase .

s223:Presence-True a s223:Occupancy-Presence ;
    rdfs:label "Presence-True" .

s223:PressureSensor a s223:Class,
        sh:NodeShape ;
    rdfs:label "Pressure sensor" ;
    rdfs:comment "A PressureSensor is a specialization of a Sensor that observes a QuantifiableObservableProperty that represents a pressure measurement." ;
    rdfs:subClassOf s223:Sensor .

s223:SingleDuctTerminal a s223:Class,
        sh:NodeShape ;
    rdfs:label "Single Duct Terminal." ;
    rdfs:comment "An air-terminal unit assembly having one ducted air inlet and a damper for regulating the airflow rate." ;
    rdfs:subClassOf s223:TerminalUnit ;
    sh:property [ rdfs:comment "A SingleDuctTerminal must be associated with at least 1 Damper by contains." ;
            sh:minCount 1 ;
            sh:path s223:contains ;
            sh:qualifiedMinCount 1 ;
            sh:qualifiedValueShape [ sh:class s223:Damper ] ] .

s223:Substance-CO2 a s223:EnumerationKind-Substance ;
    rdfs:label "Substance-CO2" .

s223:Voltage-208.0V a s223:Dimensioned-Voltage,
        s223:QuantifiableProperty ;
    rdfs:label "208.0V Voltage" ;
    s223:hasValue 208.0 ;
    qudt:hasQuantityKind quantitykind:Voltage ;
    qudt:hasUnit unit:V .

s223:Voltage-240.0V a s223:Dimensioned-Voltage,
        s223:QuantifiableProperty ;
    rdfs:label "240.0V Voltage" ;
    s223:hasValue 240.0 ;
    qudt:hasQuantityKind quantitykind:Voltage ;
    qudt:hasUnit unit:V .

s223:Window a s223:Class,
        sh:NodeShape ;
    rdfs:label "Window" ;
    rdfs:comment "A daylight opening on a vertical or nearly vertical area of a room envelope" ;
    rdfs:subClassOf s223:Equipment ;
    sh:property [ rdfs:comment "A Window shall have at least one inlet using the medium Light." ;
            sh:path s223:hasConnectionPoint ;
            sh:qualifiedMinCount 1 ;
            sh:qualifiedValueShape [ sh:class s223:InletConnectionPoint ;
                    sh:node [ sh:property [ sh:class s223:EM-Light ;
                                    sh:path s223:hasMedium ] ] ] ],
        [ rdfs:comment "A Window shall have at least one outlet using the medium Light." ;
            sh:path s223:hasConnectionPoint ;
            sh:qualifiedMinCount 1 ;
            sh:qualifiedValueShape [ sh:class s223:OutletConnectionPoint ;
                    sh:node [ sh:property [ sh:class s223:EM-Light ;
                                    sh:path s223:hasMedium ] ] ] ],
        [ sh:minCount 2 ;
            sh:path s223:hasConnectionPoint ] .

s223:commandedByProperty a rdf:Property ;
    rdfs:label "commanded by Property" ;
    rdfs:comment "The relation commandedByProperty binds an Actuator to the ActuatableProperty that it responds to. This Property will be owned by the equipment that it actuates (see `s223:actuates`)." .

s223:connectedThrough a rdf:Property ;
    rdfs:label "connected through" .

s223:encloses a rdf:Property ;
    rdfs:label "encloses" ;
    rdfs:comment "The relation encloses is used to indicate that a domain space (see: `s223:DomainSpace`) can be found inside a physical space (see `s223:PhysicalSpace`). " .

s223:hasInput a rdf:Property ;
    rdfs:label "has function input" ;
    rdfs:comment "The relation hasInput is used to relate a function input (see `s223:FunctionInput`) to a function block (see `s223:FunctionBlock`). " .

s223:hasOutput a rdf:Property ;
    rdfs:label "has function output" ;
    rdfs:comment "The relation hasOutput is used to relate a function output (see `s223:FunctionOutput`) to a function block (see `s223:FunctionBlock`). " .

s223:hasParameter a rdf:Property ;
    rdfs:label "has parameter" ;
    rdfs:comment "A Parameter (`s223:Parameter`) is associated to a function block (`s223:FunctionBlock`) using the relation hasParameter. " .

psm:AHUChilledWaterInlet a s223:InletConnectionPoint ;
    rdfs:label "AHUChilled water inlet" ;
    s223:hasMedium s223:Water-ChilledWater .

psm:AHUChilledWaterOutlet a s223:OutletConnectionPoint ;
    rdfs:label "AHUChilled water outlet" ;
    s223:hasMedium s223:Water-ChilledWater .

psm:AHUExhaustOutlet a s223:OutletConnectionPoint ;
    rdfs:label "AHUExhaust outlet" ;
    s223:hasMedium s223:Medium-Air .

psm:AHUHotWaterInlet a s223:InletConnectionPoint ;
    rdfs:label "AHUHot water inlet" ;
    s223:hasMedium s223:Water-HotWater .

psm:AHUHotWaterOutlet a s223:OutletConnectionPoint ;
    rdfs:label "AHUHot water outlet" ;
    s223:hasMedium s223:Water-HotWater .

psm:AHUOAInlet a s223:InletConnectionPoint ;
    rdfs:label "AHUOAInlet" ;
    s223:hasMedium s223:Medium-Air .

psm:AHUReturnInlet a s223:InletConnectionPoint ;
    rdfs:label "AHUReturn inlet" ;
    s223:hasMedium s223:Medium-Air .

psm:AHUSupplyOutlet a s223:OutletConnectionPoint ;
    rdfs:label "AHUSupply outlet" ;
    s223:hasMedium s223:Medium-Air .

psm:BR3InletConnectionPoint a s223:InletConnectionPoint ;
    rdfs:label "BR3Inlet connection point" ;
    s223:hasMedium s223:AC-240V-60Hz .

psm:Bathroom a s223:PhysicalSpace ;
    rdfs:label "Bathroom" ;
    s223:encloses psm:HVACSpace2,
        psm:LightingSpace3,
        psm:OccupancySpace2 .

psm:BathroomInletConnectionPoint a s223:BidirectionalConnectionPoint ;
    rdfs:label "Bathroom inlet connection point" ;
    s223:hasMedium s223:Medium-Air .

psm:BathroomLightInletCP a s223:InletConnectionPoint ;
    rdfs:label "Bathroom light inlet CP" ;
    s223:cnx psm:BathroomLight1,
        psm:LightingSpace3 ;
    s223:hasMedium s223:Light-Visible .

psm:BathroomOutletConnectionPoint a s223:OutletConnectionPoint ;
    rdfs:label "Bathroom outlet connection point" ;
    s223:hasMedium s223:Medium-Air .

psm:Corridor a s223:PhysicalSpace ;
    rdfs:label "Corridor" ;
    s223:encloses psm:HVACSpace4,
        psm:HVACSpace5,
        psm:LightingSpace5,
        psm:OccupancySpace4 .

psm:CorridorInletConnectionPointK a s223:InletConnectionPoint ;
    rdfs:label "Corridor inlet connection point k" ;
    s223:hasMedium s223:Medium-Air .

psm:CorridorInletConnectionPointPO a s223:InletConnectionPoint ;
    rdfs:label "Corridor inlet connection point po" ;
    s223:hasMedium s223:Medium-Air .

psm:CorridorOutletConnectionPointB a s223:BidirectionalConnectionPoint ;
    rdfs:label "Corridor outlet connection point b" ;
    s223:hasMedium s223:Medium-Air .

psm:CorridorOutletConnectionPointOO a s223:OutletConnectionPoint ;
    rdfs:label "Corridor outlet connection point OO" ;
    s223:hasMedium s223:Medium-Air .

psm:ELightPath1 a s223:Connection ;
    rdfs:label "ELight Path1" ;
    s223:cnx psm:LightingSpace1ELInlet ;
    s223:hasMedium s223:Light-Visible .

psm:ELightPath2 a s223:Connection ;
    rdfs:label "ELight Path2" ;
    s223:cnx psm:LightingSpace2ELInlet ;
    s223:hasMedium s223:Light-Visible .

psm:ElectricCircuit3 a s223:ElectricWire ;
    rdfs:label "Electric Circuit 3" ;
    s223:hasMedium s223:AC-240V-60Hz .

psm:HVACSpace2 a s223:DomainSpace ;
    rdfs:label "HVACSpace2" ;
    s223:hasConnectionPoint psm:BathroomInletConnectionPoint,
        psm:BathroomOutletConnectionPoint ;
    s223:hasDomain s223:Domain-HVAC .

psm:HVACSpace3 a s223:DomainSpace ;
    rdfs:label "HVACSpace3" ;
    s223:hasConnectionPoint psm:PrivateOfficeInletConnectionPoint,
        psm:PrivateOfficeOutletConnectionPoint ;
    s223:hasDomain s223:Domain-HVAC .

psm:HVACSpace6 a s223:DomainSpace ;
    rdfs:label "HVACSpace6" ;
    s223:hasConnectionPoint psm:KitchenetteInletConnectionPoint,
        psm:KitchenetteOutletConnectionPoint ;
    s223:hasDomain s223:Domain-HVAC .

psm:KitchenetteInletConnectionPoint a s223:InletConnectionPoint ;
    rdfs:label "Kitchenette inlet connection point" ;
    s223:hasMedium s223:Medium-Air .

psm:KitchenetteLightInletCP a s223:InletConnectionPoint ;
    rdfs:label "Kitchenette light inlet CP" ;
    s223:hasMedium s223:Light-Visible .

psm:KitchenetteOutletConnectionPoint a s223:OutletConnectionPoint ;
    rdfs:label "Kitchenette outlet connection point" ;
    s223:hasMedium s223:Medium-Air .

psm:LightEngine1 a s223:Equipment ;
    rdfs:label "LightEngine1" ;
    s223:hasConnectionPoint psm:LightEngine1Inlet,
        psm:LightEngine1Outlet .

psm:LightEngine1Inlet a s223:InletConnectionPoint ;
    rdfs:label "Light engine1Inlet" ;
    s223:hasMedium s223:Medium-Electricity .

psm:LightingSpace1ELInlet a s223:InletConnectionPoint ;
    rdfs:label "Lighting Space1 EL Inlet" ;
    s223:hasMedium s223:Light-Visible .

psm:LightingSpace2 a s223:DomainSpace ;
    rdfs:label "LightingSpace2" ;
    s223:hasConnectionPoint psm:LightingSpace2ELInlet ;
    s223:hasDomain s223:Domain-Lighting .

psm:LightingSpace2ELInlet a s223:InletConnectionPoint ;
    rdfs:label "Lighting Space2 EL Inlet" ;
    s223:hasMedium s223:Light-Visible .

psm:LightingSpace4 a s223:DomainSpace ;
    rdfs:label "LightingSpace4" ;
    s223:cnx psm:PrivateOfficeLightInletCP ;
    s223:hasDomain s223:Domain-Lighting .

psm:LightingSpace5 a s223:DomainSpace ;
    rdfs:label "LightingSpace5" ;
    s223:cnx psm:CorridorLightInletCP ;
    s223:hasDomain s223:Domain-Lighting .

psm:LightingSpace6 a s223:DomainSpace ;
    rdfs:label "LightingSpace6" ;
    s223:hasConnectionPoint psm:KitchenetteLightInletCP ;
    s223:hasDomain s223:Domain-Lighting .

psm:Luminaire11Outlet a s223:OutletConnectionPoint ;
    rdfs:label "Luminaire11Outlet" ;
    s223:hasMedium s223:Light-Visible .

psm:Luminaire1CCT a s223:QuantifiableActuatableProperty ;
    rdfs:label "Luminaire1CCT" ;
    qudt:hasQuantityKind quantitykind:ThermodynamicTemperature ;
    qudt:unit unit:K .

psm:Luminaire1Inlet a s223:InletConnectionPoint ;
    rdfs:label "Luminaire1Inlet" .

psm:Luminaire1Intensity a s223:QuantifiableActuatableProperty ;
    rdfs:label "Luminaire1Intensity" ;
    s223:hasValue 50.5 ;
    qudt:hasQuantityKind quantitykind:LuminousFluxRatio ;
    qudt:unit unit:PERCENT .

psm:Luminaire1OnOff a s223:EnumeratedActuatableProperty ;
    rdfs:label "Luminaire1OnOff" ;
    s223:hasEnumerationKind s223:EnumerationKind-OnOff ;
    s223:hasValue s223:OnOff-Off .

psm:Luminaire1Outlet a s223:OutletConnectionPoint ;
    rdfs:label "Luminaire1Outlet" .

psm:Luminaire2CCT a s223:QuantifiableActuatableProperty ;
    rdfs:label "Luminaire2CCT" ;
    qudt:hasQuantityKind quantitykind:ThermodynamicTemperature ;
    qudt:unit unit:K .

psm:Luminaire2Intensity a s223:QuantifiableActuatableProperty ;
    rdfs:label "Luminaire2Intensity" ;
    s223:hasValue 50.5 ;
    qudt:hasQuantityKind quantitykind:LuminousFluxRatio ;
    qudt:unit unit:PERCENT .

psm:Luminaire2OnOff a s223:EnumeratedActuatableProperty ;
    rdfs:label "Luminaire2OnOff" ;
    s223:hasEnumerationKind s223:EnumerationKind-OnOff ;
    s223:hasValue s223:OnOff-Off .

psm:MainBreakerCircuit1 a s223:ElectricWire ;
    rdfs:label "Main breaker circuit1" ;
    s223:hasMedium s223:AC-120V-60Hz .

psm:MainBreakerCircuit2 a s223:ElectricWire ;
    rdfs:label "Main breaker circuit2" ;
    s223:hasMedium s223:AC-120V-60Hz .

psm:OccupancySpace1 a s223:DomainSpace ;
    rdfs:label "Occupancy space1" ;
    s223:hasDomain s223:Domain-Occupancy .

psm:OccupancySpace2 a s223:DomainSpace ;
    rdfs:label "Occupancy space2" ;
    s223:hasDomain s223:Domain-Occupancy .

psm:OccupancySpace3 a s223:DomainSpace ;
    rdfs:label "Occupancy space3" ;
    s223:hasDomain s223:Domain-Occupancy .

psm:OccupancySpace4 a s223:DomainSpace ;
    rdfs:label "Occupancy space4" ;
    s223:hasDomain s223:Domain-Occupancy .

psm:OccupancySpace5 a s223:DomainSpace ;
    rdfs:label "OccupancySpace5" ;
    s223:hasDomain s223:Domain-Occupancy .

psm:OpenOfficeInletConnectionPoint a s223:InletConnectionPoint ;
    rdfs:label "Open office inlet connection point" ;
    s223:hasMedium s223:Medium-Air .

psm:PrivateOfficeInletConnectionPoint a s223:InletConnectionPoint ;
    rdfs:label "Private office inlet connection point" ;
    s223:hasMedium s223:Medium-Air .

psm:PrivateOfficeOutletConnectionPoint a s223:OutletConnectionPoint ;
    rdfs:label "Private office outlet connection point" ;
    s223:hasMedium s223:Medium-Air .

psm:VAV1DamperInletCP a s223:InletConnectionPoint ;
    rdfs:label "VAV1Damper inlet CP" ;
    s223:hasMedium s223:Medium-Air ;
    s223:mapsTo psm:VAVBox1Inlet .

psm:VAV1DamperOutletCP a s223:OutletConnectionPoint ;
    rdfs:label "VAV1Damper outlet CP" ;
    s223:hasMedium s223:Medium-Air .

psm:VAV1InletReheatCoilCP a s223:InletConnectionPoint ;
    rdfs:label "VAV1Inlet reheat coil CP" ;
    s223:hasMedium s223:Medium-Air .

psm:VAV2DamperOutletCP a s223:OutletConnectionPoint ;
    rdfs:label "VAV2Damper outlet CP" ;
    s223:hasMedium s223:Medium-Air .

psm:VAV2InletReheatCoilCP a s223:InletConnectionPoint ;
    rdfs:label "VAV2Inlet reheat coil CP" ;
    s223:hasMedium s223:Medium-Air .

psm:VAVBox1Inlet a s223:InletConnectionPoint ;
    rdfs:label "VAVBox1Inlet" ;
    s223:hasMedium s223:Medium-Air .

psm:VAVBox1Outlet a s223:OutletConnectionPoint ;
    rdfs:label "VAVBox1Outlet" ;
    s223:hasMedium s223:Medium-Air .

psm:VAVBox2Inlet a s223:InletConnectionPoint ;
    rdfs:label "VAVBox2Inlet" ;
    s223:hasMedium s223:Medium-Air .

psm:VAVBox2Outlet a s223:OutletConnectionPoint ;
    rdfs:label "VAVBox2Outlet" ;
    s223:hasMedium s223:Medium-Air .

psm:i00006 a s223:Connection ;
    rdfs:label "A-9.outside_air" ;
    s223:cnx psm:i00009,
        psm:i00018 ;
    s223:hasMedium s223:Medium-Air ;
    s223:hasProperty psm:oatmp .

psm:i00009 a s223:InletConnectionPoint ;
    rdfs:label "A-9.min_oa_damper.airInlet" ;
    s223:cnx psm:i00006,
        psm:i00007 ;
    s223:hasMedium s223:Medium-Air .

psm:i00010 a s223:OutletConnectionPoint ;
    rdfs:label "A-9.min_oa_damper.airOutlet" ;
    s223:cnx psm:i00007,
        psm:i00015 ;
    s223:hasMedium s223:Medium-Air .

psm:i00014 a s223:OutletConnectionPoint ;
    rdfs:label "A-9.outside_air_afms.airOutlet" ;
    s223:cnx psm:i00011,
        psm:i00020 ;
    s223:hasMedium s223:Medium-Air .

psm:i00015 a s223:Connection ;
    s223:cnx psm:i00010,
        psm:i00013 ;
    s223:hasMedium s223:Medium-Air .

psm:i00018 a s223:InletConnectionPoint ;
    rdfs:label "A-9.economizer_oa_damper.airInlet" ;
    s223:cnx psm:i00006,
        psm:i00016 ;
    s223:hasMedium s223:Medium-Air ;
    s223:mapsTo psm:AHUOAInlet .

psm:i00019 a s223:OutletConnectionPoint ;
    rdfs:label "A-9.economizer_oa_damper.airOutlet" ;
    s223:cnx psm:i00016,
        psm:i00020 ;
    s223:hasMedium s223:Medium-Air .

psm:i00023 a s223:InletConnectionPoint ;
    rdfs:label "A-9.mixed_air_filter.airInlet" ;
    s223:cnx psm:i00020,
        psm:i00021 ;
    s223:hasMedium s223:Medium-Air ;
    s223:hasProperty psm:mxtmp .

psm:i00026 a s223:InletConnectionPoint ;
    rdfs:label "A-9.hot_water_coil.airInlet" ;
    s223:cnx psm:i00025,
        psm:i00035 ;
    s223:hasMedium s223:Medium-Air .

psm:i00027 a s223:OutletConnectionPoint ;
    rdfs:label "A-9.hot_water_coil.airOutlet" ;
    s223:cnx psm:i00025,
        psm:i00046 ;
    s223:hasMedium s223:Medium-Air .

psm:i00028 a s223:InletConnectionPoint ;
    rdfs:label "A-9.hot_water_coil.hotWaterInlet" ;
    s223:cnx psm:i00025,
        psm:i00034 ;
    s223:hasMedium s223:Water-HotWater .

psm:i00032 a s223:InletConnectionPoint ;
    rdfs:label "A-9.hot_water_coil.hw_valve.hotWaterInlet" ;
    s223:cnx psm:i00030 ;
    s223:hasMedium s223:Water-HotWater ;
    s223:mapsTo psm:AHUHotWaterInlet .

psm:i00033 a s223:OutletConnectionPoint ;
    rdfs:label "A-9.hot_water_coil.hw_valve.hotWaterOutlet" ;
    s223:cnx psm:i00030,
        psm:i00034 ;
    s223:hasMedium s223:Water-HotWater .

psm:i00034 a s223:Connection ;
    s223:cnx psm:i00028,
        psm:i00033 ;
    s223:hasMedium s223:Water-HotWater .

psm:i00035 a s223:Connection ;
    s223:cnx psm:i00024,
        psm:i00026 ;
    s223:hasMedium s223:Medium-Air .

psm:i00037 a s223:InletConnectionPoint ;
    rdfs:label "A-9.chilled_water_coil.airInlet" ;
    s223:cnx psm:i00036,
        psm:i00046 ;
    s223:hasMedium s223:Medium-Air .

psm:i00038 a s223:OutletConnectionPoint ;
    rdfs:label "A-9.chilled_water_coil.airOutlet" ;
    s223:cnx psm:i00036,
        psm:i00050 ;
    s223:hasMedium s223:Medium-Air .

psm:i00039 a s223:InletConnectionPoint ;
    rdfs:label "A-9.chilled_water_coil.chilledWaterSupply" ;
    s223:cnx psm:i00036,
        psm:i00045 ;
    s223:hasMedium s223:Water-ChilledWater .

psm:i00044 a s223:OutletConnectionPoint ;
    rdfs:label "A-9.chilled_water_coil.chilled_water_valve.chilledWaterOutlet" ;
    s223:cnx psm:i00041,
        psm:i00045 ;
    s223:hasMedium s223:Water-ChilledWater .

psm:i00045 a s223:Connection ;
    s223:cnx psm:i00039,
        psm:i00044 ;
    s223:hasMedium s223:Water-ChilledWater .

psm:i00048 a s223:InletConnectionPoint ;
    rdfs:label "A-9.supply_fan.airInlet" ;
    s223:cnx psm:i00047,
        psm:i00050 ;
    s223:hasMedium s223:Medium-Air .

psm:i00049 a s223:OutletConnectionPoint ;
    rdfs:label "A-9.supply_fan.airOutlet" ;
    s223:cnx psm:VAVSupply,
        psm:i00047 ;
    s223:hasMedium s223:Medium-Air ;
    s223:mapsTo psm:AHUSupplyOutlet .

psm:i00055 a s223:Connection ;
    rdfs:label "A-9.return_air" ;
    s223:cnx psm:i00053,
        psm:i00058,
        psm:i00063 ;
    s223:hasMedium s223:Medium-Air .

psm:i00058 a s223:InletConnectionPoint ;
    rdfs:label "A-9.exhaust_air_damper.airInlet" ;
    s223:cnx psm:i00055,
        psm:i00056 ;
    s223:hasMedium s223:Medium-Air .

psm:i00059 a s223:OutletConnectionPoint ;
    rdfs:label "A-9.exhaust_air_damper.airOutlet" ;
    s223:cnx psm:i00056,
        psm:i00060 ;
    s223:hasMedium s223:Medium-Air ;
    s223:mapsTo psm:AHUExhaustOutlet .

psm:i00063 a s223:InletConnectionPoint ;
    rdfs:label "A-9.return_air_damper.airInlet" ;
    s223:cnx psm:i00055,
        psm:i00061 ;
    s223:hasMedium s223:Medium-Air .

psm:i00064 a s223:OutletConnectionPoint ;
    rdfs:label "A-9.return_air_damper.airOutlet" ;
    s223:cnx psm:i00020,
        psm:i00061 ;
    s223:hasMedium s223:Medium-Air .

psm:mxtmp a s223:QuantifiableObservableProperty ;
    rdfs:label "Mixed Air Temperature" ;
    s223:hasValue 78.0 ;
    qudt:hasQuantityKind quantitykind:Temperature ;
    qudt:unit unit:DEG_F .

psm:oatmp a s223:QuantifiableObservableProperty ;
    rdfs:label "Outside Air Temperature" ;
    qudt:hasQuantityKind quantitykind:Temperature ;
    qudt:unit unit:DEG_F .

psm:ratmp a s223:QuantifiableObservableProperty ;
    rdfs:label "Return Air Temperature" ;
    qudt:hasQuantityKind quantitykind:Temperature ;
    qudt:unit unit:DEG_F .

psm:sap a s223:QuantifiableObservableProperty ;
    rdfs:label "Supply Air Pressure" ;
    s223:hasValue 15.6 ;
    qudt:hasQuantityKind quantitykind:Pressure ;
    qudt:unit unit:PSI .

g36:AirFlowStationRule a sh:NodeShape ;
    sh:class s223:Sensor ;
    sh:property [ rdfs:comment "The Air Flow Station must hasObservationLocation the Damper InletConnectionPoint." ;
            sh:class s223:InletConnectionPoint ;
            sh:maxCount 1 ;
            sh:minCount 1 ;
            sh:node [ sh:property [ sh:class s223:Damper ;
                            sh:minCount 1 ;
                            sh:path [ sh:inversePath s223:hasConnectionPoint ] ] ] ;
            sh:path s223:hasObservationLocation ],
        [ sh:class s223:Medium-Air ;
            sh:minCount 1 ;
            sh:path s223:measuresSubstance ],
        [ sh:class s223:Medium-Air ;
            sh:minCount 1 ;
            sh:path s223:measuresSubstance ] .

g36:BinaryIn a s223:Class,
        sh:NodeShape ;
    rdfs:label "Binary in" ;
    rdfs:subClassOf s223:EnumeratedObservableProperty ;
    sh:rule [ a sh:TripleRule ;
            rdfs:comment "An instance of g36:BinaryIn has a value that is a member of the EnumerationKind g36:RunStatus." ;
            sh:object g36:RunStatus ;
            sh:predicate s223:hasEnumerationKind ;
            sh:subject sh:this ] .

g36:HotWaterCoil a s223:Class,
        sh:NodeShape ;
    rdfs:label "HotWater/ReheatCoil" ;
    rdfs:subClassOf s223:HeatingCoil ;
    sh:class s223:HeatingCoil ;
    sh:property [ sh:class g36:HotWaterValve ;
            sh:comment "Valve should be contained ? " ;
            sh:minCount 1 ;
            sh:path s223:contains ;
            sh:severity s223:g36 ],
        [ rdfs:comment "The HotWaterCoil outlet connection point must map to exactly one VAV outlet connection point" ;
            sh:path s223:hasConnectionPoint ;
            sh:qualifiedMinCount 1 ;
            sh:qualifiedValueShape [ sh:class s223:OutletConnectionPoint ;
                    sh:node [ sh:property [ sh:class s223:OutletConnectionPoint ;
                                    sh:maxCount 1 ;
                                    sh:minCount 1 ;
                                    sh:node [ sh:property [ sh:class g36:VAVWithReheat ;
                                                    sh:minCount 1 ;
                                                    sh:path [ sh:inversePath s223:hasConnectionPoint ] ] ] ;
                                    sh:path s223:mapsTo ] ] ] ],
        [ sh:class g36:HotWaterValve ;
            sh:comment "Must have Valve Connected." ;
            sh:minCount 1 ;
            sh:path [ sh:alternativePath ( s223:connectedFrom s223:connectedTo ) ] ;
            sh:severity s223:g36 ] ;
    sh:severity s223:g36 .

g36:HotWaterValve a s223:Class,
        sh:NodeShape ;
    rdfs:label "Hot Water Valve" ;
    rdfs:subClassOf s223:Valve ;
    sh:class s223:Valve ;
    sh:property [ rdfs:comment "HW Valve Signal. Add Aspects to this?" ;
            sh:minCount 1 ;
            sh:path s223:hasProperty ;
            sh:qualifiedMinCount 1 ;
            sh:qualifiedValueShape [ sh:class g36:AnalogOut ;
                    sh:node [ sh:property [ sh:hasValue s223:QuantityKind-RelativePosition ;
                                    sh:path qudt:hasQuantityKind ] ] ] ] .

sh:qualifiedValueShape a rdf:Property ;
    rdfs:label "qualified value shape"@en ;
    rdfs:comment "The shape that a specified number of values must conform to."@en ;
    rdfs:isDefinedBy sh: ;
    rdfs:range sh:Shape .

sh:qualifiedValueShapesDisjoint a rdf:Property ;
    rdfs:label "qualified value shapes disjoint"@en ;
    rdfs:comment "Can be used to mark the qualified value shape to be disjoint with its sibling shapes."@en ;
    rdfs:isDefinedBy sh: ;
    rdfs:range xsd:boolean .

s223:Attribute-DayOfWeek a s223:Attribute-DayOfWeek,
        s223:Class,
        sh:NodeShape ;
    rdfs:label "Day of Week" ;
    rdfs:comment "This class has enumerated instances of Monday, Tuesday, Wednesday, Thursday, Friday, Saturday and Sunday. The Weekend and Weekday EnumerationKinds define subsets of this EnumerationKind for Mon-Fri and Sat,Sun, respectively" ;
    rdfs:subClassOf s223:Context-Attribute .

s223:Coil a s223:Class,
        sh:NodeShape ;
    rdfs:label "Coil" ;
    rdfs:comment "A cooling or heating element made of pipe or tube that may or may not be finned and formed into helical or serpentine shape." ;
    rdfs:subClassOf s223:HeatExchanger ;
    sh:property [ rdfs:comment "A Coil shall have at least one inlet using the medium Air." ;
            sh:path s223:hasConnectionPoint ;
            sh:qualifiedMinCount 1 ;
            sh:qualifiedValueShape [ sh:class s223:InletConnectionPoint ;
                    sh:node [ sh:property [ sh:class s223:Medium-Air ;
                                    sh:path s223:hasMedium ] ] ] ],
        [ rdfs:comment "A Coil shall have at least one outlet using the medium Air." ;
            sh:path s223:hasConnectionPoint ;
            sh:qualifiedMinCount 1 ;
            sh:qualifiedValueShape [ sh:class s223:OutletConnectionPoint ;
                    sh:node [ sh:property [ sh:class s223:Medium-Air ;
                                    sh:path s223:hasMedium ] ] ] ] .

s223:DayOfWeek-Weekend a s223:Class,
        s223:DayOfWeek-Weekend,
        sh:NodeShape ;
    rdfs:label "Day of week-Weekend",
        "Weekend" ;
    rdfs:comment "This class defines the EnumerationKind values of Saturday and Sunday" ;
    rdfs:subClassOf s223:Attribute-DayOfWeek .

s223:Dimensioned-Frequency a s223:Class,
        s223:Dimensioned-Frequency,
        sh:NodeShape ;
    rdfs:label "Dimensioned Frequency" ;
    rdfs:subClassOf s223:Context-Dimensioned .

s223:Dimensionless-NumberOfElectricalPhases a s223:Class,
        s223:Dimensionless-NumberOfElectricalPhases,
        sh:NodeShape ;
    rdfs:label "Dimensionless Number of Electrical Phases" ;
    rdfs:subClassOf s223:Context-Dimensionless .

s223:Filter a s223:Class,
        sh:NodeShape ;
    rdfs:label "Filter" ;
    rdfs:comment "A device that removes contaminates from gases or liquids." ;
    rdfs:subClassOf s223:Equipment ;
    sh:property [ rdfs:comment "A Filter shall have at least one inlet." ;
            sh:path s223:hasConnectionPoint ;
            sh:qualifiedMinCount 1 ;
            sh:qualifiedValueShape [ sh:class s223:InletConnectionPoint ] ],
        [ rdfs:comment "A Filter shall have at least one outlet." ;
            sh:path s223:hasConnectionPoint ;
            sh:qualifiedMinCount 1 ;
            sh:qualifiedValueShape [ sh:class s223:OutletConnectionPoint ] ],
        [ sh:minCount 2 ;
            sh:path s223:hasConnectionPoint ] .

s223:FlowSensor a s223:Class,
        sh:NodeShape ;
    rdfs:label "Flow sensor" ;
    rdfs:comment "A FlowSensor is a specialization of a Sensor that produces an ObservableProperty that is quantifiable and represents a flow measurement." ;
    rdfs:subClassOf s223:Sensor .

s223:LightSensor a s223:Class,
        sh:NodeShape ;
    rdfs:label "Light sensor" ;
    rdfs:comment "A LightSensor is a specialization of a Sensor that observes a QuantifiableObservableProperty that represents a luminance measurement." ;
    rdfs:subClassOf s223:Sensor .

s223:LineNeutralVoltage-1.73kV a s223:Dimensioned-LineNeutralVoltage ;
    rdfs:label "1.73kV Line-Neutral Voltage" ;
    s223:hasVoltage s223:Voltage-1.73kV .

s223:LineNeutralVoltage-1.91kV a s223:Dimensioned-LineNeutralVoltage ;
    rdfs:label "1.91kV Line-Neutral Voltage" ;
    s223:hasVoltage s223:Voltage-1.91kV .

s223:LineNeutralVoltage-110.0V a s223:Dimensioned-LineNeutralVoltage ;
    rdfs:label "110.0V Line-Neutral Voltage" ;
    s223:hasVoltage s223:Voltage-110.0V .

s223:LineNeutralVoltage-127.0V a s223:Dimensioned-LineNeutralVoltage ;
    rdfs:label "127.0V Line-Neutral Voltage" ;
    s223:hasVoltage s223:Voltage-127.0V .

s223:LineNeutralVoltage-139.0V a s223:Dimensioned-LineNeutralVoltage ;
    rdfs:label "139.0V Line-Neutral Voltage" ;
    s223:hasVoltage s223:Voltage-139.0V .

s223:LineNeutralVoltage-2.4kV a s223:Dimensioned-LineNeutralVoltage ;
    rdfs:label "2.4kV Line-Neutral Voltage" ;
    s223:hasVoltage s223:Voltage-2.4kV .

s223:LineNeutralVoltage-219.0V a s223:Dimensioned-LineNeutralVoltage ;
    rdfs:label "219.0V Line-Neutral Voltage" ;
    s223:hasVoltage s223:Voltage-219.0V .

s223:LineNeutralVoltage-231.0V a s223:Dimensioned-LineNeutralVoltage ;
    rdfs:label "231.0V Line-Neutral Voltage" ;
    s223:hasVoltage s223:Voltage-231.0V .

s223:LineNeutralVoltage-240.0V a s223:Dimensioned-LineNeutralVoltage ;
    rdfs:label "240.0V Line-Neutral Voltage" ;
    s223:hasVoltage s223:Voltage-240.0V .

s223:LineNeutralVoltage-277.0V a s223:Dimensioned-LineNeutralVoltage ;
    rdfs:label "277.0V Line-Neutral Voltage" ;
    s223:hasVoltage s223:Voltage-277.0V .

s223:LineNeutralVoltage-3.46kV a s223:Dimensioned-LineNeutralVoltage ;
    rdfs:label "3.46kV Line-Neutral Voltage" ;
    s223:hasVoltage s223:Voltage-3.46kV .

s223:LineNeutralVoltage-3.81kV a s223:Dimensioned-LineNeutralVoltage ;
    rdfs:label "3.81kV Line-Neutral Voltage" ;
    s223:hasVoltage s223:Voltage-3.81kV .

s223:LineNeutralVoltage-347.0V a s223:Dimensioned-LineNeutralVoltage ;
    rdfs:label "347.0V Line-Neutral Voltage" ;
    s223:hasVoltage s223:Voltage-347.0V .

s223:LineNeutralVoltage-5.77kV a s223:Dimensioned-LineNeutralVoltage ;
    rdfs:label "5.77kV Line-Neutral Voltage" ;
    s223:hasVoltage s223:Voltage-5.77kV .

s223:ObservableProperty a s223:Class,
        sh:NodeShape ;
    rdfs:label "Observable Property" ;
    rdfs:comment "This class describes non-numeric properties of which real-time value cannot be modified by a user or a machine outside of the model. Sensors reading are typically observable properties as their value naturally fluctuate, but is not meant to be modified by a user." ;
    rdfs:subClassOf s223:Property .

s223:OccupancySensor a s223:Class,
        sh:NodeShape ;
    rdfs:label "Occupancy sensor" ;
    rdfs:comment "An OccuppancySensor is a specialization of a Sensor that observes a Property that represents measurement of occupancy in a space." ;
    rdfs:subClassOf s223:Sensor .

s223:OnOff-On a s223:EnumerationKind-OnOff ;
    rdfs:label "On" .

s223:Signal-Modulated a s223:Class,
        s223:Signal-Modulated,
        sh:NodeShape ;
    rdfs:label "Signal-Modulated" ;
    rdfs:subClassOf s223:Electricity-Signal .

s223:SymmetricProperty a s223:Class,
        sh:NodeShape ;
    rdfs:label "Symmetric property" ;
    rdfs:comment "Symmetric properties used to associate adjacent entities. See s223:cnx, s223:connected, s223:lnx" ;
    rdfs:subClassOf rdf:Property .

s223:Water-GlycolSolution a s223:Class,
        s223:Water-GlycolSolution,
        sh:NodeShape ;
    rdfs:label "Water-GlycolSolution" ;
    s223:hasProperty [ a s223:QuantifiableProperty ;
            rdfs:label "Unspecified" ;
            s223:hasAspect s223:Medium-Glycol ;
            qudt:hasQuantityKind quantitykind:VolumeFraction ;
            qudt:hasUnit unit:PERCENT ],
        [ a s223:QuantifiableProperty ;
            rdfs:label "Unspecified" ;
            s223:hasAspect s223:Medium-Water ;
            qudt:hasQuantityKind quantitykind:VolumeFraction ;
            qudt:hasUnit unit:PERCENT ] ;
    rdfs:subClassOf s223:Medium-Water ;
    sh:property [ rdfs:comment "The water percentage." ;
            sh:path s223:hasProperty ;
            sh:qualifiedMinCount 1 ;
            sh:qualifiedValueShape [ sh:class s223:QuantifiableProperty ;
                    sh:node [ sh:property [ s223:hasAspect s223:Medium-Water ;
                                    sh:hasValue quantitykind:VolumeFraction ;
                                    sh:path qudt:hasQuantityKind ] ] ] ],
        [ rdfs:comment "The glycol percentage." ;
            sh:path s223:hasProperty ;
            sh:qualifiedMinCount 1 ;
            sh:qualifiedValueShape [ sh:class s223:QuantifiableProperty ;
                    sh:node [ sh:property [ s223:hasAspect s223:Medium-Glycol ;
                                    sh:hasValue quantitykind:VolumeFraction ;
                                    sh:path qudt:hasQuantityKind ] ] ] ] .

s223:connected a s223:SymmetricProperty,
        rdf:Property ;
    rdfs:label "connected" ;
    rdfs:comment "The relation connected indicates that two connectable things are connected without regard to any directionality of a process flow.  " .

s223:isConnectionPointOf a rdf:Property ;
    rdfs:label "is connection point of" ;
    s223:inverseOf s223:hasConnectionPoint ;
    rdfs:comment "The relation isConnectionPointOf is part of a pair of relations that bind a ConnectionPoint to a Connectable thing. It is the inverse of the relation hasConnectionPoint (see `s223:hasConnectionPoint`)." .

s223:lnx a s223:SymmetricProperty ;
    rdfs:label "lnx" ;
    rdfs:comment "The lnx property is a symmetric property associating adjacent entities in a Segment-Junction Network." .

s223:ofSubstance a rdf:Property ;
    rdfs:label "of substance" .

s223:uses a rdf:Property ;
    rdfs:label "uses" ;
    rdfs:comment "The relation uses is used to relate a function block input (see `s223:FunctionInput`) to a property (see `s223:Property`). This allows one to specify that the value of this property is used by the function block. " .

psm:BathroomLight1 a s223:Connection ;
    rdfs:label "Bathroom light1" ;
    s223:cnx psm:BathroomLightInletCP ;
    s223:hasMedium s223:Light-Visible .

psm:CorridorLight1 a s223:Connection ;
    rdfs:label "Corridor light1" ;
    s223:hasMedium s223:Light-Visible .

psm:HVACSpace1 a s223:DomainSpace ;
    rdfs:label "HVACSpace1" ;
    s223:hasConnectionPoint psm:OpenOfficeInletConnectionPoint,
        psm:OpenOfficeOutletConnectionPoint ;
    s223:hasDomain s223:Domain-HVAC .

psm:HVACSpace4 a s223:DomainSpace ;
    rdfs:label "HVACSpace4" ;
    s223:hasConnectionPoint psm:CorridorInletConnectionPointPO,
        psm:CorridorOutletConnectionPointB,
        psm:CorridorOutletConnectionPointOO ;
    s223:hasDomain s223:Domain-HVAC .

psm:HVACSpace5 a s223:DomainSpace ;
    rdfs:label "HVACSpace5" ;
    s223:hasConnectionPoint psm:CorridorInletConnectionPointK,
        psm:OutletIntraCorridor5CP ;
    s223:hasDomain s223:Domain-HVAC .

psm:Kitchenette a s223:PhysicalSpace ;
    rdfs:label "Kitchenette" ;
    s223:encloses psm:HVACSpace6,
        psm:LightingSpace6,
        psm:OccupancySpace5 .

psm:LightingSpace1 a s223:DomainSpace ;
    rdfs:label "LightingSpace1" ;
    s223:hasConnectionPoint psm:LIghtingSpace1DLInlet,
        psm:LightingSpace1ELInlet ;
    s223:hasDomain s223:Domain-Lighting .

psm:LightingSpace3 a s223:DomainSpace ;
    rdfs:label "LightingSpace3" ;
    s223:hasConnectionPoint psm:BathroomLightInletCP ;
    s223:hasDomain s223:Domain-Lighting .

psm:OccupancyProp1 a s223:QuantifiableObservableProperty ;
    rdfs:label "Occupancy prop1" ;
    s223:hasValue 5.0 ;
    qudt:hasQuantityKind quantitykind:Population ;
    qudt:unit unit:NUM .

psm:OpenOfficeDaylightLevel a s223:QuantifiableObservableProperty ;
    rdfs:label "Open office daylight level" ;
    qudt:hasQuantityKind quantitykind:Illuminance ;
    qudt:unit unit:LUX .

psm:PrivateOfficeLight1 a s223:Connection ;
    rdfs:label "Private office light1" ;
    s223:hasMedium s223:Light-Visible .

psm:VAV1OuletReheatCoilCP a s223:OutletConnectionPoint ;
    rdfs:label "VAV1Oulet reheat coil CP" ;
    s223:hasMedium s223:Medium-Air ;
    s223:mapsTo psm:VAVBox1Outlet .

psm:VAV2OuletReheatCoilCP a s223:OutletConnectionPoint ;
    rdfs:label "VAV2Oulet reheat coil CP" ;
    s223:hasMedium s223:Medium-Air ;
    s223:mapsTo psm:VAVBox2Outlet .

psm:i00013 a s223:InletConnectionPoint ;
    rdfs:label "A-9.outside_air_afms.airInlet" ;
    s223:cnx psm:i00011,
        psm:i00015 ;
    s223:hasMedium s223:Medium-Air .

psm:i00024 a s223:OutletConnectionPoint ;
    rdfs:label "A-9.mixed_air_filter.airOutlet" ;
    s223:cnx psm:i00021,
        psm:i00035 ;
    s223:hasMedium s223:Medium-Air .

psm:i00030 a s223:Valve ;
    rdfs:label "A-9.hot_water_coil.hw_valve" ;
    s223:cnx psm:i00032,
        psm:i00033 ;
    s223:hasProperty psm:i00031 .

psm:i00041 a s223:Valve ;
    rdfs:label "A-9.chilled_water_coil.chilled_water_valve" ;
    s223:cnx psm:i00043,
        psm:i00044 ;
    s223:hasProperty psm:i00042 .

psm:i00046 a s223:Connection ;
    s223:cnx psm:i00027,
        psm:i00037 ;
    s223:hasMedium s223:Medium-Air .

psm:i00050 a s223:Connection ;
    s223:cnx psm:i00038,
        psm:i00048 ;
    s223:hasMedium s223:Medium-Air .

psm:i00052 a s223:InletConnectionPoint ;
    rdfs:label "A-9.return_fan.airInlet" ;
    s223:cnx psm:i00051 ;
    s223:hasMedium s223:Medium-Air ;
    s223:mapsTo psm:AHUReturnInlet .

psm:i00053 a s223:OutletConnectionPoint ;
    rdfs:label "A-9.return_fan.airOutlet" ;
    s223:cnx psm:i00051 ;
    s223:hasMedium s223:Medium-Air .

psm:i00061 a s223:MotorizedDamper ;
    rdfs:label "A-9.return_air_damper" ;
    s223:cnx psm:i00063,
        psm:i00064 ;
    s223:hasProperty psm:i00062 .

g36:VAVWithReheat a s223:Class,
        sh:NodeShape ;
    rdfs:label "VAV with Reheat" ;
    rdfs:subClassOf g36:VAV ;
    sh:property [ sh:path s223:contains ;
            sh:qualifiedMaxCount 1 ;
            sh:qualifiedMinCount 1 ;
            sh:qualifiedValueShape [ sh:class g36:HotWaterCoil ] ;
            sh:qualifiedValueShapesDisjoint true ;
            sh:severity s223:g36 ],
        [ rdfs:comment "Temperature property should be at the outlet of the equipment or a connection point that maps to the outlet",
                "Temperature sensor has measurement location at Outlet of hot water coil or VAV" ;
            sh:minCount 1 ;
            sh:path s223:hasConnectionPoint ;
            sh:qualifiedMinCount 1 ;
            sh:qualifiedValueShape [ sh:class s223:OutletConnectionPoint ;
                    sh:node [ sh:property [ sh:hasValue quantitykind:Temperature ;
                                    sh:path ( [ sh:zeroOrMorePath [ sh:inversePath s223:mapsTo ] ] s223:hasProperty qudt:hasQuantityKind ) ] ] ] ;
            sh:severity s223:g36 ] .

g36:Zone a s223:Class,
        sh:Nodeshape ;
    rdfs:label "Zone with relevant points" ;
    rdfs:subClassOf s223:Zone ;
    sh:node g36:ZoneRule .

qudt:hasUnit rdfs:comment "A reference to the unit of measure of a QuantifiableProperty of interest." .

sh:Warning a sh:Severity ;
    rdfs:label "Warning"@en ;
    rdfs:comment "The severity for a warning validation result."@en ;
    rdfs:isDefinedBy sh: .

s223:ActuatableProperty a s223:Class,
        sh:NodeShape ;
    rdfs:label "Actuatable Property" ;
    rdfs:comment "This class describes non-numeric properties of which real-time value can be modified by a user or a machine outside of the model." ;
    rdfs:subClassOf s223:Property .

s223:BidirectionalConnectionPoint a s223:Class,
        sh:NodeShape ;
    rdfs:label "Bidirectional Connection Point" ;
    rdfs:comment "A BidirectionalConnectionPoint is a predefined subclass of ConnectionPoint. Using a BidirectionalConnectionPoint implies that the flow direction is not fixed in one direction. It depends on the status of some other part of the system, such as a valve position, that is expected to change during operation (see `s223:Direction-Bidirectional`) or to model energy transfer occurring without specific flow direction." ;
    rdfs:subClassOf s223:ConnectionPoint .

s223:EnumerationKind-Binary a s223:Class,
        s223:EnumerationKind-Binary,
        sh:NodeShape ;
    rdfs:label "EnumerationKind Binary" ;
    rdfs:comment "This class has enumerated instances of True, False and Unknown used to describe the possible values of a binary property" ;
    rdfs:subClassOf s223:EnumerationKind .

s223:EnumerationKind-Context a s223:Class,
        s223:EnumerationKind-Context,
        sh:NodeShape ;
    rdfs:label "EnumerationKind-Context" ;
    rdfs:comment "This class has enumerated instances to specify contexts used with the s223:hasAspect relation for a s223:Property." ;
    rdfs:subClassOf s223:EnumerationKind .

s223:EnumerationKind-Direction a s223:Class,
        s223:EnumerationKind-Direction,
        sh:NodeShape ;
    rdfs:label "Direction" ;
    rdfs:comment "This class has enumerated instances of Bidirectional, Inlet and Outlet used to qualify ConnectionPoints." ;
    rdfs:subClassOf s223:EnumerationKind .

s223:EnumerationKind-PositionStatus a s223:Class,
        s223:EnumerationKind-PositionStatus,
        sh:NodeShape ;
    rdfs:label "Position status" ;
    rdfs:subClassOf s223:EnumerationKind .

s223:EnumerationKind-RunStatus a s223:Class,
        s223:EnumerationKind-RunStatus,
        sh:NodeShape ;
    rdfs:label "Run status" ;
    rdfs:subClassOf s223:EnumerationKind .

s223:LineLineVoltage-10.0kV a s223:Dimensioned-LineLineVoltage ;
    rdfs:label "10.0kV Line-Line Voltage" ;
    s223:hasVoltage s223:Voltage-10.0kV .

s223:LineLineVoltage-190.0V a s223:Dimensioned-LineLineVoltage ;
    rdfs:label "190.0V Line-Line Voltage" ;
    s223:hasVoltage s223:Voltage-190.0V .

s223:LineLineVoltage-208.0V a s223:Dimensioned-LineLineVoltage ;
    rdfs:label "208.0V Line-Line Voltage" ;
    s223:hasVoltage s223:Voltage-208.0V .

s223:LineLineVoltage-220.0V a s223:Dimensioned-LineLineVoltage ;
    rdfs:label "220.0V Line-Line Voltage" ;
    s223:hasVoltage s223:Voltage-220.0V .

s223:LineLineVoltage-3.0kV a s223:Dimensioned-LineLineVoltage ;
    rdfs:label "3.0kV Line-Line Voltage" ;
    s223:hasVoltage s223:Voltage-3.0kV .

s223:LineLineVoltage-3.3kV a s223:Dimensioned-LineLineVoltage ;
    rdfs:label "3.3kV Line-Line Voltage" ;
    s223:hasVoltage s223:Voltage-3.3kV .

s223:LineLineVoltage-380.0V a s223:Dimensioned-LineLineVoltage ;
    rdfs:label "380.0V Line-Line Voltage" ;
    s223:hasVoltage s223:Voltage-380.0V .

s223:LineLineVoltage-4.16kV a s223:Dimensioned-LineLineVoltage ;
    rdfs:label "4.16kV Line-Line Voltage" ;
    s223:hasVoltage s223:Voltage-4.16kV .

s223:LineLineVoltage-400.0V a s223:Dimensioned-LineLineVoltage ;
    rdfs:label "400.0V Line-Line Voltage" ;
    s223:hasVoltage s223:Voltage-400.0V .

s223:LineLineVoltage-415.0V a s223:Dimensioned-LineLineVoltage ;
    rdfs:label "415.0V Line-Line Voltage" ;
    s223:hasVoltage s223:Voltage-415.0V .

s223:LineLineVoltage-480.0V a s223:Dimensioned-LineLineVoltage ;
    rdfs:label "480.0V Line-Line Voltage" ;
    s223:hasVoltage s223:Voltage-480.0V .

s223:LineLineVoltage-6.0kV a s223:Dimensioned-LineLineVoltage ;
    rdfs:label "6.0kV Line-Line Voltage" ;
    s223:hasVoltage s223:Voltage-6.0kV .

s223:LineLineVoltage-6.6kV a s223:Dimensioned-LineLineVoltage ;
    rdfs:label "6.6kV Line-Line Voltage" ;
    s223:hasVoltage s223:Voltage-6.6kV .

s223:LineLineVoltage-600.0V a s223:Dimensioned-LineLineVoltage ;
    rdfs:label "600.0V Line-Line Voltage" ;
    s223:hasVoltage s223:Voltage-600.0V .

s223:Medium-EM a s223:Class,
        s223:Medium-EM,
        sh:NodeShape ;
    rdfs:label "Electromagnetic Wave" ;
    rdfs:subClassOf s223:EnumerationKind-Medium .

s223:Medium-Glycol a s223:EnumerationKind-Medium ;
    rdfs:label "Medium-Glycol" .

s223:Role-Cooling a s223:EnumerationKind-Role ;
    rdfs:label "Role-Cooling" .

s223:TerminalUnit a s223:Class,
        sh:NodeShape ;
    rdfs:label "Terminal Unit" ;
    rdfs:comment "An air terminal that modulates the volume of air delivered to a space." ;
    rdfs:subClassOf s223:Equipment ;
    sh:property [ rdfs:comment "A TerminalUnit shall have at least one inlet ConnectionPoint using the medium Air." ;
            sh:path s223:hasConnectionPoint ;
            sh:qualifiedMinCount 1 ;
            sh:qualifiedValueShape [ sh:class s223:InletConnectionPoint ;
                    sh:node [ sh:property [ sh:class s223:Medium-Air ;
                                    sh:path s223:hasMedium ] ] ] ],
        [ rdfs:comment "A TerminalUnit shall have at least one outlet ConnectionPoint using the medium Air." ;
            sh:minCount 2 ;
            sh:path s223:hasConnectionPoint ;
            sh:qualifiedMinCount 1 ;
            sh:qualifiedValueShape [ sh:class s223:OutletConnectionPoint ;
                    sh:node [ sh:property [ sh:class s223:Medium-Air ;
                                    sh:path s223:hasMedium ] ] ] ] .

s223:connectsAt a rdf:Property ;
    rdfs:label "connects at" ;
    s223:inverseOf s223:connectsThrough ;
    rdfs:comment "The connectsAt relation binds a Connection to a specific ConnectionPoint. See Figure x.y." .

s223:connectsThrough a rdf:Property ;
    rdfs:label "connects through" ;
    s223:inverseOf s223:connectsAt ;
    rdfs:comment "The relation connectedThrough binds a Connectable thing to a Connection without regard to the direction of flow. It is used to discover what connection links two connectable things." .

s223:hasObservationLocationLow a rdf:Property ;
    rdfs:label "has observation location low" ;
    rdfs:comment "The relation hasObservationLocationLow associates a differential sensor to one of the topological locations where a differential property is observed (see `s223:observes`)." ;
    rdfs:subPropertyOf s223:hasObservationLocation .

s223:hasValue a rdf:Property ;
    rdfs:label "hasValue" ;
    rdfs:comment "hasValue is used to contain a fixed value that is part of a 223 model, rather than a computed, measured, or externally derived variable." .

s223:measuresSubstance a rdf:Property ;
    rdfs:label "measures Substance" ;
    rdfs:comment "The relation measuresSubstance is used to relate a sensor (see `s223:Sensor`) to a substance (see `s223:EnumerationKind-Substance`). Some sensors measure a specific property inside a medium and this substance can be defined by relating the sensor to it using the relation measuresSubstance (ex. Substance-CO2 in Medium-Air). " .

psm:OpenOffice a s223:PhysicalSpace ;
    rdfs:label "Open office" ;
    s223:encloses psm:HVACSpace1,
        psm:LightingSpace1,
        psm:LightingSpace2,
        psm:OccupancySpace1 .

psm:VAV2DamperInletCP a s223:InletConnectionPoint ;
    rdfs:label "VAV2Damper inlet CP" ;
    s223:hasMedium s223:Medium-Air ;
    s223:mapsTo psm:VAVBox2Inlet .

psm:i00007 a s223:MotorizedDamper ;
    rdfs:label "A-9.min_oa_damper" ;
    s223:cnx psm:i00009,
        psm:i00010 ;
    s223:hasProperty psm:i00008 .

psm:i00011 a s223:Equipment ;
    rdfs:label "A-9.outside_air_afms" ;
    s223:cnx psm:i00013,
        psm:i00014 ;
    s223:hasProperty psm:i00012 .

psm:i00016 a s223:MotorizedDamper ;
    rdfs:label "A-9.economizer_oa_damper" ;
    s223:cnx psm:i00018,
        psm:i00019 ;
    s223:hasProperty psm:i00017 .

psm:i00020 a s223:Connection ;
    rdfs:label "A-9.mixed_air" ;
    s223:cnx psm:i00014,
        psm:i00019,
        psm:i00023,
        psm:i00064 ;
    s223:hasMedium s223:Medium-Air .

psm:i00021 a s223:Equipment,
        s223:Filter ;
    rdfs:label "A-9.mixed_air_filter" ;
    s223:cnx psm:i00023,
        psm:i00024 ;
    s223:hasProperty psm:i00022 .

psm:i00047 a s223:Fan ;
    rdfs:label "A-9.supply_fan" ;
    s223:cnx psm:i00048,
        psm:i00049 ;
    s223:hasConnectionPoint psm:SupplyFanElectricInCP ;
    s223:hasProperty psm:SupplyFanStatus .

psm:i00051 a s223:Fan ;
    rdfs:label "A-9.return_fan" ;
    s223:cnx psm:i00052,
        psm:i00053 ;
    s223:hasProperty psm:ReturnFanStatus .

psm:i00056 a s223:MotorizedDamper ;
    rdfs:label "A-9.exhaust_air_damper" ;
    s223:cnx psm:i00058,
        psm:i00059 ;
    s223:hasProperty psm:i00057 .

g36:RunCommand a s223:Class,
        g36:RunCommand,
        sh:NodeShape ;
    rdfs:label "Run command" ;
    rdfs:subClassOf s223:EnumerationKind .

g36:VAV a s223:Class,
        sh:NodeShape ;
    rdfs:label "VAV" ;
    rdfs:subClassOf s223:SingleDuctTerminal ;
    sh:node g36:VAVRule .

s223:Domain-Occupancy a s223:EnumerationKind-Domain ;
    rdfs:label "Domain-Occupancy" ;
    rdfs:comment "The domain Occupancy represents equipment used to determine if people are present in a space or count the number of people in a space." .

s223:EnumerationKind-ThreeSpeedSetting a s223:Class,
        s223:EnumerationKind-ThreeSpeedSetting,
        sh:NodeShape ;
    rdfs:label "Three speed setting" ;
    rdfs:subClassOf s223:EnumerationKind .

s223:Fan a s223:Class,
        sh:NodeShape ;
    rdfs:label "Fan" ;
    rdfs:comment "A machine used to create flow within a gas such as air. " ;
    rdfs:subClassOf s223:Equipment ;
    sh:property [ rdfs:comment "A Fan shall have at least one inlet using the medium Air." ;
            sh:path s223:hasConnectionPoint ;
            sh:qualifiedMinCount 1 ;
            sh:qualifiedValueShape [ sh:class s223:InletConnectionPoint ;
                    sh:node [ sh:property [ sh:class s223:Medium-Air ;
                                    sh:path s223:hasMedium ] ] ] ],
        [ rdfs:comment "A Fan shall have at least one outlet using the medium Air." ;
            sh:path s223:hasConnectionPoint ;
            sh:qualifiedMinCount 1 ;
            sh:qualifiedValueShape [ sh:class s223:OutletConnectionPoint ;
                    sh:node [ sh:property [ sh:class s223:Medium-Air ;
                                    sh:path s223:hasMedium ] ] ] ],
        [ sh:minCount 2 ;
            sh:path s223:hasConnectionPoint ] .

s223:FunctionInput a s223:Class,
        sh:NodeShape ;
    rdfs:label "Input" ;
    rdfs:comment "A Function Input is an input to a Function Block. It can be related to a property by s223:uses." ;
    rdfs:subClassOf s223:Concept ;
    sh:property [ rdfs:comment "An instance of Input must be associated with one Property instance using the relation 'uses'." ;
            sh:class s223:Property ;
            sh:maxCount 1 ;
            sh:message "This Function Input must be associated with exactly one property by s223:uses predicate." ;
            sh:minCount 1 ;
            sh:path s223:uses ],
        [ sh:class s223:FunctionBlock ;
            sh:maxCount 1 ;
            sh:message "This Input must be associated with exactly one FunctionBlock." ;
            sh:minCount 1 ;
            sh:path [ sh:inversePath s223:hasInput ] ] .

s223:HeatingCoil a s223:Class,
        sh:NodeShape ;
    rdfs:label "Heating coil" ;
    rdfs:subClassOf s223:Coil ;
    sh:property [ rdfs:comment "A heating coil must be related to the role 'Role-Heating' using the relation 'hasRole'." ;
            sh:hasValue s223:Role-Heating ;
            sh:minCount 1 ;
            sh:path s223:hasRole ] ;
    sh:rule [ a sh:TripleRule ;
            rdfs:comment "Heating coils will always have the role Role-Heating" ;
            sh:object s223:Role-Heating ;
            sh:predicate s223:hasRole ;
            sh:subject sh:this ] .

s223:Medium-Refrigerant a s223:Class,
        s223:Medium-Refrigerant,
        sh:NodeShape ;
    rdfs:label "Medium-Refrigerant" ;
    rdfs:subClassOf s223:EnumerationKind-Medium .

s223:Segment a s223:Class,
        sh:NodeShape ;
    rdfs:label "Segment" ;
    rdfs:comment "When necessary, a Connection may be subdivided into a network of Segments, joined at Junctions. This can be useful for identifying a duct segment of a duct before a split, for example." ;
    rdfs:subClassOf s223:Concept ;
    sh:property [ rdfs:comment "A Segment must be associated with two Junctions or ConnectionPoints using the relation lnx" ;
            sh:maxCount 2 ;
            sh:message "Segment is missing one or both endpoints (Junction or ConnectionPoint)" ;
            sh:minCount 2 ;
            sh:or ( [ sh:class s223:Junction ] [ sh:class s223:ConnectionPoint ] ) ;
            sh:path s223:lnx ;
            sh:qualifiedMaxCount 1 ;
            sh:qualifiedValueShape [ sh:class s223:ConnectionPoint ] ;
            sh:severity sh:Warning ] .

s223:Substance-Particulate a s223:Class,
        s223:Substance-Particulate,
        sh:NodeShape ;
    rdfs:label "Particulate" ;
    rdfs:subClassOf s223:EnumerationKind-Substance .

s223:System a s223:Class,
        sh:NodeShape ;
    rdfs:label "System" ;
    rdfs:comment "A System is a logical grouping (collection) of Equipment for some functional or system reason, such as a chilled water system, or HVAC system. A System does not participate in Connections." ;
    rdfs:subClassOf s223:Concept ;
    sh:property [ a sh:PropertyShape ;
            rdfs:comment "A System can be associated with zero or any number of other instances of Equipment or System using the relation hasMember" ;
            sh:minCount 0 ;
            sh:or ( [ sh:class s223:Equipment ] [ sh:class s223:System ] ) ;
            sh:path s223:hasMember ],
        [ rdfs:comment "A System can be associated with any number of EnumerationKind-Roles using the relation hasRole" ;
            sh:class s223:EnumerationKind-Role ;
            sh:path s223:hasRole ] .

s223:connectedFrom a rdf:Property ;
    rdfs:label "connected from" ;
    s223:inverseOf s223:connectedTo ;
    rdfs:comment "The relation connectedFrom means that connectable things are connected with a specific flow direction. B is connectedFrom A, means a directionality beginning at A and ending at B.  The inverse direction is indicated by connectedTo (see `s223:connectedTo`)." ;
    rdfs:domain s223:Equipment .

s223:hasEnumerationKind a rdf:Property ;
    rdfs:label "has enumeration kind" ;
    rdfs:comment "The relation hasEnumerationKind associates an EnumerableProperty with a class of enumeration values. This is used to, for example, identify what kind of substance is transported along a Connection or which day of the week a setpoint is active" .

s223:hasObservationLocationHigh a rdf:Property ;
    rdfs:label "has observation location high" ;
    rdfs:comment "The relation hasObservationLocationHigh associates a differential sensor to one of the topological locations where a differential property is observed (see `s223:observes`)." ;
    rdfs:subPropertyOf s223:hasObservationLocation .

psm:ElectricCircuit1 a s223:ElectricWire ;
    rdfs:label "Electric Circuit 1" ;
    s223:hasMedium s223:AC-120V-60Hz .

g36:RunStatus a s223:Class,
        g36:RunStatus,
        sh:NodeShape ;
    rdfs:label "Run status" ;
    rdfs:subClassOf s223:EnumerationKind .

sh:Literal a sh:NodeKind ;
    rdfs:label "Literal"@en ;
    rdfs:comment "The node kind of all literals."@en ;
    rdfs:isDefinedBy sh: .

s223:Context-Dimensionless a s223:Class,
        s223:Context-Dimensionless,
        sh:NodeShape ;
    rdfs:label "Context-Dimensionless" ;
    rdfs:comment "This class has enumerated instances of contexts often used with the s223:hasAspect relation for a s223:Property with a dimensionless numerical value." ;
    rdfs:subClassOf s223:EnumerationKind-Context .

s223:DayOfWeek-Weekday a s223:Class,
        s223:DayOfWeek-Weekday,
        sh:NodeShape ;
    rdfs:label "Day of week-Weekday",
        "Weekday" ;
    rdfs:comment "This class defines the EnumerationKind values of Monday, Tuesday, Wednesday, Thursday, and Friday" ;
    rdfs:subClassOf s223:Attribute-DayOfWeek .

s223:ElectricBreaker a s223:Class,
        sh:NodeShape ;
    rdfs:label "Electric breaker" ;
    rdfs:comment "A device designed to open the circuit automatically at a predetermined overcurrent without damage to itself (when properly applied within its rating)." ;
    rdfs:subClassOf s223:Equipment ;
    sh:property [ rdfs:comment "An ElectricBreaker shall have at least one outlet using the medium Electricity." ;
            sh:path s223:hasConnectionPoint ;
            sh:qualifiedMinCount 1 ;
            sh:qualifiedValueShape [ sh:class s223:OutletConnectionPoint ;
                    sh:node [ sh:property [ sh:class s223:Medium-Electricity ;
                                    sh:path s223:hasMedium ] ] ] ],
        [ sh:minCount 2 ;
            sh:path s223:hasConnectionPoint ] .

s223:Electricity-Signal a s223:Class,
        s223:Electricity-Signal,
        sh:NodeShape ;
    rdfs:label "Electricity Signal" ;
    rdfs:subClassOf s223:Medium-Electricity .

s223:EnumeratedActuatableProperty a s223:Class,
        sh:NodeShape ;
    rdfs:label "Enumerated actuatable property" ;
    rdfs:comment "An EnumeratedActuatableProperty is a property with an enumerated (fixed) set of possible values that can be changed (actuated)" ;
    rdfs:subClassOf s223:ActuatableProperty,
        s223:EnumerableProperty .

s223:EnumeratedObservableProperty a s223:Class,
        sh:NodeShape ;
    rdfs:label "Enumerated observable property" ;
    rdfs:comment "An EnumeratedActuatableProperty is a property with an enumerated (fixed) set of possible values that can only be observed (not changed)" ;
    rdfs:subClassOf s223:EnumerableProperty,
        s223:ObservableProperty .

s223:EnumerationKind-HVACOperatingMode a s223:Class,
        s223:EnumerationKind-HVACOperatingMode,
        sh:NodeShape ;
    rdfs:label "HVAC system/equipment operating mode. The policy under which the system is operating." ;
    rdfs:subClassOf s223:EnumerationKind .

s223:EnumerationKind-HVACOperatingStatus a s223:Class,
        s223:EnumerationKind-HVACOperatingStatus,
        sh:NodeShape ;
    rdfs:label "HVAC system/equipment operating status. What the system is currently doing." ;
    rdfs:subClassOf s223:EnumerationKind .

s223:EnumerationKind-Occupancy a s223:Class,
        s223:EnumerationKind-Occupancy,
        sh:NodeShape ;
    rdfs:label "Occupancy status" ;
    rdfs:subClassOf s223:EnumerationKind .

s223:EnumerationKind-Phase a s223:Class,
        s223:EnumerationKind-Phase,
        sh:NodeShape ;
    rdfs:label "EnumerationKind-Phase" ;
    rdfs:subClassOf s223:EnumerationKind .

s223:EnumerationKind-Substance a s223:Class,
        s223:EnumerationKind-Substance,
        sh:NodeShape ;
    rdfs:label "Substance" ;
    rdfs:comment "This class has enumerated instances of the substances that are consumed, produced, transported, sensed, controlled or otherwise interacted with (e.g. water, air, etc.)." ;
    rdfs:subClassOf s223:EnumerationKind .

s223:FunctionBlock a s223:Class,
        sh:NodeShape ;
    rdfs:label "Function block" ;
    rdfs:comment "A FunctionBlock is used to model transfer and/or transformation of information (i.e. Property). It has relations to input properties and output properties. The actual algorithms that perform the transformations are described in CDL and are out of scope of the 223 standard." ;
    rdfs:subClassOf s223:Concept ;
    sh:property [ rdfs:comment "An instance of Function block can be associated with any number of Constant instances using the relation 'has constant'." ;
            sh:class s223:Constant ;
            sh:path s223:hasConstant ],
        [ rdfs:comment "An instance of Function block can be associated with any number of Input instances using the relation 'has function input'." ;
            sh:class s223:FunctionInput ;
            sh:path s223:hasInput ],
        [ rdfs:comment "An instance of Function block can be associated with any number of Output instances using the relation 'has function output'." ;
            sh:class s223:FunctionOutput ;
            sh:path s223:hasOutput ],
        [ rdfs:comment "An instance of Function block can be associated with any number of Parameter instances using the relation 'has parameter'." ;
            sh:class s223:Parameter ;
            sh:path s223:hasParameter ] .

s223:LineNeutralVoltage-120.0V a s223:Dimensioned-LineNeutralVoltage ;
    rdfs:label "120.0V Line-Neutral Voltage" ;
    s223:hasVoltage s223:Voltage-120.0V .

s223:MotorizedDamper a s223:Class ;
    rdfs:label "Motorized damper" ;
    rdfs:subClassOf s223:Damper .

s223:Occupancy-Motion a s223:Class,
        s223:Occupancy-Motion,
        sh:NodeShape ;
    rdfs:label "Occupancy Motion" ;
    rdfs:subClassOf s223:EnumerationKind-Occupancy .

s223:Occupancy-Presence a s223:Class,
        s223:Occupancy-Presence,
        sh:NodeShape ;
    rdfs:label "Occupancy Presence" ;
    rdfs:subClassOf s223:EnumerationKind-Occupancy .

s223:Role-Heating a s223:EnumerationKind-Role ;
    rdfs:label "Role-Heating" .

s223:Valve a s223:Class,
        sh:NodeShape ;
    rdfs:label "Valve" ;
    rdfs:comment "A device to regulate or stop the flow of fluid in a pipe or a duct by throttling." ;
    rdfs:subClassOf s223:Equipment ;
    sh:property [ rdfs:comment "A Valve shall have at least one inlet." ;
            sh:path s223:hasConnectionPoint ;
            sh:qualifiedMinCount 1 ;
            sh:qualifiedValueShape [ sh:class s223:InletConnectionPoint ] ],
        [ rdfs:comment "A Valve shall have at least one outlet." ;
            sh:path s223:hasConnectionPoint ;
            sh:qualifiedMinCount 1 ;
            sh:qualifiedValueShape [ sh:class s223:OutletConnectionPoint ] ],
        [ sh:minCount 2 ;
            sh:path s223:hasConnectionPoint ] .

psm:i00025 a s223:HeatingCoil ;
    rdfs:label "A-9.hot_water_coil" ;
    s223:cnx psm:i00026,
        psm:i00027,
        psm:i00028,
        psm:i00029 .

psm:i00036 a s223:CoolingCoil ;
    rdfs:label "A-9.chilled_water_coil" ;
    s223:cnx psm:i00037,
        psm:i00038,
        psm:i00039,
        psm:i00040 .

sh:Info a sh:Severity ;
    rdfs:label "Info"@en ;
    rdfs:comment "The severity for an informational validation result."@en ;
    rdfs:isDefinedBy sh: .

s223:FunctionOutput a s223:Class,
        sh:NodeShape ;
    rdfs:label "Output" ;
    rdfs:comment "A Function Output is an output from a Function Block and represents the action the function block has on the value its Function Input propert(ies). It is related to a property by s223:produces." ;
    rdfs:subClassOf s223:Concept ;
    sh:property [ sh:class s223:FunctionBlock ;
            sh:maxCount 1 ;
            sh:message "This Output must be associated with exactly one FunctionBlock." ;
            sh:minCount 1 ;
            sh:path [ sh:inversePath s223:hasOutput ] ],
        [ rdfs:comment "An instance of Output must be associated with any number of Property instances using the relation 'produces'." ;
            sh:class s223:Property ;
            sh:maxCount 1 ;
            sh:minCount 1 ;
            sh:path s223:produces ] .

s223:cnx a s223:SymmetricProperty ;
    rdfs:label "cnx" ;
    rdfs:comment "The cnx property is a symmetric property used to associate adjacent entities in a connection path (comprised of Equipment-ConnectionPoint-Connection-ConnectionPoint-Equipment sequences)." .

sh:IRI a sh:NodeKind ;
    rdfs:label "IRI"@en ;
    rdfs:comment "The node kind of all IRIs."@en ;
    rdfs:isDefinedBy sh: .

s223:EM-Light a s223:Class,
        s223:EM-Light,
        sh:NodeShape ;
    rdfs:label "EM-Light" ;
    rdfs:subClassOf s223:Medium-EM .

s223:PhysicalSpace a s223:Class,
        sh:NodeShape ;
    rdfs:label "Physical Space" ;
    rdfs:comment "A PhysicalSpace is an architectural concept representing a room, a collection of rooms such as a floor, a part of a room, or any physical space that might not even be thought of as a room, such as a patio space or a roof." ;
    rdfs:subClassOf s223:Concept ;
    sh:property [ rdfs:comment "A PhysicalSpace can be associated with any number of other PhysicalSpaces using the relation contains" ;
            sh:class s223:PhysicalSpace ;
            sh:path s223:contains ],
        [ rdfs:comment "A PhysicalSpace can be associated with any number of DomainSpaces using the relation encloses" ;
            sh:class s223:DomainSpace ;
            sh:path s223:encloses ] .

s223:hasDomain a rdf:Property ;
    rdfs:label "has domain" ;
    rdfs:comment "The relation hasDomain is used to indicate what domain a Zone or DomainSpace pertains to (e.g. HVAC, lighting, electrical, etc.). Possible values are defined in EnumerationKind-Domain (see `s223:EnumerationKind-Domain`)." .

s223:LineLineVoltage-240.0V a s223:Dimensioned-LineLineVoltage ;
    rdfs:label "240.0V Line-Line Voltage" ;
    s223:hasVoltage s223:Voltage-240.0V .

s223:TemperatureSensor a s223:Class,
        sh:NodeShape ;
    rdfs:label "Temp sensor" ;
    rdfs:comment "A TemperatureSensor is a specialization of a Sensor that observes a QuantifiableObservableProperty that represents a temperature measurement." ;
    rdfs:subClassOf s223:Sensor ;
    sh:property [ rdfs:comment "A TemperatureSensor will always observe a Property that has a QuantityKind of Temperature." ;
            sh:path s223:observes ;
            sh:qualifiedMinCount 1 ;
            sh:qualifiedValueShape [ sh:class s223:Property ;
                    sh:node [ sh:property [ sh:hasValue quantitykind:Temperature ;
                                    sh:path qudt:hasQuantityKind ] ] ] ] .

s223:Water-ChilledWater a s223:Medium-Water ;
    rdfs:label "Water-Chilled water" .

psm:ElectricCircuit2 a s223:ElectricWire ;
    rdfs:label "Electric Circuit 2" ;
    s223:hasMedium s223:AC-120V-60Hz .

s223:Context-Attribute a s223:Class,
        s223:Context-Attribute,
        sh:NodeShape ;
    rdfs:label "Context-Attribute" ;
    rdfs:comment "This class has enumerated instances to specify contexts used with the s223:hasAspect relation for a s223:Property with a non-numerical value." ;
    rdfs:subClassOf s223:EnumerationKind-Context .

s223:Damper a s223:Class,
        sh:NodeShape ;
    rdfs:label "Damper" ;
    rdfs:comment "An element inserted into an air-distribution system or element of an air-distribution system permitting modification of the air resistance of the system and consequently changing the airflow rate or shutting off the airflow." ;
    rdfs:subClassOf s223:Equipment ;
    sh:property [ sh:minCount 2 ;
            sh:path s223:hasConnectionPoint ],
        [ rdfs:comment "A Damper shall have at least one inlet using the medium Air." ;
            sh:path s223:hasConnectionPoint ;
            sh:qualifiedMinCount 1 ;
            sh:qualifiedValueShape [ sh:class s223:InletConnectionPoint ;
                    sh:node [ sh:property [ sh:class s223:Medium-Air ;
                                    sh:path s223:hasMedium ] ] ] ],
        [ rdfs:comment "A Damper shall have at least one outlet using the medium Air." ;
            sh:path s223:hasConnectionPoint ;
            sh:qualifiedMinCount 1 ;
            sh:qualifiedValueShape [ sh:class s223:OutletConnectionPoint ;
                    sh:node [ sh:property [ sh:class s223:Medium-Air ;
                                    sh:path s223:hasMedium ] ] ] ] .

s223:Domain-HVAC a s223:EnumerationKind-Domain ;
    rdfs:label "Domain-HVAC" ;
    rdfs:comment "The domain HVAC represents equipment used to provide space conditioning and ventilation within a building. Example equipment that might fall within an HVAC domain include fans, pumps, air-handling units, and variable air volume boxes. " .

s223:ElectricWire a s223:Class,
        sh:NodeShape ;
    rdfs:label "Electric wire" ;
    rdfs:comment "An ElectricWire is a subclass of Connection, that represents one or more electrical conductors used to convey electricity." ;
    rdfs:subClassOf s223:Connection ;
    sh:property [ rdfs:comment "An ElectricWire must be associated with one Medium-Electricity using the relation hasMedium" ;
            sh:class s223:Medium-Electricity ;
            sh:maxCount 1 ;
            sh:minCount 1 ;
            sh:path s223:hasMedium ] .

s223:hasObservationLocation a rdf:Property ;
    rdfs:label "has observation location" ;
    rdfs:comment "The relation hasObservationLocation associates a sensor to the topological location where it is observing the property (see `s223:observes`). The observation location can be a ConnectionPoint, Connection, Segment or a DomainSpace." .

g36:AnalogOut a s223:Class,
        sh:NodeShape ;
    rdfs:label "Analog out" ;
    rdfs:subClassOf s223:QuantifiableActuatableProperty ;
    sh:rule [ a sh:TripleRule ;
            rdfs:comment "An AnalogOut is a QuantifiableActuatableProperty." ;
            sh:object s223:QuantifiableActuatableProperty ;
            sh:predicate rdf:type ;
            sh:subject sh:this ] .

s223:Attribute-ElectricalPhaseIdentifier a s223:Attribute-ElectricalPhaseIdentifier,
        s223:Class,
        sh:NodeShape ;
    rdfs:label "Attribute-Electrical phase identifier" ;
    rdfs:comment "The value of the associated Property identifies the electrical phase of the Connection." ;
    rdfs:subClassOf s223:Context-Attribute .

s223:Connectable a s223:Class,
        sh:NodeShape ;
    rdfs:label "Connectable" ;
    s223:abstract true ;
    rdfs:comment "Connectable is an abstract class representing a thing (Equipment or DomainSpace) that can be connected via ConnectionPoints and Connections." ;
    rdfs:subClassOf s223:Concept ;
    sh:property [ rdfs:comment "A Connectable can be associated with any number of other Connectables using the relation connected" ;
            sh:class s223:Connectable ;
            sh:name "SymmetricConnectableToConnectableShape" ;
            sh:path s223:connected ],
        [ rdfs:comment "A Connectable can be associated with any number of other Connectables using the relation connectedFrom" ;
            sh:class s223:Connectable ;
            sh:path s223:connectedFrom ],
        [ rdfs:comment "A Connectable can be associated with any number of Connections using the relation connectedThrough" ;
            sh:class s223:Connection ;
            sh:name "EquipmentToConnectionShape" ;
            sh:path s223:connectedThrough ],
        [ rdfs:comment "A Connectable can be associated with any number of other Connectables using the relation connectedTo" ;
            sh:class s223:Connectable ;
            sh:name "ConnectableToConnectableShape" ;
            sh:path s223:connectedTo ],
        [ rdfs:comment "A Connectable can be associated with any number of ConnectionPoints using the relation hasConnectionPoint" ;
            sh:class s223:ConnectionPoint ;
            sh:name "EquipmentToConnectionPointShape" ;
            sh:path s223:hasConnectionPoint ],
        [ rdfs:comment "If a CP mapsTo another CP, the respective Equipment should have a contains relation." ;
            sh:path s223:mapsTo ;
            sh:sparql [ a sh:SPARQLConstraint ;
                    rdfs:comment "If a Connectable is s223:connected (high-level), it must eventually have the underlying cnx relations." ;
                    sh:message "{$this} is s223:connected (high-level) to {?otherC} but not yet connected at the cnx-level." ;
                    sh:prefixes s223: ;
                    sh:select """
SELECT $this ?otherC
WHERE {
$this s223:connected ?otherC .
FILTER NOT EXISTS {$this s223:cnx+ ?otherC}
}
""" ;
                    sh:severity sh:Warning ] ] ;
    sh:rule [ a sh:SPARQLRule ;
            rdfs:comment "Infer the connected relationship for BiDirectional connections" ;
            sh:construct """
CONSTRUCT {$this s223:connected ?d2 .}
WHERE {
$this s223:connectedThrough/^s223:connectedThrough ?d2 .
FILTER ($this != ?d2) .
FILTER NOT EXISTS {$this s223:contains* ?d2} .
FILTER NOT EXISTS {?d2 s223:contains* $this} .
}
""" ;
            sh:name "InferredEquipmentToDownstreamEquipmentProperty" ;
            sh:prefixes s223: ],
        [ a sh:TripleRule ;
            rdfs:comment "Infer the connected relationship using connectedTo" ;
            sh:name "InferredEquipmentToEquipmentPropertyfromconnectedTo" ;
            sh:object [ sh:path s223:connectedTo ] ;
            sh:predicate s223:connected ;
            sh:subject sh:this ],
        [ a sh:TripleRule ;
            rdfs:comment "Infer the connectedThrough relationship using hasConnectionPoint and connectsThrough" ;
            sh:name "InferredEquipmentToConnectionProperty" ;
            sh:object [ sh:path ( s223:hasConnectionPoint s223:connectsThrough ) ] ;
            sh:predicate s223:connectedThrough ;
            sh:subject sh:this ],
        [ a sh:TripleRule ;
            rdfs:comment "Infer the hasConnectionPoint relationship using cnx" ;
            sh:name "InferredEquipmentToConnectionPointProperty" ;
            sh:object [ sh:path s223:cnx ] ;
            sh:predicate s223:hasConnectionPoint ;
            sh:subject sh:this ],
        [ a sh:SPARQLRule ;
            rdfs:comment "Infer the connectedFrom relationship" ;
            sh:construct """
CONSTRUCT {$this s223:connectedFrom ?equipment .}
WHERE {
$this s223:hasConnectionPoint ?cp .
?cp a s223:InletConnectionPoint .
?cp s223:connectsThrough/s223:connectsFrom ?equipment .
}
""" ;
            sh:name "InferredEquipmentToUpstreamEquipmentProperty" ;
            sh:prefixes s223: ],
        [ a sh:SPARQLRule ;
            rdfs:comment "Infer the connectedTo relationship" ;
            sh:construct """
CONSTRUCT {$this s223:connectedTo ?equipment .}
WHERE {
$this s223:hasConnectionPoint ?cp .
?cp a s223:OutletConnectionPoint .
?cp s223:connectsThrough/s223:connectsTo ?equipment .
}
""" ;
            sh:name "InferredEquipmentToDownstreamEquipmentProperty" ;
            sh:prefixes s223: ],
        [ a sh:TripleRule ;
            rdfs:comment "Infer the cnx relationship from hasConnectionPoint" ;
            sh:name "InferredEquipmentToConnectionPointCnxProperty" ;
            sh:object [ sh:path s223:hasConnectionPoint ] ;
            sh:predicate s223:cnx ;
            sh:subject sh:this ],
        [ a sh:TripleRule ;
            rdfs:comment "Infer the cnx relationship from isConnectionPointOf" ;
            sh:name "InferredEquipmentToConnectionPointCnxPropertyFromInverse" ;
            sh:object [ sh:path [ sh:inversePath s223:isConnectionPointOf ] ] ;
            sh:predicate s223:cnx ;
            sh:subject sh:this ],
        [ a sh:TripleRule ;
            rdfs:comment "Infer the connected relationship using connectedFrom" ;
            sh:name "InferredEquipmentToEquipmentPropertyfromconnectedFrom" ;
            sh:object [ sh:path s223:connectedFrom ] ;
            sh:predicate s223:connected ;
            sh:subject sh:this ] .

s223:ConnectionPoint a s223:Class,
        sh:NodeShape ;
    rdfs:label "ConnectionPoint" ;
    s223:abstract true ;
    rdfs:comment """
A ConnectionPoint is an abstract modeling construct used to represent the fact that one connectable thing can be connected to another connectable thing using a Connection. It is the abstract representation of the flange, wire terminal, or other physical feature where a connection is made. Equipment and DomainSpaces can have one or more ConnectionPoints (see `s223:Connectable` and `s223:Connection`).

A ConnectionPoint must constrained to relate to a specific medium such as air, water, or electricity which determines what other things can be connected to it. For example, constraining a ConnectionPoint to be for air means it cannot be used for an electrical connection.

A ConnectionPoint belongs to exactly one connectable thing.

ConnectionPoints are represented graphically in this standard by a triangle with the point indicating a direction of flow, or a diamond in the case of a bidirectional connection as shown in Figure 5-2. 

![Figure 5-2. Graphical Representation of a ConnectionPoint.](figures/Figure_5-2_Graphical_Depiciton_of_Connection_Points.svg)

 """ ;
    rdfs:subClassOf s223:Concept ;
    sh:property [ rdfs:comment "A ConnectionPoint should be associated with one Connection using the relation connectsThrough" ;
            sh:class s223:Connection ;
            sh:maxCount 1 ;
            sh:message "This ConnectionPoint should eventually be associated with exactly one Connection." ;
            sh:minCount 1 ;
            sh:name "ConnectionPointToConnectionShape" ;
            sh:path s223:connectsThrough ;
            sh:severity sh:Info ],
        [ rdfs:comment "A ConnectionPoint must be associated with one EnumerationKind-Medium using the relation hasMedium" ;
            sh:class s223:EnumerationKind-Medium ;
            sh:maxCount 1 ;
            sh:minCount 1 ;
            sh:name "ConnectionPoint medium" ;
            sh:path s223:hasMedium ],
        [ rdfs:comment "A ConnectionPoint can be associated with at most one Connectable using the relation isConnectionPointOf" ;
            sh:class s223:Connectable ;
            sh:maxCount 1 ;
            sh:name "ConnectionPointToEquipmentShape" ;
            sh:path s223:isConnectionPointOf ],
        [ rdfs:comment "A ConnectionPoint can be associated with any number of Segments using the relation lnx" ;
            sh:class s223:Segment ;
            sh:path s223:lnx ],
        [ rdfs:comment "A ConnectionPoint can be associated with at most one other ConnectionPoint using the relation mapsTo" ;
            sh:class s223:ConnectionPoint ;
            sh:maxCount 1 ;
            sh:path s223:mapsTo ],
        [ s223:description "If a CP mapsTo another CP, the respective Equipment should have a contains relation." ;
            sh:path s223:mapsTo ;
            sh:sparql [ a sh:SPARQLConstraint ;
                    rdfs:comment "If a CP mapsTo another CP, the respective Equipment should have a contains relation." ;
                    sh:message "{?otherEquipment} should contain {?equipment} because ConnectionPoint {$this} has a mapsTo relation." ;
                    sh:prefixes s223: ;
                    sh:select """
SELECT $this ?equipment ?otherEquipment
WHERE {
$this s223:mapsTo ?otherCP .
?equipment s223:hasConnectionPoint $this .
?otherEquipment s223:hasConnectionPoint ?otherCP .
FILTER NOT EXISTS {?otherEquipment s223:contains ?equipment}
}
""" ] ],
        [ sh:name "Test for compatible declared Medium" ;
            sh:path s223:hasMedium ;
            sh:sparql [ a sh:SPARQLConstraint ;
                    rdfs:comment "Ensure that the Medium identified by a ConnectionPoint via the s223:hasMedium relation is compatible with the Medium identified by the entity identified by the mapsTo+ relation." ;
                    sh:message "{$this} declares a Medium of {?a}, but the Medium of {?b} is declared by {?target} pointed to by the mapsTo+ relation." ;
                    sh:prefixes s223: ;
                    sh:select """
SELECT DISTINCT $this ?a ?b ?target
WHERE {
$this s223:hasMedium ?a .
$this s223:mapsTo+ ?target .
?target s223:hasMedium ?b .
?a a/rdfs:subClassOf* s223:EnumerationKind-Medium .
?b a/rdfs:subClassOf* s223:EnumerationKind-Medium .
FILTER (?a != ?b ) .
FILTER (NOT EXISTS {?b a/rdfs:subClassOf* ?a}) .
FILTER (NOT EXISTS {?a a/rdfs:subClassOf* ?b}) .
}
""" ] ] .

s223:EnumerationKind-Medium a s223:Class,
        s223:EnumerationKind-Medium,
        sh:NodeShape ;
    rdfs:label "Medium" ;
    rdfs:subClassOf s223:EnumerationKind .

g36:AnalogIn a s223:Class,
        sh:NodeShape ;
    rdfs:label "Analog in" ;
    rdfs:subClassOf s223:QuantifiableObservableProperty ;
    sh:rule [ a sh:TripleRule ;
            rdfs:comment "An AnalogIn is a QuantifiableObervableProperty.",
                "Getting validation reports about AnalogIn not being Property or ObservableProperty. Should probably move this rule up." ;
            sh:object s223:QuantifiableObservableProperty ;
            sh:predicate rdf:type ;
            sh:subject sh:this ] .

s223:Actuator a s223:Class,
        sh:NodeShape ;
    rdfs:label "Actuator" ;
    rdfs:comment "A device, either electrically, pneumatically, or hydraulically operated, that acts as a motor to change the position of movable devices such as valves or dampers." ;
    rdfs:subClassOf s223:Equipment ;
    sh:property [ sh:class s223:Equipment ;
            sh:path s223:actuates ],
        [ rdfs:comment "An instance of Actuator must be associated with at least 1 actuatable property instance using the relation 'commanded by Property'." ;
            sh:class s223:ActuatableProperty ;
            sh:minCount 1 ;
            sh:path s223:commandedByProperty ] .

s223:Domain-Lighting a s223:EnumerationKind-Domain ;
    rdfs:label "Domain-Lighting" ;
    rdfs:comment "The domain Lighting represents equipment used to provide illumination within or outside a building. Example equipment that might fall within a Lighting domain includes luminaires, daylight sensors, and movable sun shades." .

s223:Luminaire a s223:Class,
        sh:NodeShape ;
    rdfs:label "Luminaire" ;
    rdfs:comment "A complete lighting unit consisting of a lamp or lamps together with the housing designed to distribute the light, position and protect the lamps, and connect the lamps to the power supply." ;
    rdfs:subClassOf s223:Equipment ;
    sh:property [ rdfs:comment "A Luminaire shall have at least one inlet using the medium Electricity." ;
            sh:path s223:hasConnectionPoint ;
            sh:qualifiedMinCount 1 ;
            sh:qualifiedValueShape [ sh:class s223:InletConnectionPoint ;
                    sh:node [ sh:property [ sh:class s223:Medium-Electricity ;
                                    sh:path s223:hasMedium ] ] ] ],
        [ rdfs:comment "A Luminaire shall have at least one outlet using the medium EM-Light." ;
            sh:path s223:hasConnectionPoint ;
            sh:qualifiedMinCount 1 ;
            sh:qualifiedValueShape [ sh:class s223:OutletConnectionPoint ;
                    sh:node [ sh:property [ sh:class s223:EM-Light ;
                                    sh:path s223:hasMedium ] ] ] ],
        [ sh:minCount 2 ;
            sh:path s223:hasConnectionPoint ] .

s223:Zone a s223:Class,
        sh:NodeShape ;
    rdfs:label "Zone" ;
    rdfs:comment "A Zone is a logical grouping (collection) of domain spaces for some functional or system reason, to identify a domain of control, such as a Lighting Zone, or a heating zone" ;
    rdfs:subClassOf s223:Concept ;
    sh:property [ rdfs:comment "A Zone can be associated with any number of other DomainSpaces or Zones using the relation contains" ;
            sh:or ( [ sh:class s223:DomainSpace ] [ sh:class s223:Zone ] ) ;
            sh:path s223:contains ],
        [ rdfs:comment "A Zone must be associated with one EnumerationKind-Domain using the relation hasDomain" ;
            sh:class s223:EnumerationKind-Domain ;
            sh:maxCount 1 ;
            sh:minCount 1 ;
            sh:path s223:hasDomain ] ;
    sh:rule [ a sh:TripleRule ;
            rdfs:comment "Traverse down the contains hierarchy to determine the domain" ;
            sh:object [ sh:path ( [ sh:zeroOrMorePath s223:contains ] s223:hasDomain ) ] ;
            sh:predicate s223:hasDomain ;
            sh:subject sh:this ] .

s223:connectedTo a rdf:Property ;
    rdfs:label "connected to" ;
    s223:inverseOf s223:connectedFrom ;
    rdfs:comment "The relation connectedTo indicates that connectable things are connected with a specific flow direction. A is connectedTo B, means a directionality beginning at A and ending at B.  The inverse direction is indicated by connectedFrom (see `s223:connectedFrom`)." ;
    rdfs:domain s223:Equipment .

s223:mapsTo a rdf:Property ;
    rdfs:label "mapsTo" ;
    rdfs:comment "The relation mapsTo is used to associate a ConnectionPoint of an Equipment to a corresponding ConnectionPoint of the Equipment containing it. The associated ConnectionPoints must have the same direction (see `s223:EnumerationKind-Direction`)." .

s223:EnumerationKind-Domain a s223:Class,
        s223:EnumerationKind-Domain,
        sh:NodeShape ;
    rdfs:label "EnumerationKind Domain" ;
    rdfs:subClassOf s223:EnumerationKind .

s223:OnOff-Off a s223:EnumerationKind-OnOff ;
    rdfs:label "Off" .

s223:Water-HotWater a s223:Medium-Water ;
    rdfs:label "Water-Hot water" .

s223:hasRole a rdf:Property ;
    rdfs:label "hasRole" ;
    rdfs:comment "The relation hasRole is used to indicate the role of an Equipment, Connection, or System within a building (e.g., a heating coil will be associated with Role-Heating). Possible values are defined in EnumerationKind-Role (see `s223:EnumerationKind-Role`)." .

s223:observes a rdf:Property ;
    rdfs:label "observes" ;
    rdfs:comment "The relation observes binds a sensor to one `s223:ObservableProperty` which is used by the sensor to generate a measurement value (ex. a temperature) or a simple observation of a stimulus causing a reaction (a current binary switch that closes a dry contact when a fan is powered on)." .

s223:Sensor a s223:Class,
        sh:NodeShape ;
    rdfs:label "Sensor" ;
    rdfs:comment "A Sensor observes an ObservableProperty (see `s223:ObservableProperty`) which may be quantifiable (see `s223:QuantifiableObservableProperty`), such as a temperature, flowrate, or concentration, or Enumerable (see `s223:EnumeratedObservableProperty)`, such as an alarm state or occupancy state." ;
    rdfs:subClassOf s223:AbstractSensor ;
    sh:rule [ a sh:SPARQLRule ;
            rdfs:comment "Infer the hasObservationLocation relationship for a Sensor from the Property that it is observing, only if the location is unambiguous." ;
            sh:construct """
CONSTRUCT {$this s223:hasObservationLocation ?something .}
WHERE {
{
SELECT ?prop (COUNT (DISTINCT ?measurementLocation) AS ?count) $this
WHERE {
FILTER (NOT EXISTS {$this s223:hasObservationLocation ?anything}) .
$this s223:observes ?prop .
?measurementLocation s223:hasProperty ?prop .
}
GROUP BY ?prop $this
}
FILTER (?count = 1) .
?something s223:hasProperty ?prop .
{?something a/rdfs:subClassOf* s223:Connectable}
UNION
{?something a/rdfs:subClassOf* s223:Connection}
UNION
{?something a/rdfs:subClassOf* s223:Segment}
UNION
{?something a/rdfs:subClassOf* s223:ConnectionPoint}
}
""" ;
            sh:name "InferredMeasurementLocation" ;
            sh:prefixes s223: ] ;
    sh:xone ( [ sh:property [ rdfs:comment "A Sensor must be associated with exactly 1 of Connectable, Connection, Segment, or ConnectionPoint using the relation hasObservationLocation." ;
                        sh:class s223:Connectable ;
                        sh:path s223:hasObservationLocation ] ] [ sh:property [ rdfs:comment "A Sensor must be associated with exactly 1 of Connectable, Connection, Segment, or ConnectionPoint using the relation hasObservationLocation." ;
                        sh:class s223:Connection ;
                        sh:path s223:hasObservationLocation ] ] [ sh:property [ rdfs:comment "A Sensor must be associated with exactly 1 of Connectable, Connection, Segment, or ConnectionPoint using the relation hasObservationLocation." ;
                        sh:class s223:Segment ;
                        sh:path s223:hasObservationLocation ] ] [ sh:property [ rdfs:comment "A Sensor must be associated with exactly 1 of Connectable, Connection, Segment, or ConnectionPoint using the relation hasObservationLocation." ;
                        sh:class s223:ConnectionPoint ;
                        sh:path s223:hasObservationLocation ] ] ),
        ( [ sh:property [ rdfs:comment "A Sensor must be associated with exactly 1 of QuantifiableObservableProperty or EnumeratedObservableProperty using the relation observes." ;
                        sh:class s223:QuantifiableObservableProperty ;
                        sh:path s223:observes ] ] [ sh:property [ rdfs:comment "A Sensor must be associated with exactly 1 of QuantifiableObservableProperty or EnumeratedObservableProperty using the relation observes." ;
                        sh:class s223:EnumeratedObservableProperty ;
                        sh:path s223:observes ] ] ) .

s223:EnumerableProperty a s223:Class,
        sh:NodeShape ;
    rdfs:label "Enumerable Property" ;
    rdfs:subClassOf s223:Property ;
    sh:property [ rdfs:comment "An EnumerableProperty must be associated with one EnumerationKind using the relation hasEnumerationKind" ;
            sh:class s223:EnumerationKind ;
            sh:maxCount 1 ;
            sh:minCount 1 ;
            sh:path s223:hasEnumerationKind ],
        [ rdfs:comment "Checks for valid enumeration value" ;
            sh:path s223:hasValue ;
            sh:sparql [ a sh:SPARQLConstraint ;
                    sh:message "{$this} has an enumeration value of {?value} which is not a valid {?kind}." ;
                    sh:prefixes s223: ;
                    sh:select """
SELECT $this ?value ?kind
WHERE {
$this s223:hasValue ?value .
$this s223:hasEnumerationKind ?kind .
FILTER (NOT EXISTS {?value a/rdfs:subClassOf* ?kind}) .
}
""" ] ] .

s223:QuantifiableActuatableProperty a s223:Class,
        sh:NodeShape ;
    rdfs:label "Quantifiable Actuatable Property" ;
    rdfs:comment "This class is for quantifiable properties of which numerical values are specified to be modifiable by a user or a machine outside of the model, like a setpoint." ;
    rdfs:subClassOf s223:ActuatableProperty,
        s223:QuantifiableProperty .

sh:this a rdfs:Resource ;
    rdfs:label "this"@en ;
    rdfs:comment "A node expression that represents the current focus node."@en ;
    rdfs:isDefinedBy sh: .

s223:Concept a s223:Class,
        sh:NodeShape ;
    rdfs:label "Concept" ;
    s223:abstract true ;
    rdfs:comment "This is the superclass of all classes defined in the 223 standard." ;
    rdfs:subClassOf rdfs:Resource ;
    sh:property [ rdfs:comment "A Concept can use the relation cnx" ;
            sh:path s223:cnx ],
        [ rdfs:comment "A Concept can use the relation hasProperty" ;
            sh:path s223:hasProperty ],
        [ rdfs:comment "A Concept can use the relation label" ;
            sh:path rdfs:label ] ;
    sh:sparql [ a sh:SPARQLConstraint ;
            rdfs:comment "Ensure that any instance that is declared to be an instance of an abstract class must also be declared an instance of at least one subClass of that abstract class" ;
            sh:message "{$this} cannot be declared an instance of only abstract class {?class}." ;
            sh:prefixes s223: ;
            sh:select """
SELECT DISTINCT $this ?class
WHERE {
?class s223:abstract true .
$this a ?class .
OPTIONAL {
?otherClass rdfs:subClassOf+ ?class .
$this a ?otherClass .
FILTER (?class != ?otherClass) .
}
FILTER (!bound (?otherClass)) .
}
""" ] .

s223:EnumerationKind-OnOff a s223:Class,
        s223:EnumerationKind-OnOff,
        sh:NodeShape ;
    rdfs:label "OnOff enumeration" ;
    rdfs:subClassOf s223:EnumerationKind .

s223:EnumerationKind-Role a s223:Class,
        s223:EnumerationKind-Role,
        sh:NodeShape ;
    rdfs:label "Role" ;
    rdfs:subClassOf s223:EnumerationKind .

s223:QuantifiableObservableProperty a s223:Class,
        sh:NodeShape ;
    rdfs:label "Quantifiable Observable Property" ;
    rdfs:comment "This class is for quantifiable properties of which numerical values cannot be modified by a user or a machine outside of the model, but only observed, like a temperature reading or a voltage measure." ;
    rdfs:subClassOf s223:ObservableProperty,
        s223:QuantifiableProperty .

s223:contains a rdf:Property ;
    rdfs:label "contains" .

s223:hasProperty a rdf:Property ;
    rdfs:label "has Property" .

s223:EnumerationKind a s223:Class,
        s223:EnumerationKind,
        sh:NodeShape ;
    rdfs:label "Enumeration kind" ;
    rdfs:comment "This is the encapsulating class for all EnumerationKinds. EnumerationKinds define the (closed) set of permissible values for a given purpose. For example, the DayOfWeek EnumerationKind enumerates the days of the week and allows no other values." ;
    rdfs:subClassOf s223:Concept .

qudt:hasQuantityKind rdfs:comment "A reference to the QuantityKind of a QuantifiableProperty of interest, e.g. quantitykind:Temperature." .

s223:Context-Dimensioned a s223:Class,
        s223:Context-Dimensioned,
        sh:NodeShape ;
    rdfs:label "Context-Dimensioned" ;
    rdfs:comment "This class has enumerated instances of contexts often used with the s223:hasAspect relation for a s223:Property with a numerical value, unit and quantitykind." ;
    rdfs:subClassOf s223:EnumerationKind-Context .

s223:Property a s223:Class,
        sh:NodeShape ;
    rdfs:label "Property" ;
    rdfs:comment """An attribute, quality, or characteristic of a feature of interest.

The Property class is the parent of all variations of a property, which are:
ActuatableProperty - parent of subclass of properties that can be modified by user or machine outside of the model (typically command)
ObservableProperty - parent of subclass of properties that can not be modified by user or machine outside of the model (typically measures)
EnumerableProperty - parent of subclass of properties defined by EnumerationKind
QuantifiableProperty - parent of subclass of properties defined by numerical values

And their different associations :
QuantifiableActuatableProperty
QuantifiableObservableProperty
EnumeratedObservableProperty
EnumeratedActuatableProperty

A QuantifiableProperty (or subClass thereof) must always be associated with a Unit and a QuantityKind, either explicitly from the Property, or through the associated Value. If the Unit is defined, the SHACL reasoner (if invoked) will figure out and assert the QuantityKind (the most general version).

Enumerable properties must be associated with an EnumerationKind.
""" ;
    rdfs:subClassOf s223:Concept ;
    sh:property [ rdfs:comment "A Property can be associated with any number of EnumerationKinds using the relation hasAspect" ;
            sh:class s223:EnumerationKind ;
            sh:path s223:hasAspect ],
        [ rdfs:comment "A Property can use at most one relation hasValue if it is required to provide a static value in the model. It is not meant for real-time value (see ref:hasExternalReference)" ;
            sh:maxCount 1 ;
            sh:path s223:hasValue ],
        [ rdfs:comment "A Property can be associated with at most one EnumerationKind-Medium using the relation ofMedium" ;
            sh:class s223:EnumerationKind-Medium ;
            sh:maxCount 1 ;
            sh:path s223:ofMedium ],
        [ rdfs:comment "A Property can be associated with at most one EnumerationKind-Substance using the relation ofSubstance" ;
            sh:class s223:EnumerationKind-Substance ;
            sh:maxCount 1 ;
            sh:path s223:ofSubstance ],
        [ rdfs:comment "A Property can be associated with any number of ExternalReferences using the relation hasExternalReference" ;
            sh:class ref:ExternalReference ;
            sh:path ref:hasExternalReference ] ;
    sh:sparql [ a sh:SPARQLConstraint ;
            rdfs:comment "A Property instance cannot be declared an instance of both an ActuatableProperty and an ObservableProperty." ;
            sh:message "{$this} cannot be declared an instance of both an ActuatableProperty and an ObservableProperty." ;
            sh:prefixes s223: ;
            sh:select """
SELECT $this
WHERE {
$this a/rdfs:subClassOf* s223:ActuatableProperty .
$this a/rdfs:subClassOf* s223:ObservableProperty .
}
""" ] .

s223:DomainSpace a s223:Class,
        sh:NodeShape ;
    rdfs:label "Domain Space" ;
    rdfs:comment "A DomainSpace is a member (or component) of a Zone and is associated with a Domain such as Lighting, HVAC, PhysicalSecurity, etc. Physical spaces enclose Domain spaces." ;
    rdfs:subClassOf s223:Connectable ;
    sh:property [ rdfs:comment "A DomainSpace must be associated with one EnumerationKind-Domain using the relation hasDomain" ;
            sh:class s223:EnumerationKind-Domain ;
            sh:maxCount 1 ;
            sh:minCount 1 ;
            sh:path s223:hasDomain ],
        [ rdfs:comment "This DomainSpace must eventually be enclosed by a PhysicalSpace." ;
            sh:message "This DomainSpace must eventually be enclosed by a PhysicalSpace." ;
            sh:minCount 1 ;
            sh:path [ sh:inversePath s223:encloses ] ;
            sh:severity sh:Info ] .

s223:Frequency-50Hz a s223:Dimensioned-Frequency,
        s223:QuantifiableProperty ;
    rdfs:label "50 Hertz" ;
    s223:hasValue 50.0 ;
    qudt:hasQuantityKind quantitykind:Frequency ;
    qudt:hasUnit unit:HZ .

s223:Light-Visible a s223:EM-Light ;
    rdfs:label "Light-Visible" .

s223:Medium-Water a s223:Class,
        s223:Medium-Water,
        sh:NodeShape ;
    rdfs:label "Medium-Water" ;
    rdfs:subClassOf s223:EnumerationKind-Medium .

s223:Medium-Electricity a s223:Class,
        s223:Medium-Electricity,
        sh:NodeShape ;
    rdfs:label "Electricity" ;
    rdfs:subClassOf s223:EnumerationKind-Medium .

s223:Dimensioned-LineLineVoltage a s223:Class,
        s223:Context-Dimensioned,
        s223:Dimensioned-LineLineVoltage,
        sh:NodeShape ;
    rdfs:label "Dimensioned Line-Line Voltage",
        "Dimensioned-Line Line Voltage" ;
    rdfs:comment "The value of the associated Property identifies the Line-to-line voltage of the medium" ;
    rdfs:subClassOf s223:Context-Dimensioned .

s223:Dimensioned-Voltage a s223:Class,
        s223:Dimensioned-Voltage,
        sh:NodeShape ;
    rdfs:label "Dimensioned Voltage" ;
    rdfs:subClassOf s223:Context-Dimensioned .

s223:NumberOfElectricalPhases-ThreePhase a s223:Dimensionless-NumberOfElectricalPhases ;
    rdfs:label "Three Phase AC Electricity" .

s223:Dimensioned-LineNeutralVoltage a s223:Class,
        s223:Context-Dimensioned,
        s223:Dimensioned-LineNeutralVoltage,
        sh:NodeShape ;
    rdfs:label "Dimensioned Line-Neutral Voltage",
        "Dimensioned-Line Neutral Voltage" ;
    rdfs:comment "The value of the associated Property identifies the Line-to-neutral voltage of the medium" ;
    rdfs:subClassOf s223:Context-Dimensioned .

s223: a owl:Ontology ;
    sh:declare [ sh:namespace "http://data.ashrae.org/standard223#"^^xsd:anyURI ;
            sh:prefix "s223" ],
        [ sh:namespace "http://www.w3.org/2000/01/rdf-schema#"^^xsd:anyURI ;
            sh:prefix "rdfs" ],
        [ sh:namespace "http://qudt.org/schema/qudt/"^^xsd:anyURI ;
            sh:prefix "qudt" ],
        [ sh:namespace "http://qudt.org/vocab/quantitykind/"^^xsd:anyURI ;
            sh:prefix "quantitykind" ],
        [ sh:namespace "http://data.ashrae.org/standard223#"^^xsd:anyURI ;
            sh:prefix "s223" ],
        [ sh:namespace "http://www.w3.org/2000/01/rdf-schema#"^^xsd:anyURI ;
            sh:prefix "rdfs" ],
        [ sh:namespace "http://data.ashrae.org/standard223#"^^xsd:anyURI ;
            sh:prefix "s223" ],
        [ sh:namespace "http://qudt.org/schema/qudt/"^^xsd:anyURI ;
            sh:prefix "qudt" ],
        [ sh:namespace "http://data.ashrae.org/standard223#"^^xsd:anyURI ;
            sh:prefix "s223" ],
        [ sh:namespace "http://data.ashrae.org/standard223/1.0/vocab/role#"^^xsd:anyURI ;
            sh:prefix "role" ],
        [ sh:namespace "http://qudt.org/vocab/quantitykind/"^^xsd:anyURI ;
            sh:prefix "qudtqk" ],
        [ sh:namespace "http://qudt.org/vocab/unit/"^^xsd:anyURI ;
            sh:prefix "unit" ],
        [ sh:namespace "http://www.w3.org/2000/01/rdf-schema#"^^xsd:anyURI ;
            sh:prefix "rdfs" ],
        [ sh:namespace "http://data.ashrae.org/standard223#"^^xsd:anyURI ;
            sh:prefix "s223" ],
        [ sh:namespace "http://data.ashrae.org/standard223/1.0/vocab/enumeration#"^^xsd:anyURI ;
            sh:prefix "enum" ],
        [ sh:namespace "http://www.w3.org/1999/02/22-rdf-syntax-ns#"^^xsd:anyURI ;
            sh:prefix "rdf" ],
        [ sh:namespace "http://www.w3.org/2000/01/rdf-schema#"^^xsd:anyURI ;
            sh:prefix "rdfs" ],
        [ sh:namespace "http://www.w3.org/ns/shacl#"^^xsd:anyURI ;
            sh:prefix "sh" ],
        [ sh:namespace "http://data.ashrae.org/standard223#"^^xsd:anyURI ;
            sh:prefix "s223" ],
        [ sh:namespace "http://www.w3.org/2000/01/rdf-schema#"^^xsd:anyURI ;
            sh:prefix "rdfs" ],
        [ sh:namespace "http://data.ashrae.org/standard223#"^^xsd:anyURI ;
            sh:prefix "s223" ] .

s223:QuantifiableProperty a s223:Class,
        sh:NodeShape ;
    rdfs:label "Quantifiable Property" ;
    rdfs:comment "This class is for quantifiable values that describe an object (System, Equipment, etc.) that are typically static (hasValue). That is, they are neither measured nor specified in the course of operations." ;
    rdfs:subClassOf s223:Property,
        qudt:Quantity ;
    sh:property [ rdfs:comment "A QuantifiableProperty can be associated with any number of Setpoints using the relation hasSetpoint" ;
            sh:class s223:Setpoint ;
            sh:path s223:hasSetpoint ],
        [ rdfs:comment "A QuantifiableProperty can be associated with a decimal value using the relation hasValue" ;
            sh:datatype xsd:decimal ;
            sh:path s223:hasValue ],
        [ rdfs:comment "A QuantifiableProperty must be associated with at least one quantitykind using the relation hasQuantityKind." ;
            sh:class qudt:QuantityKind ;
            sh:minCount 1 ;
            sh:path qudt:hasQuantityKind ],
        [ rdfs:comment "A QuantifiableProperty should be associated with at least one unit using the relation hasUnit." ;
            sh:class qudt:Unit ;
            sh:minCount 1 ;
            sh:path qudt:hasUnit ;
            sh:severity sh:Info ],
        [ rdfs:comment "This QuantifiableProperty and the Setpoint associated with it have non-commensurate QuantityKinds" ;
            sh:path qudt:hasQuantityKind ;
            sh:sparql [ a sh:SPARQLConstraint ;
                    sh:message "{$this} uses QuantityKind {?pqk} with DimensionVector {?pdv}, while Setpoint {?setpoint} uses QuantityKind {?sqk} with DimensionVector {?sdv}. These are non-commensurate" ;
                    sh:prefixes s223: ;
                    sh:select """
SELECT $this ?setpoint ?pqk ?sqk ?pdv ?sdv
WHERE {
$this qudt:hasQuantityKind ?pqk .
$this s223:hasSetpoint ?setpoint .
?setpoint qudt:hasQuantityKind ?sqk .
?pqk qudt:hasDimensionVector ?pdv .
?sqk qudt:hasDimensionVector ?sdv .
FILTER (?pqk != ?sqk) .
FILTER (?pdv != ?sdv) .
}
""" ] ],
        [ rdfs:comment "This QuantifiableProperty and the associated Setpoint use non-commensurate Units" ;
            sh:path qudt:hasUnit ;
            sh:sparql [ a sh:SPARQLConstraint ;
                    sh:message "{$this} uses Unit {?punit}, while Setpoint {?setpoint} uses Unit {?sunit}. These are non-commensurate." ;
                    sh:prefixes s223: ;
                    sh:select """
SELECT $this ?setpoint ?punit ?sunit
WHERE {
$this qudt:hasUnit ?punit .
$this s223:hasSetpoint ?setpoint .
?setpoint qudt:hasUnit ?sunit .
?punit qudt:hasDimensionVector ?pdv .
?sunit qudt:hasDimensionVector ?sdv .
FILTER (?punit != ?sunit) .
FILTER (?pdv != ?sdv) .
}
""" ] ],
        [ rdfs:comment "This QuantifiableProperty uses a different Unit than the Setpoint associated with it" ;
            sh:path qudt:hasUnit ;
            sh:severity sh:Info ;
            sh:sparql [ a sh:SPARQLConstraint ;
                    sh:message "{$this} uses Unit {?punit}, while Setpoint {?setpoint} uses Unit {?sunit}. Be careful." ;
                    sh:prefixes s223: ;
                    sh:select """
SELECT $this ?setpoint ?punit ?sunit
WHERE {
$this qudt:hasUnit ?punit .
$this s223:hasSetpoint ?setpoint .
?setpoint qudt:hasUnit ?sunit .
?punit qudt:hasDimensionVector ?pdv .
?sunit qudt:hasDimensionVector ?sdv .
FILTER (?punit != ?sunit) .
FILTER (?pdv = ?sdv) .
}
""" ] ] ;
    sh:rule [ a sh:SPARQLRule ;
            rdfs:comment "Infer the hasQuantityKind relationship if it is unambiguous" ;
            sh:construct """
CONSTRUCT {
$this qudt:hasQuantityKind ?uniqueqk
}
WHERE {
{
SELECT $this (COUNT (DISTINCT (?qk)) AS ?count)
WHERE {
FILTER (NOT EXISTS {$this qudt:hasQuantityKind ?something}) .
$this qudt:hasUnit/qudt:hasQuantityKind ?qk .
}
GROUP BY $this
}
FILTER (?count = 1)
$this qudt:hasUnit/qudt:hasQuantityKind ?uniqueqk .
}
""" ;
            sh:prefixes s223: ] ;
    sh:sparql [ a sh:SPARQLConstraint ;
            rdfs:comment "Checks for consistent dimension vectors for a QuantityKind and the Unit" ;
            sh:message "Inconsistent dimensionalities among the Property's Unit and Property's Quantity Kind" ;
            sh:prefixes s223: ;
            sh:select """
SELECT $this ?count
WHERE {  
{ SELECT  $this (COUNT (DISTINCT ?qkdv) AS ?count)
   WHERE 
{
      {
      $this qudt:hasQuantityKind/qudt:hasDimensionVector ?qkdv .
      }
      UNION
      {
      $this qudt:hasUnit/qudt:hasDimensionVector ?qkdv .
      }
}
 GROUP BY $this 
}
FILTER (?count > 1) .
}
""" ] .

s223:Connection a s223:Class,
        sh:NodeShape ;
    rdfs:label "Connection" ;
    rdfs:comment """A Connection is the modeling construct used to represent a physical thing (e.g., pipe, duct, or wire) that is used to convey some Medium (e.g., water, air, or electricity) between two connectable things. All Connections have two or more ConnectionPoints bound to either Equipment (see `s223:Equipment`) or DomainSpace (see `s223:DomainSpace`). If the direction of flow is constrained, that constraint is indicated by using one or more InletConnectionPoints (see `s223:InletConnectionPoint`) to represent the inflow points and OutletConnectionPoints (see `s223:OutletConnectionPoint`) to represent the outflow points.
  
A Connection may contain branches or intersections. These are modeled using Segments (see `s223:Segment`) and Junctions (see `s223:Junction`).
""" ;
    rdfs:subClassOf s223:Concept ;
    sh:property [ rdfs:comment "A Connection can be associated with any number of ConnectionPoints using the relation connectsAt" ;
            sh:class s223:ConnectionPoint ;
            sh:path s223:connectsAt ],
        [ rdfs:comment "A Connection can be associated with any number of Connectables using the relation connectsFrom" ;
            sh:class s223:Connectable ;
            sh:name "ConnectionToUpstreamConnectableShape" ;
            sh:path s223:connectsFrom ],
        [ rdfs:comment "A Connection can be associated with any number of Connectables using the relation connectsTo" ;
            sh:class s223:Connectable ;
            sh:name "ConnectionToDownstreamConnectableShape" ;
            sh:path s223:connectsTo ],
        [ rdfs:comment "A Connection must be associated with one EnumerationKind-Medium using the relation hasMedium" ;
            sh:class s223:EnumerationKind-Medium ;
            sh:maxCount 1 ;
            sh:minCount 1 ;
            sh:name "Connection medium" ;
            sh:path s223:hasMedium ],
        [ sh:class s223:EnumerationKind-Phase ;
            sh:path s223:hasPhase ],
        [ rdfs:comment "A Connection can be associated with an EnumerationKind-Role using the relation hasRole" ;
            sh:class s223:EnumerationKind-Role ;
            sh:path s223:hasRole ],
        [ sh:name "Test for compatible declared Medium" ;
            sh:path s223:hasMedium ;
            sh:sparql [ a sh:SPARQLConstraint ;
                    rdfs:comment "Ensure that the Medium identified by a ConnectionPoint via the s223:hasMedium relation is compatible with the Medium identified by the associated Connection." ;
                    sh:message "{$this} with Medium {?m2} is incompatible with {?cp} with Medium {?m1}." ;
                    sh:prefixes s223: ;
                    sh:select """
SELECT $this ?m2 ?cp ?m1
WHERE {
$this s223:cnx ?cp .
?cp a/rdfs:subClassOf* s223:ConnectionPoint .
?cp s223:hasMedium ?m1 .
$this s223:hasMedium ?m2 .
FILTER (?m1 != ?m2 ) .
FILTER (NOT EXISTS {?m2 a/rdfs:subClassOf* ?m1}) .
FILTER (NOT EXISTS {?m1 a/rdfs:subClassOf* ?m2}) .
}
""" ] ] ;
    sh:rule [ a sh:SPARQLRule ;
            rdfs:comment "Infer the connectsFrom relationship" ;
            sh:construct """
CONSTRUCT {$this s223:connectsFrom ?equipment .}
WHERE {
$this s223:connectsAt ?cp .
?cp a s223:OutletConnectionPoint .
?cp s223:isConnectionPointOf ?equipment .
}
""" ;
            sh:name "InferredConnectionToUpstreamEquipmentProperty" ;
            sh:prefixes s223: ],
        [ a sh:SPARQLRule ;
            rdfs:comment "Infer the connectsTo relationship" ;
            sh:construct """
CONSTRUCT {$this s223:connectsTo ?equipment .}
WHERE {
$this s223:connectsAt ?cp .
?cp a s223:InletConnectionPoint .
?cp s223:isConnectionPointOf ?equipment .
}
""" ;
            sh:name "InferredConnectionToDownstreamEquipmentProperty" ;
            sh:prefixes s223: ],
        [ a sh:TripleRule ;
            rdfs:comment "Infer cnx relationship from connectsAt",
                "InferredConnectionToConnectionPointBaseProperty" ;
            sh:object [ sh:path s223:connectsAt ] ;
            sh:predicate s223:cnx ;
            sh:subject sh:this ],
        [ a sh:TripleRule ;
            rdfs:comment "Infer cnx relationship from connectsThrough",
                "InferredConnectionToConnectionPointBasePropertyFromInverse" ;
            sh:object [ sh:path [ sh:inversePath s223:connectsThrough ] ] ;
            sh:predicate s223:cnx ;
            sh:subject sh:this ],
        [ a sh:TripleRule ;
            rdfs:comment "Infer the connectsAt relationship from cnx",
                "InferredConnectionToConnectionPointProperty" ;
            sh:object [ sh:path s223:cnx ] ;
            sh:predicate s223:connectsAt ;
            sh:subject sh:this ] .

s223:NumberOfElectricalPhases-SinglePhase a s223:Dimensionless-NumberOfElectricalPhases ;
    rdfs:label "Single Phase AC Electricity" .

s223:Equipment a s223:Class,
        sh:NodeShape ;
    rdfs:label "Equipment" ;
    rdfs:comment "A Equipment is the modeling construct used to represent a mechanical device designed to accomplish a specific task that one might buy from a vendor. Examples of possible devices include a pump, fan, heat exchanger, luminaire, temperature sensor, or flow meter." ;
    rdfs:subClassOf s223:Connectable ;
    sh:property [ a sh:PropertyShape ;
            rdfs:comment "A Equipment can be associated with Equipment using the relation contains" ;
            sh:class s223:Equipment ;
            sh:minCount 0 ;
            sh:name "device contains shape" ;
            sh:path s223:contains ],
        [ rdfs:comment "A Equipment can be associated with an ActuatableProperty using the relation commandedByProperty" ;
            sh:class s223:ActuatableProperty ;
            sh:path s223:commandedByProperty ],
        [ rdfs:comment "A Equipment can be associated with a PhysicalSpace using the relation hasPhysicalLocation" ;
            sh:class s223:PhysicalSpace ;
            sh:path s223:hasPhysicalLocation ],
        [ rdfs:comment "A Equipment can be associated with an EnumerationKind-Role using the relation hasRole" ;
            sh:class s223:EnumerationKind-Role ;
            sh:path s223:hasRole ],
        [ rdfs:comment "Make sure that a containing Equipment inherits the incoming connectedFrom relations of contained Equipment if they are not internal connections." ;
            sh:path s223:connectedFrom ;
            sh:sparql [ a sh:SPARQLConstraint ;
                    rdfs:comment "Make sure that a containing Equipment inherits the incoming connectedFrom relations of contained Equipment if they are not internal connections." ;
                    sh:message "{?container} does not have a connectedFrom relation to {?otherDev} even though {?container} contains {$this} which does." ;
                    sh:prefixes s223: ;
                    sh:select """
SELECT $this ?container ?otherDev
WHERE {
$this s223:connectedFrom ?otherDev .
$this ^s223:contains ?container .
?container a/rdfs:subClassOf* s223:Equipment .
FILTER NOT EXISTS {?container s223:contains ?otherDev .}
FILTER NOT EXISTS {?container s223:connectedFrom ?otherDev .}
}
""" ] ],
        [ rdfs:comment "Make sure that a containing Equipment inherits the outgoing connectedTo relations of contained Equipment if they are not internal connections." ;
            sh:path s223:connectedTo ;
            sh:sparql [ a sh:SPARQLConstraint ;
                    rdfs:comment "Make sure that a containing Equipment inherits the outgoing connectedTo relations of contained Equipment if they are not internal connections." ;
                    sh:message "{?container} does not have a connectedTo relation to {?otherDev} even though {?container} contains {$this} which does." ;
                    sh:prefixes s223: ;
                    sh:select """
SELECT $this ?container ?otherDev
WHERE {
$this s223:connectedTo ?otherDev .
$this ^s223:contains ?container .
?container a/rdfs:subClassOf* s223:Equipment .
FILTER NOT EXISTS {?container s223:contains ?otherDev .}
FILTER NOT EXISTS {?container s223:connectedTo ?otherDev .}
}
""" ] ],
        [ rdfs:comment "Warning about a subClass of Equipment of type A containing something that is in the same subClass branch." ;
            sh:path s223:contains ;
            sh:sparql [ a sh:SPARQLConstraint ;
                    rdfs:comment "Warning about a subClass of Equipment of type A containing something that is in the same subClass branch." ;
                    sh:message "{$this}, of type {?type1}, contains {?subEquip} of type {?type2}, that could result in double-counting items in the class hierarchy of {?type1}." ;
                    sh:prefixes s223: ;
                    sh:select """
SELECT $this ?subEquip ?type1 ?type2
WHERE {
  FILTER NOT EXISTS {$this a s223:Equipment} .
$this s223:contains+ ?subEquip .
  FILTER NOT EXISTS {?subEquip a s223:Equipment} .
$this a ?type1 .
?subEquip a ?type2 .
{
?type2 rdfs:subClassOf* ?type1 .
}
UNION
{
?type1 rdfs:subClassOf* ?type2 .
}
}
""" ;
                    sh:severity sh:Warning ] ] ;
    sh:rule [ a sh:SPARQLRule ;
            rdfs:comment "Infer a higher-level cnx and Medium from the mapsTo relation" ;
            sh:construct """
CONSTRUCT {?parentCp s223:cnx ?connection .
    ?parentCp s223:hasMedium ?medium .
}
WHERE {
  $this s223:hasConnectionPoint ?cp .
  ?cp s223:mapsTo ?parentCp .
  ?cp s223:connectsThrough ?connection .
  ?cp s223:hasMedium ?medium .
}
""" ;
            sh:prefixes s223: ],
        [ a sh:SPARQLRule ;
            rdfs:comment "Infer a lower-level cnx and Medium from the mapsTo relation" ;
            sh:construct """
CONSTRUCT {?childCp s223:cnx ?connection .
    ?childCp s223:hasMedium ?medium .
}
WHERE {
  $this s223:hasConnectionPoint ?cp .
  ?childCp s223:mapsTo ?cp .
  ?cp s223:connectsThrough ?connection .
  ?cp s223:hasMedium ?medium .
}
""" ;
            sh:prefixes s223: ] .

s223:Frequency-60Hz a s223:Dimensioned-Frequency,
        s223:QuantifiableProperty ;
    rdfs:label "60 Hertz" ;
    s223:hasValue 60.0 ;
    qudt:hasQuantityKind quantitykind:Frequency ;
    qudt:hasUnit unit:HZ .

s223:hasMedium a rdf:Property ;
    rdfs:label "has Medium" ;
    rdfs:comment "The relation hasMedium is used to indicate what medium is flowing through the connection (e.g., air, water, electricity). The possible values are defined in EnumerationKind-Medium (see `s223:EnumerationKind-Medium`)." .

s223:Electricity-AC a s223:Class,
        s223:Electricity-AC,
        sh:NodeShape ;
    rdfs:label "Electricity AC" ;
    rdfs:subClassOf s223:Medium-Electricity .

s223:OutletConnectionPoint a s223:Class,
        sh:NodeShape ;
    rdfs:label "Outlet Connection Point" ;
    rdfs:comment "An OutletConnectionPoint indicates that a substance must flow out of the domain space at this connection point and cannot flow in the other direction. An OutletConnectionPoint is a predefined subclass of ConnectionPoint." ;
    rdfs:subClassOf s223:ConnectionPoint ;
    sh:property [ rdfs:comment "An OutletConnectionPoint can be associated with one other OutletConnectionPoint using the relation mapsTo" ;
            sh:class s223:OutletConnectionPoint ;
            sh:path s223:mapsTo ],
        [ rdfs:comment "Ensure an OutletCP does not mapsTo a subordinate OutletCP that is part of an internal Connection" ;
            sh:path s223:mapsTo ;
            sh:sparql [ a sh:SPARQLConstraint ;
                    rdfs:comment "Ensure a CP does not mapsTo a subordinate CP that is part of an internal Connection" ;
                    sh:message "{$this} should not have a mapsTo {?otherCP} because {?otherCP} participates in an internal Connection to {?destinationDevice}." ;
                    sh:prefixes s223: ;
                    sh:select """
SELECT $this ?otherCP ?destinationDevice
WHERE {
$this s223:mapsTo ?otherCP .
?equipment s223:hasConnectionPoint $this .
?otherEquipment s223:hasConnectionPoint ?otherCP .
?otherCP s223:connectsThrough/s223:connectsTo ?destinationDevice .
?destinationDevice s223:contains ?equipment .
}
""" ] ] .

s223:Medium-Air a s223:Class,
        s223:Medium-Air,
        sh:NodeShape ;
    rdfs:label "Medium-Air" ;
    rdfs:subClassOf s223:EnumerationKind-Medium .

s223:InletConnectionPoint a s223:Class,
        sh:NodeShape ;
    rdfs:label "Inlet Connection Point" ;
    rdfs:comment "An InletConnectionPoint indicates that a substance must flow into the equipment or domain space at this connection point and cannot flow the other direction. An IntletConnectionPoint is a subclass of ConnectionPoint." ;
    rdfs:subClassOf s223:ConnectionPoint ;
    sh:property [ rdfs:comment "An InletConnectionPoint can ne associated with one other InletConnectionPoint using the relation mapsTo" ;
            sh:class s223:InletConnectionPoint ;
            sh:path s223:mapsTo ],
        [ rdfs:comment "Ensure an InletCP does not mapsTo a subordinate InletCP that is part of an internal Connection" ;
            sh:path s223:mapsTo ;
            sh:sparql [ a sh:SPARQLConstraint ;
                    rdfs:comment "Ensure a CP does not mapsTo a subordinate CP that is part of an internal Connection" ;
                    sh:message "{$this} should not have a mapsTo {?otherCP} because {?otherCP} participates in an internal Connection from {?destinationDevice}." ;
                    sh:prefixes s223: ;
                    sh:select """
SELECT $this ?otherCP ?destinationDevice
WHERE {
$this s223:mapsTo ?otherCP .
?equipment s223:hasConnectionPoint $this .
?otherEquipment s223:hasConnectionPoint ?otherCP .
?otherCP s223:connectsThrough/s223:connectsFrom ?destinationDevice .
?destinationDevice s223:contains ?equipment .
}
""" ] ] .

s223:hasConnectionPoint a rdf:Property ;
    rdfs:label "has connection point" ;
    s223:inverseOf s223:isConnectionPointOf ;
    rdfs:comment "The relation hasConnectionPoint is part of a pair of relations that bind a Connectable thing to a ConnectionPoint. It is the inverse of the relation isConnectionPointOf (see `s223:isConnectionPointOf`)." .

rdf:Property a sh:NodeShape ;
    sh:property [ rdfs:comment "This Property must have aa label" ;
            sh:path rdfs:label ;
            sh:sparql [ a sh:SPARQLConstraint ;
                    sh:message "{$this} must have an rdfs:label" ;
                    sh:prefixes s223: ;
                    sh:select """
SELECT $this
WHERE {
BIND(REPLACE(STR($this), "^(.*)(/|#)([^#/]*)$", "$1") AS ?prop) .
FILTER (?prop = "http://data.ashrae.org/standard223") .
FILTER (NOT EXISTS {$this rdfs:label ?something}) .
}
""" ] ] .

sh: a owl:Ontology ;
    rdfs:label "W3C Shapes Constraint Language (SHACL) Vocabulary"@en ;
    rdfs:comment "This vocabulary defines terms used in SHACL, the W3C Shapes Constraint Language."@en ;
    sh:declare [ sh:namespace "http://www.w3.org/ns/shacl#" ;
            sh:prefix "sh" ] ;
    sh:suggestedShapesGraph <http://www.w3.org/ns/shacl-shacl#> .

[] sh:minCount 1 .

